@prefix dct: <http://purl.org/dc/terms/> .
@prefix evtAgRole: <http://id.loc.gov/vocabulary/preservation/eventRelatedAgentRole/> .
@prefix evtObjRole: <http://id.loc.gov/vocabulary/preservation/eventRelatedObjectRole/> .
@prefix evtOutcome: <http://id.loc.gov/vocabulary/preservation/eventOutcome/> .
@prefix org: <http://www.w3.org/ns/org#> .
@prefix owl: <http://www.w3.org/2002/07/owl#> .
@prefix pav: <http://purl.org/pav/> .
@prefix premis: <http://www.loc.gov/premis/rdf/v3/> .
@prefix prov: <http://www.w3.org/ns/prov#> .
@prefix rdf: <http://www.w3.org/1999/02/22-rdf-syntax-ns#> .
@prefix rdfs: <http://www.w3.org/2000/01/rdf-schema#> .
@prefix schema: <https://schema.org/> .
@prefix sh: <http://www.w3.org/ns/shacl#> .
@prefix skos: <http://www.w3.org/2004/02/skos/core#> .
@prefix vann: <http://purl.org/vocab/vann/> .
@prefix xsd: <http://www.w3.org/2001/XMLSchema#> .

_:n0eda34ab87e64af8be809e1d9077553ab1 a rdfs:Class,
        owl:Class ;
    owl:unionOf ( skos:Concept skos:Collection ) .

_:na87fcceb263b4ca493cedf23101c1dd8b1 a rdfs:Class,
        owl:Class ;
    owl:unionOf ( premis:RightsStatus premis:Rule ) .

_:na87fcceb263b4ca493cedf23101c1dd8b17 a rdfs:Class,
        owl:Class ;
    owl:unionOf ( premis:RightsStatus premis:Rule ) .

dct:FileFormat a rdfs:Class ;
    rdfs:label "File format"@en,
        "Format de fichier"@fr,
        "Bestandsformaat"@nl ;
    dct:description "Examples include the formats defined by the list of Internet Media Types."@en ;
    dct:hasVersion <http://dublincore.org/usage/terms/history/#FileFormat-001> ;
    dct:issued "2008-01-14"^^xsd:date ;
    rdfs:isDefinedBy dct: ;
    rdfs:subClassOf dct:MediaType ;
    skos:definition "A digital resource format."@en,
        "Un format de ressource numérique."@fr,
        "Een formaat van een digitale bron."@nl .

<http://www.ebu.ch/metadata/ontologies/ebucore/ebucore#Annotation> a rdfs:Class ;
    rdfs:label "Annotation"@en,
        "Annotation"@fr,
        "Annotatie"@nl ;
    rdfs:subClassOf owl:Thing ;
    skos:definition "A class used to annotate Assets."@en,
        "Une classe utilisée pour annoter les éléments."@fr,
        "Een klasse die wordt gebruikt om items te annoteren."@nl .

<http://www.ebu.ch/metadata/ontologies/ebucore/ebucore#TextAnnotation> a rdfs:Class ;
    rdfs:label "Text Annotation"@en,
        "Annotation texte"@fr,
        "Tekstannotatie"@nl ;
    rdfs:subClassOf <http://www.ebu.ch/metadata/ontologies/ebucore/ebucore#Annotation> ;
    skos:definition "A class specific to the annotation of a text or portions of text."@en,
        "Une classe spécifique à l'annotation d'un texte ou de portions de texte."@fr,
        "Een klasse die specifiek is voor de annotatie van een tekst of delen van tekst."@nl .

premis:Agent a rdfs:Class,
        owl:Class ;
    rdfs:label "Agent"@en,
        "Acteur"@fr,
        "Agent"@nl ;
    rdfs:isDefinedBy premis: ;
    rdfs:subClassOf prov:Agent,
        <http://xmlns.com/foaf/0.1/Agent> ;
    skos:definition "Actor (human, machine, or software) associated with one or more Event and/or Rights statement associated with a digital object."@en,
        "Acteur (humain, machine ou logiciel) associé à un ou plusieurs événements (Events) et/ou déclaration(s) de droits associé(s) à un objet numérique."@fr,
        "Agens (mens, machine of software) geassocieerd met één of meer gebeurtenissen (Events) en/of rechtenuitdrukking(en) geassocieerd met een digitaal object."@nl .

premis:Event a rdfs:Class,
        owl:Class ;
    rdfs:label "Event"@en,
        "Événement"@fr,
        "Gebeurtenis"@nl ;
    rdfs:isDefinedBy premis: ;
    rdfs:seeAlso <http://id.loc.gov/vocabulary/preservation/eventType> ;
    rdfs:subClassOf prov:Activity ;
    skos:definition "Action performed within or outside the repository that affects its capability to preserve Objects over the long term."@en,
        "Action réalisée à l'intérieur ou à l'extérieur du dépôt qui affecte sa capacité à préserver des objets sur le long terme."@fr,
        "Handeling uitgevoerd binnen of buiten het archief die het vermogen beïnvloedt om objecten op lange termijn te bewaren."@nl .

premis:File a rdfs:Class,
        owl:Class ;
    rdfs:label "File"@en,
        "Fichier"@fr,
        "Bestand"@nl ;
    rdfs:isDefinedBy premis: ;
    rdfs:subClassOf premis:Object ;
    owl:disjointWith premis:Bitstream,
        premis:IntellectualEntity,
        premis:Representation ;
    skos:definition "Named and ordered sequence of bytes that is known to an operating system."@en,
        "Séquence nommée et ordonnée d'octets/bytes connue par un système d'exploitation."@fr,
        "Genoemde en geordende sequentie van bytes gekend door een besturingssysteem."@nl .

premis:Fixity a rdfs:Class,
        owl:Class ;
    rdfs:label "Fixity"@en,
        "Fixité"@fr,
        "Fixity"@nl ;
    rdfs:isDefinedBy premis: ;
    rdfs:seeAlso <http://id.loc.gov/vocabulary/preservation/cryptographicHashFunctions> ;
    skos:definition "Information used to verify whether an object has been altered in an undocumented or unauthorized way."@en,
        "Informations utilisées pour vérifier si un objet a été modifié de manière non documentée ou non autorisée."@fr,
        "Informatie die wordt gebruikt om na te gaan of een object op een ongedocumenteerde of ongeoorloofde manier werd gewijzigd."@nl .

premis:HardwareAgent a rdfs:Class,
        owl:Class ;
    rdfs:label "Hardware agent"@en,
        "Matériel acteur"@fr,
        "Hardware agent"@nl ;
    rdfs:isDefinedBy premis: ;
    rdfs:subClassOf premis:Agent ;
    owl:disjointWith premis:Organization,
        premis:Person,
        premis:SoftwareAgent ;
    owl:sameAs <http://id.loc.gov/vocabulary/preservation/agentType/har> ;
    skos:definition "Hardware agent (e.g., a computer) that is associated with one or more Events and/or Rights statement associated with a digital object."@en,
        "Agent matériel (par ex. un ordinateur) associé à un ou plusieurs événements (Events) et/ou déclaration(s) de droits associé(s) à un objet numérique."@fr,
        "Hardwareagent (bv. een computer) die gekoppeld is aan één of meer gebeurtenissen (Events) en/of rechtenuitdrukking(en) geassocieerd met een digitaal object."@nl .

premis:IntellectualEntity a rdfs:Class,
        owl:Class ;
    rdfs:label "Intellectual entity"@en,
        "Entité intellectuelle"@fr,
        "Intellectuele entiteit"@nl ;
    rdfs:isDefinedBy premis: ;
    rdfs:seeAlso <http://id.loc.gov/vocabulary/preservation/environmentFunctionType> ;
    rdfs:subClassOf premis:Object ;
    owl:disjointWith premis:Bitstream,
        premis:File,
        premis:Representation ;
    skos:definition "A set of content that is considered a single intellectual unit for purposes of management and description: for example, a particular book, map, photograph, database, or piece of hardware or software. An Intellectual Entity can include other Intellectual Entities; for example, a web site can include a web page; a web page can include an image. An Intellectual Entity may have one or more digital representations. An Intellectual Entity may also describe an environment, defined as technology supporting a digital object in some way (e.g. by rendering or executing it). Environments can consist of software, hardware, or a combination of both."@en,
        "Ensemble de contenu qui est considéré comme une unité intellectuelle pour des objectifs de gestion et de description."@fr,
        "Set van inhoud die beschouwd wordt als één enkele intellectuele eenheid met als doeleinden beheer en beschrijving."@nl .

premis:Object a rdfs:Class,
        owl:Class ;
    rdfs:label "Object"@en,
        "Objet"@fr,
        "Object"@nl ;
    rdfs:isDefinedBy premis: ;
    rdfs:subClassOf prov:Entity ;
    skos:definition "Discrete unit of information subject to digital preservation. Subclasses of Object are Intellectual Entity, Representation, File and Bitstream."@en,
        "Unité discrète d'information soumise à la préservation numérique. Les sous-classes d'objet sont le Intellectual Entity (entité intellectuelle), la Representation (représentation), le File (fichier) et le Bitstream (flux binaire)."@fr,
        "Discrete eenheid van informatie die digitaal moet worden bewaard. Subklassen van Object zijn Intellectual Entity (intellectuele entiteit), Representation (voorstelling/weergave), File (bestand) en Bitstream (bitstream)."@nl .

premis:OutcomeStatus a rdfs:Class,
        owl:Class ;
    rdfs:label "Outcome status"@en,
        "Statut de résultat"@fr,
        "Uitkomststatus"@nl ;
    rdfs:isDefinedBy premis: ;
    rdfs:seeAlso <http://id.loc.gov/vocabulary/preservation/eventOutcome> ;
    skos:definition "Overall result of the Event in terms of success, partial success, or failure."@en,
        "Résultat global de l'événement en termes de succès, de succès partiel ou d'échec."@fr,
        "Algemeen resultaat van het Event in termen van succes, gedeeltelijk succes of falen."@nl .

premis:Representation a rdfs:Class,
        owl:Class ;
    rdfs:label "Representation"@en,
        "Représentation"@fr,
        "Representatie"@nl ;
    rdfs:isDefinedBy premis: ;
    rdfs:subClassOf premis:Object ;
    owl:disjointWith premis:Bitstream,
        premis:File,
        premis:IntellectualEntity ;
    skos:definition "Digital or physical Object instantiating or embodying an Intellectual Entity. A digital representation is the set of stored digital files and structural metadata needed to provide a complete and reasonable rendition of the Intellectual Entity. A physical representation is an item such as a manuscript, video cassette, or printed document."@en,
        "Objet numérique ou physique instanciant ou incarnant une Entité Intellectuelle (Intellectual Entity). Une représentation numérique (Digital Representation) est l'ensemble des fichiers numériques stockés et des métadonnées structurelles nécessaires pour fournir une interprétation complète et raisonnable de l'entité intellectuelle (Intellectual Entity). Une représentation physique (Physical Representation) est un élément tel qu'un manuscrit, une cassette vidéo ou un document imprimé."@fr,
        "Digitaal of fysiek object dat een intellectuele entiteit (Intellectual Entity) vormgeeft of belichaamt. Een digitale weergave (Digital Representation) is de set van opgeslagen digitale bestanden en structurele metadata die nodig zijn om een volledige en redelijke weergave van de Intellectuele Entiteit (Intellectual Entity) te bieden. Een fysieke representatie (Physical Representation) is een item zoals een manuscript, videocassette of gedrukt document."@nl .

premis:SoftwareAgent a rdfs:Class,
        owl:Class ;
    rdfs:label "Software agent"@en,
        "Logiciel acteur"@fr,
        "Software agent"@nl ;
    rdfs:isDefinedBy premis: ;
    rdfs:subClassOf premis:Agent,
        prov:SoftwareAgent ;
    owl:disjointWith premis:HardwareAgent,
        premis:Organization,
        premis:Person ;
    skos:definition "Software agent (e.g., a computer program) that is associated with one or more Event and/or Rights statement associated with a digital object."@en,
        "Agent logiciel (par ex. un programme informatique) associé à un ou plusieurs événements (Events) et/ou déclaration(s) de droits associé(s) à un objet numérique."@fr,
        "Softwareagent (bv. een computerprogramma) die gekoppeld is aan één of meer gebeurtenissen (Events) en/of rechtenuitdrukking(en) geassocieerd met een digitaal object."@nl .

premis:StorageLocation a rdfs:Class,
        owl:Class ;
    rdfs:label "Storage location"@en,
        "Emplacement de stockage"@fr,
        "Opslagplaats"@nl ;
    rdfs:isDefinedBy premis: ;
    rdfs:seeAlso <http://id.loc.gov/vocabulary/preservation/contentLocationType> ;
    skos:definition "Information needed to retrieve a physical item from its physical storage location or a file from the storage system, or to access a bitstream within a file."@en,
        "Informations nécessaires pour extraire un élément physique de son emplacement de stockage physique ou un fichier du système de stockage, ou pour accéder à un flux binaire (bitstream) dans un fichier (file)."@fr,
        "Informatie die nodig is om een fysiek voorwerp van zijn fysieke opslagplaats of een bestand uit het opslagsysteem op te halen, of om toegang te krijgen tot een bitstream binnen een bestand (file)."@nl .

premis:StorageMedium a rdfs:Class,
        owl:Class ;
    rdfs:label "Storage medium"@en,
        "Support de stockage"@fr,
        "Opslagmedium"@nl ;
    rdfs:isDefinedBy premis: ;
    rdfs:seeAlso <http://id.loc.gov/vocabulary/preservation/storageMedium> ;
    skos:definition "The physical medium on which the Object is stored (e.g., magnetic tape, hard disk, CD-ROM, DVD)."@en,
        "Le support physique sur lequel l'Objet (Object) est stocké (par exemple, bande magnétique, le disque dur, le CD-ROM, le DVD)."@fr,
        "Het fysieke medium waarop het Object is opgeslagen (bijvoorbeeld, de magnetische tape, de harde schijf, de CD-ROM, de DVD)."@nl .

rdf:List a rdfs:Class ;
    rdfs:label "List"@en,
        "Liste"@fr,
        "Lijst"@nl ;
    rdfs:isDefinedBy rdf: ;
    rdfs:subClassOf rdfs:Resource ;
    skos:definition "The class of RDF Lists."@en,
        "La classe des listes RDF."@fr,
        "De klasse van RDF-lijsten."@nl .

skos:Collection a rdfs:Class,
        owl:Class ;
    rdfs:label "Collection"@en,
        "Collection"@fr,
        "Verzameling"@nl ;
    rdfs:isDefinedBy <http://www.w3.org/2004/02/skos/core> ;
    owl:disjointWith skos:Concept,
        skos:ConceptScheme ;
    skos:definition "A meaningful collection of concepts."@en,
        "Une collection de concepts ayant un sens."@fr,
        "Een betekenisvolle verzameling van concepten."@nl ;
    skos:scopeNote "Labelled collections can be used where you would like a set of concepts to be displayed under a 'node label' in the hierarchy."@en,
        "Les collections étiquetées peuvent être utilisées pour afficher un ensemble de concepts sous un 'label de nœud' dans la hiérarchie."@fr,
        "Gelabelde verzamelingen kunnen gebruikt worden waar je een set concepten onder een 'node label' in de hiërarchie wilt weergeven."@nl .

skos:Concept a rdfs:Class,
        owl:Class ;
    rdfs:label "Concept"@en,
        "Concept"@fr,
        "Concept"@nl ;
    rdfs:isDefinedBy <http://www.w3.org/2004/02/skos/core> ;
    skos:definition "A SKOS concept can be viewed as an idea or notion; a unit of thought. However, what constitutes a unit of thought is subjective, and this definition is meant to be suggestive, rather than restrictive."@en,
        "Un concept SKOS peut être considéré comme une idée ou une notion, une unité de pensée. Cependant, ce qui constitue une unité de pensée est subjectif, et cette définition se veut suggestive, plutôt que restrictive."@fr,
        "Een SKOS-concept kan als idee of begrip worden gezien; een gedachte-eenheid. Echter, wat  een gedachte-eenheid is, is subjectief, en deze definitie is eerder suggestief dan beperkend bedoeld."@nl .

skos:ConceptScheme a rdfs:Class,
        owl:Class ;
    rdfs:label "Concept scheme"@en,
        "Schéma de concepts"@fr,
        "Conceptenschema"@nl ;
    rdfs:isDefinedBy <http://www.w3.org/2004/02/skos/core> ;
    owl:disjointWith skos:Concept ;
    skos:definition "A set of concepts, optionally including statements about semantic relationships between those concepts."@en,
        "Un ensemble de concepts, éventuellement accompagné de déclarations sur les relations sémantiques entre ces concepts."@fr,
        "Een set van concepten, eventueel vergezeld van verklaringen over de semantische relaties tussen die concepten."@nl ;
    skos:example "Thesauri, classification schemes, subject heading lists, taxonomies, 'folksonomies', and other types of controlled vocabulary are all examples of concept schemes. Concept schemes are also embedded in glossaries and terminologies."@en,
        "Thésaurus, classifications, listes de sujets, taxonomies, 'folksonomies', et d'autres types de vocabulaires contrôlés sont tous des exemples de schémas de concepts. Les schémas de concepts sont aussi intégrés dans les glossaires et les terminologies."@fr,
        "Thesauri, classificaties, onderwerplijsten, taxonomieën, folksonomieën, en andere soorten gecontroleerde vocabularia zijn allemaal voorbeelden van conceptenschema's. Conceptenschema's worden ook ingebed in glossaria en terminologieën."@nl ;
    skos:scopeNote "A concept scheme may be defined to include concepts from different sources."@en,
        "Un schéma de concepts peut être défini pour inclure des concepts provenant de différentes sources."@fr,
        "Een conceptenschema kan gedefinieerd worden om concepten uit verschillende bronnen te bevatten."@nl .

skos:OrderedCollection a rdfs:Class,
        owl:Class ;
    rdfs:label "Ordered collection"@en,
        "Collection ordonnée"@fr,
        "Geordende collectie"@nl ;
    rdfs:isDefinedBy <http://www.w3.org/2004/02/skos/core> ;
    rdfs:subClassOf skos:Collection ;
    skos:definition "An ordered collection of concepts, where both the grouping and the ordering are meaningful."@en,
        "Une collection ordonnée de concepts, où le regroupement et l'ordre sont significatifs."@fr,
        "Een geordende collectie van concepten, waar zowel de groepering als de volgorde betekenisvol zijn."@nl ;
    skos:scopeNote "Ordered collections can be used where you would like a set of concepts to be displayed in a specific order, and optionally under a 'node label'."@en,
        "Les collections ordonnées peuvent être utilisées lorsque vous souhaitez afficher un ensemble de concepts dans un ordre spécifique, et éventuellement sous une \"étiquette de nœud\"."@fr,
        "Geordende collecties kunnen worden gebruikt waar je een set van concepten wilt weergeven in een specifieke volgorde, en optioneel onder een 'knooppuntlabel'."@nl .

<http://www.w3.org/2008/05/skos-xl#Label> a rdfs:Class,
        owl:Class ;
    rdfs:label "Label"@en,
        "Étiquette"@fr,
        "Label"@nl ;
    rdfs:isDefinedBy <http://www.w3.org/2008/05/skos-xl> ;
    rdfs:subClassOf [ a owl:Restriction ;
            owl:cardinality "1"^^xsd:nonNegativeInteger ;
            owl:onProperty <http://www.w3.org/2008/05/skos-xl#literalForm> ] ;
    owl:disjointWith skos:Collection,
        skos:Concept,
        skos:ConceptScheme ;
    skos:definition "A special class of lexical entities."@en,
        "Une classe spéciale d'entités lexicales."@fr,
        "Een speciale klasse van lexicale entiteiten."@nl .

org:Organization a rdfs:Class,
        owl:Class ;
    rdfs:label "Organization"@en,
        "Organisation"@fr,
        "Organisatie"@nl ;
    rdfs:isDefinedBy <http://www.w3.org/ns/org> ;
    rdfs:subClassOf <http://xmlns.com/foaf/0.1/Agent> ;
    owl:disjointWith schema:Person ;
    owl:equivalentClass <http://xmlns.com/foaf/0.1/Organization>,
        schema:Organization ;
    skos:definition "Represents a collection of people organized together into a community or other social, commercial or political structure. The group has some common purpose or reason for existence which goes beyond the set of people belonging to it and can act as an Agent. Organizations are often decomposable into hierarchical structures.  It is recommended that SKOS lexical labels should be used to label the Organization. In particular `skos:prefLabel` for the primary (possibly legally recognized name), `skos:altLabel` for alternative names (trading names, colloquial names) and `skos:notation` to denote a code from a code list. Alternative names: _Collective_ _Body_ _Org_ _Group_"@en,
        "Représente un groupe de personnes organisées en communauté où tout autre forme de structure sociale, commerciale ou politique. Le groupe a un but commun ou une raison d'être qui va au-delà de la somme des personnes qui en font partie et peut agir en tant que `Agent`. Les organisations sont souvent décomposables en structures hiérarchisées. Il est recommandé d'utiliser des labels lexicaux SKOS pour nommer l'Organisation. En particulier `skos:prefLabel` pour le nom principal (en général le nom légal), `skos:altLabel` pour les noms alternatifs (marques, sigles, appellations familières) et `skos:notation` pour indiquer un code provenant d'une liste de codes."@fr,
        "Stelt een groep personen voor, georganiseerd in een gemeenschap of een andere sociale, commerciële of politieke structuur. De groep heeft een gemeenschappelijk doel of reden van bestaan dat verder gaat dan de som van de mensen die ertoe behoren en kan handelen als `Agent`. De organisaties zijn vaak onder te verdelen in hiërarchische structuren. Het wordt aanbevolen om SKOS labels te gebruiken om de organisatie te benoemen. In het bijzonder `skos:prefLabel` voor de primaire (mogelijks juridisch geldende) naam, `skos:altLabel` voor alternatieve namen (handelsnamen, colloquialismen) en `skos:notation` om een code aan te duiden uit een codelijst."@nl .

org:OrganizationalUnit a rdfs:Class,
        owl:Class ;
    rdfs:label "OrganizationalUnit"@en,
        "Unité opérationnelle"@fr,
        "Organisatie-eenheid"@nl ;
    rdfs:isDefinedBy <http://www.w3.org/ns/org> ;
    rdfs:subClassOf org:Organization ;
    skos:definition "An Organization such as a University Support Unit which is part of some larger FormalOrganization and only has full recognition within the context of that FormalOrganization, it is not a Legal Entity in its own right. Units can be large and complex containing other Units and even FormalOrganizations. Alternative names: _OU_ _Unit_ _Department_"@en,
        "Une organisation (par exemple le support informatique d'une université) qui fait partie d'une Organisation Formelle plus importante et qui ne peut être reconnue qu'en tant que membre de cette organisation supérieure, ce n'est pas une entité légale en elle-même. Les unités opérationnelles peuvent être étendues, complexes et inclure elles-mêmes d'autres branches ou Unités Opérationnelles, voire des Organisations Formelles."@fr,
        "Een organisatie zoals een afdeling of dienst die deel uitmaakt van de grotere organisatie en zijn bestaansreden daaraan ontleent. Heeft geen juridische status op zich."@nl .

org:Post a rdfs:Class,
        owl:Class ;
    rdfs:label "Post"@en,
        "Poste"@fr,
        "Positie"@nl ;
    rdfs:isDefinedBy <http://www.w3.org/ns/org> ;
    skos:definition "A Post represents some position within an organization that exists independently of the person or persons filling it. Posts may be used to represent situations where a person is a member of an organization ex officio (for example the Secretary of State for Scotland is part of UK Cabinet by virtue of being Secretary of State for Scotland, not as an individual person). A post can be held by multiple people and hence can be treated as a organization in its own right."@en,
        "Un Poste représente une position au sein d'une Organisation qui existe indépendamment de la personne ou des personnes qui le remplissent. Les postes peuvent être utilisés pour représenter des situations où une personne est membre d'une Organisation d'office (par exemple, le Secrétaire d'Etat pour l'Ecosse fait partie du Cabinet du Royaume-Uni du fait d'être Secrétaire d'Etat pour l'Ecosse, non pas comme une personne physique). Un poste après peut être occupé par plusieurs personnes et peut donc être considéré comme une Organisation à part entière."@fr,
        "Functie binnen een organisatie, kan bestaan los van de persoon/personen die ze invult/invullen."@nl .

org:Role a rdfs:Class,
        owl:Class ;
    rdfs:label "Role"@en,
        "Rôle"@fr,
        "Rol"@nl ;
    rdfs:isDefinedBy <http://www.w3.org/ns/org> ;
    rdfs:subClassOf skos:Concept ;
    skos:definition "Denotes a role that a Person or other Agent can take in an organization. Instances of this class describe the abstract role; to denote a specific instance of a person playing that role in a specific organization use an instance of `org:Membership`. It is common for roles to be arranged in some taxonomic structure and we use SKOS to represent that. The normal SKOS lexical properties should be used when labelling the Role. Additional descriptive properties for the Role, such as a Salary band, may be added by extension vocabularies."@en,
        "Indique le rôle qu'une Personne ou un autre Agent peut avoir dans une Organisation. Les instances de cette classe décrivent le rôle dans l'absolu; pour indiquer une personne ayant ce rôle spécifique dans une Organisation, utilisez une instance de `org:Membership`. Il est courant que les rôles soient organisés dans une sorte de taxonomie, ce qui peut être représenté avec SKOS. Les propriétés de libellés standards de SKOS devraient être utilisées pour libeller le Rôle. D'autres propriétés additionnelles pour ce rôle, comme une fourchette de Salaire peuvent être ajoutées par une extension de ce vocabulaire."@fr,
        "Rol die een persoon of agent kan vervullen in een organisatie."@nl .

org:Site a rdfs:Class,
        owl:Class ;
    rdfs:label "Site"@en,
        "Site"@fr,
        "Vestiging"@nl ;
    rdfs:isDefinedBy <http://www.w3.org/ns/org> ;
    skos:definition "An office or other premise at which the organization is located. Many organizations are spread across multiple sites and many sites will host multiple locations. In most cases a Site will be a physical location. However, we don't exclude the possibility of non-physical sites such as a virtual office with an associated post box and phone reception service. Extensions may provide subclasses to denote particular types of site."@en,
        "Un établissement ou tout autre lieu dans lequel une Organisation est localisé. Beaucoup d'organisations sont dispersées à travers plusieurs sites. Dans la plupart des cas un Site sera un lieu physique. Toutefois, nous n'excluons pas la possibilité de sites non-physiques comme un bureau virtuel avec une boîte postale et un service de secrétariat mutualisé. Des extensions pourraient fournir des sous-classes pour décrire des types de sites particuliers."@fr,
        "Een kantoor of ander pand waar een organisatie gevestigd is. Organisaties kunnen over meerdere vestigingen verspreid zijn en vestigingen kunnen op meerdere locaties betrekking hebben."@nl .

prov:Activity a rdfs:Class,
        owl:Class ;
    rdfs:label "Activity"@en,
        "Activité"@fr,
        "Activiteit"@nl ;
    rdfs:isDefinedBy <http://www.w3.org/ns/prov-o#> ;
    owl:disjointWith prov:Entity ;
    skos:definition "An activity is something that occurs over a period of time and acts upon or with entities; it may include consuming, processing, transforming, modifying, relocating, using, or generating entities."@en,
        "Une activité est quelque chose qui se passe pendant un certain temps et qui agit sur/avec des entités. Cela peut inclure la consommation, le traitement, la transformation, la modification, le déplacement, l'utilisation ou la génération d'entités."@fr,
        "Een activiteit is iets dat zich gedurende een bepaalde periode voordoet en op/met entiteiten handelt. Het kan onder meer volgende zaken inhouden: consumeren, verwerken, transformeren, wijzigen, verplaatsen, gebruiken of genereren van entiteiten."@nl .

prov:Agent a rdfs:Class,
        owl:Class ;
    rdfs:label "Agent"@en,
        "Agent"@fr,
        "Agent"@nl ;
    rdfs:isDefinedBy <http://www.w3.org/ns/prov-o#> ;
    owl:disjointWith prov:InstantaneousEvent ;
    skos:definition "An agent is something that bears some form of responsibility for an activity taking place, for the existence of an entity, or for another agent's activity. "@en,
        "Un agent est quelque chose qui porte une forme de responsabilité pour une activité qui se passe, pour l'existence d'une entité ou pour l'activité d'un autre agent. "@fr,
        "Een agent is iets dat een bepaalde vorm van verantwoordelijkheid voor een activiteit neemt, voor het bestaan van een entiteit of voor de activiteit van een andere agent. "@nl .

prov:Entity a rdfs:Class,
        owl:Class ;
    rdfs:label "Entity"@en,
        "Entité"@fr,
        "Entiteit"@nl ;
    rdfs:isDefinedBy <http://www.w3.org/ns/prov-o#> ;
    owl:disjointWith prov:InstantaneousEvent ;
    skos:definition "An entity is a physical, digital, conceptual, or other kind of thing with some fixed aspects; entities may be real or imaginary. "@en,
        "Une entité est un objet physique, numérique, conceptuel ou autre de type fixe ; les entités peuvent être réelles ou imaginaires."@fr,
        "Een entiteit is een fysiek, digitaal, conceptueel of een ander soort ding met enkele vaste aspecten; entiteiten kunnen echt of denkbeeldig zijn."@nl .

<https://data.hetarchief.be/ns/description/Audio> a rdfs:Class ;
    rdfs:label "Audio"@en,
        "Audio"@fr,
        "Audio"@nl ;
    rdfs:isDefinedBy <https://data.hetarchief.be/ns/description/> ;
    rdfs:subClassOf premis:IntellectualEntity ;
    skos:definition "This class applies to media in meemoo's archive that is originally derived from digital born audio or an analog carrier of type audio."@en,
        "Cette classe s'applique aux médias dans les archives de meemoo qui proviennent à l'origine de l'audio né numérique ou à l'origine d'un support analogue du type audio."@fr,
        "Deze klasse is van toepassing op media in meemoo's archief dat oorspronkelijk afkomstig is van digitaal geboren audio of dat oorspronkelijk afkomstig is van een analoge drager van het type audio."@nl .

<https://data.hetarchief.be/ns/description/AudioReel> a rdfs:Class ;
    rdfs:label "Audio reel"@en,
        "Bobine audio"@fr,
        "Geluidsspoel"@nl ;
    rdfs:isDefinedBy <https://data.hetarchief.be/ns/description/> ;
    skos:definition "A reel of an analog film carrier that contains audio."@en,
        "Une bobine d'un porte-film analogique qui contient de l'audio."@fr,
        "Een band van een analoge film drager die audio bevat."@nl .

<https://data.hetarchief.be/ns/description/DVD> a rdfs:Class ;
    rdfs:label "DVD"@en,
        "DVD"@fr,
        "Dvd"@nl ;
    rdfs:isDefinedBy <https://data.hetarchief.be/ns/description/> ;
    rdfs:subClassOf premis:IntellectualEntity ;
    skos:definition "This class applies to media in meemoo's archive that is originally derived from an analog carrier of type DVD, and represents the DVD as a whole."@en,
        "Cette classe s'applique aux médias dans les archives de meemoo qui proviennent à l'origine d'un support analogue du type DVD, et représentent le DVD dans son ensemble."@fr,
        "Deze klasse is van toepassing op media in meemoo's archief dat oorspronkelijk afkomstig is van een analoge drager van het type dvd, en de dvd als geheel voorstelt."@nl .

<https://data.hetarchief.be/ns/description/DVDChapter> a rdfs:Class ;
    rdfs:label "DVD chapter"@en,
        "Chapitre DVD"@fr,
        "Dvd-hoofdstuk"@nl ;
    rdfs:isDefinedBy <https://data.hetarchief.be/ns/description/> ;
    rdfs:subClassOf premis:IntellectualEntity ;
    skos:definition "This class applies to media in meemoo's archive that is originally derived from an analog carrier of type DVD, and represents a specific DVD chapter."@en,
        "Cette classe s'applique aux médias des archives de meemoo qui proviennent à l'origine d'un support analogue du type DVD, et représentent un chapitre DVD spécifique."@fr,
        "Deze klasse is van toepassing op media in meemoo's archief dat oorspronkelijk afkomstig is van een analoge drager van het type dvd, en een specifiek dvd-hoofdstuk voorstelt."@nl .

<https://data.hetarchief.be/ns/description/Film> a rdfs:Class ;
    rdfs:label "Film"@en,
        "Film"@fr,
        "Film"@nl ;
    rdfs:isDefinedBy <https://data.hetarchief.be/ns/description/> ;
    rdfs:subClassOf premis:IntellectualEntity ;
    skos:definition "This class applies to media in meemoo's archive that is originally derived from an analog carrier of type film."@en,
        "Cette classe s'applique aux médias dans les archives de meemoo qui proviennent à l'origine d'un support analogue du type film."@fr,
        "Deze klasse is van toepassing op media in meemoo's archief dat oorspronkelijk afkomstig is van een analoge drager van het type film."@nl .

<https://data.hetarchief.be/ns/description/Image> a rdfs:Class ;
    rdfs:label "Image"@en,
        "Image"@fr,
        "Afbeelding"@nl ;
    rdfs:isDefinedBy <https://data.hetarchief.be/ns/description/> ;
    rdfs:subClassOf premis:IntellectualEntity ;
    skos:definition "This class applies to media in meemoo's archive that is originally derived from a digital born image or an analog carrier of type image."@en,
        "Cette classe s'applique aux médias dans les archives de meemoo qui proviennent à l'origine d'une image née numérique ou d'un support analogue du type vidéo."@fr,
        "Deze klasse is van toepassing op media in meemoo's archief dat oorspronkelijk afkomstig is van een digitaal geboren afbeelding of van een analoge drager van het type afbeelding."@nl .

<https://data.hetarchief.be/ns/description/ImageReel> a rdfs:Class ;
    rdfs:label "Image reel"@en,
        "Bobine d'image"@fr,
        "Beeldspoel"@nl ;
    rdfs:isDefinedBy <https://data.hetarchief.be/ns/description/> ;
    skos:definition "A reel of an analog film carrier that contains video."@en,
        "Une bobine d'un porte-film analogique qui contient une vidéo."@fr,
        "Een speo van een analoge film drager die beeld bevat."@nl .

<https://data.hetarchief.be/ns/description/NewspaperIssue> a rdfs:Class ;
    rdfs:label "Newspaper edition"@en,
        "Edition de journal"@fr,
        "Kranteneditie"@nl ;
    rdfs:isDefinedBy <https://data.hetarchief.be/ns/description/> ;
    rdfs:subClassOf premis:IntellectualEntity ;
    skos:definition "This class applies to media in meemoo's archive that is originally derived from an analog carrier of type newspaper, and represents the newspaper edition as a whole."@en,
        "Cette classe s'applique aux médias dans les archives de meemoo qui proviennent à l'origine d'un support analogue du type journal, et représentent l'édition du journal dans son ensemble."@fr,
        "Deze klasse is van toepassing op media in meemoo's archief dat oorspronkelijk afkomstig is van een analoge drager van het type krant, en de kranteneditie als geheel voorstelt."@nl .

<https://data.hetarchief.be/ns/description/NewspaperIssuePage> a rdfs:Class ;
    rdfs:label "Newspaper issue page"@en,
        "Page d'édition de journal"@fr,
        "Kranteneditiepagina"@nl ;
    rdfs:isDefinedBy <https://data.hetarchief.be/ns/description/> ;
    rdfs:subClassOf premis:IntellectualEntity ;
    skos:definition "This class applies to media in meemoo's archive that is originally derived from an analog carrier of type newspaper, and represents a specific newspaper page."@en,
        "Cette classe s'applique aux médias des archives de meemoo qui proviennent à l'origine d'un support analogue du type journal, et représentent une page de journal spécifique."@fr,
        "Deze klasse is van toepassing op media in meemoo's archief dat oorspronkelijk afkomstig is van een analoge drager van het type krant, en een specifieke krantenpagina voorstelt."@nl .

<https://data.hetarchief.be/ns/description/SilentFilm> a rdfs:Class ;
    rdfs:label "Silent film"@en,
        "Film muet"@fr,
        "Stomme film"@nl ;
    rdfs:isDefinedBy <https://data.hetarchief.be/ns/description/> ;
    rdfs:subClassOf <https://data.hetarchief.be/ns/description/Film> ;
    skos:definition "This class applies to media in meemoo's archive that is originally derived from an analog carrier for silent film."@en,
        "Cette classe s'applique aux médias dans les archives de meemoo qui proviennent à l'origine d'un support analogue pour le film muet."@fr,
        "Deze klasse is van toepassing op media in meemoo's archief dat oorspronkelijk afkomstig is van een analoge drager voor stomme film."@nl .

<https://data.hetarchief.be/ns/description/SoundFilm> a rdfs:Class ;
    rdfs:label "Sound film"@en,
        "Film sonore"@fr,
        "Geluidsfilm"@nl ;
    rdfs:isDefinedBy <https://data.hetarchief.be/ns/description/> ;
    rdfs:subClassOf <https://data.hetarchief.be/ns/description/Film> ;
    skos:definition "This class applies to media in meemoo's archive that is originally derived from an analog carrier for sound film."@en,
        "Cette classe s'applique aux médias dans les archives de meemoo qui proviennent à l'origine d'un support analogue pour le film sonore."@fr,
        "Deze klasse is van toepassing op media in meemoo's archief dat oorspronkelijk afkomstig is van een analoge drager voor geluidsfilm."@nl .

<https://data.hetarchief.be/ns/description/Video> a rdfs:Class ;
    rdfs:label "Video"@en,
        "Vidéo"@fr,
        "Video"@nl ;
    rdfs:isDefinedBy <https://data.hetarchief.be/ns/description/> ;
    rdfs:subClassOf premis:IntellectualEntity ;
    skos:definition "This class applies to media in meemoo's archive that is originally derived from digital born video or an analog carrier of type video."@en,
        "Cette classe s'applique aux médias dans les archives de meemoo qui proviennent à l'origine de la vidéo née numérique ou à l'origine d'un support analogue du type vidéo."@fr,
        "Deze klasse is van toepassing op media in meemoo's archief dat oorspronkelijk afkomstig is van digitaal geboren video of dat oorspronkelijk afkomstig is van een analoge drager van het type video."@nl .

<https://data.hetarchief.be/ns/mediahaven/Fragment> a rdfs:Class ;
    rdfs:label "Mediahaven fragment"@en,
        "Fragment Mediahaven"@fr,
        "Mediahavenfragment"@nl ;
    rdfs:isDefinedBy <https://data.hetarchief.be/ns/mediahaven/> ;
    skos:definition "A fragment in the Mediahaven asset management system."@en,
        "Un fragment dans le système de gestion d'actifs Mediahaven."@fr,
        "Een fragment in het Mediahaven asset management systeem."@nl .

<https://data.hetarchief.be/ns/mediahaven/Record> a rdfs:Class ;
    rdfs:label "Mediahaven record"@en,
        "Enregistrement Mediahaven"@fr,
        "Mediahavenrecord"@nl ;
    rdfs:isDefinedBy <https://data.hetarchief.be/ns/mediahaven/> ;
    skos:definition "A record in the Mediahaven asset management system."@en,
        "Un enregistrement dans le système de gestion d'actifs Mediahaven."@fr,
        "Een record in het Mediahaven asset management systeem."@nl .

<https://data.hetarchief.be/ns/object/CarrierRepresentation> a rdfs:Class ;
    rdfs:label "Carrier representation"@en,
        "Représentation de porteur"@fr,
        "Drager representatie"@nl ;
    rdfs:isDefinedBy <https://data.hetarchief.be/ns/object/> ;
    rdfs:subClassOf premis:Representation ;
    skos:definition "A physical or digital representation of an archived intellectual entity that is stored on a physical carrier such as a video tape, film reel, paper or canvas."@en,
        "Une représentation physique ou numérique d'une entité intellectuelle (Intellectual Entity) archivée qui est stockée sur un porteur physique tel qu'une bande vidéo, une bobine de film, du papier ou une toile."@fr,
        "Een fysieke of digitale weergave van een gearchiveerde intellectuele entiteit (Intellectual Entity) die is opgeslagen op een fysieke drager zoals een videoband, filmrol, papier of canvas."@nl .

<https://data.hetarchief.be/ns/object/DigitalRepresentation> a rdfs:Class ;
    rdfs:label "Digital representation"@en,
        "Représentation digitale"@fr,
        "Digitale representatie"@nl ;
    rdfs:isDefinedBy <https://data.hetarchief.be/ns/object/> ;
    rdfs:subClassOf premis:Representation ;
    skos:definition "Digital representation of an archived intellectual entity."@en,
        "Représentation digitale d'une entité intellectuelle (Intellectual Entity) archivée."@fr,
        "Digitale representatie van een gearchiveerde intellectuele entiteit (Intellectual Entity)."@nl .

<https://data.hetarchief.be/ns/object/FragmentRepresentation> a rdfs:Class ;
    rdfs:label "Fragment representation"@en,
        "Représentation fragment"@fr,
        "Fragment representatie"@nl ;
    rdfs:isDefinedBy <https://data.hetarchief.be/ns/object/> ;
    rdfs:subClassOf premis:DigitalRepresentation ;
    owl:equivalentClass <http://www.ebu.ch/metadata/ontologies/ebucore/ebucore#MediaFragment> ;
    skos:definition "A spatial or temporal segment of a file that serves as a partial digital representation of an archived Intellectual Entity."@en,
        "Un segment spatial ou temporel d'un fichier qui sert de représentation numérique partielle d'une entité intellectuelle archivée."@fr,
        "Een spatiaal of temporeel segment van een bestand die fungeert als een partiële digitale representatie van een gearchiveerde intellectuele entiteit (Intellectual Entity)."@nl .

<https://data.hetarchief.be/ns/object/LocalIdentifier> a rdfs:Class ;
    rdfs:label "Local identifier"@en,
        "Identifiant local"@fr,
        "Lokale identificatie"@nl ;
    rdfs:isDefinedBy <https://data.hetarchief.be/ns/object/> ;
    rdfs:subClassOf premis:Identifier,
        skos:Concept ;
    skos:definition "A local identifier for an object defined by or known to the content partner, such as a barcode, an identifier from an external database or the identifier in the contentpartner's collection registration system."@en,
        "Un identifiant local pour un objet défini par ou connu par le partenaire de contenu, par exemple un code barre, un identifiant d'une base de données externe ou l'identifiant dans le système d'enregistrement de collection du partenaire de contenu."@fr,
        "Een lokale identificatie voor een object gedefinieerd door of bekend bij de contentpartner, bijvoorbeeld een barcode, een identificatie uit een externe database of de identificatie in het registratiesysteem van de collectie van de contentpartner."@nl .

<https://data.hetarchief.be/ns/object/PhysicalCarrier> a rdfs:Class ;
    rdfs:label "Physical carrier"@en,
        "Porteur physique"@fr,
        "Fysieke drager"@nl ;
    rdfs:isDefinedBy <https://data.hetarchief.be/ns/object/> ;
    rdfs:subClassOf premis:StorageLocation ;
    skos:definition "A physical carrier in which data, sound, images, etc., are stored.  For certain categories of material, the physical carrier consists of a storage medium (e.g., tape, film) sometimes encased in a plastic, metal, etc., housing (e.g., cassette, cartridge) that is an integral part of the item."@en,
        "Un porteur physique dans lequel les données, le son, les images, etc., sont stockées.Pour certaines catégories de matériaux, le support physique se compose d'un support de stockage (par exemple, du ruban adhésif, du film) parfois enfermé dans un boîtier en plastique, en métal, etc., (par exemple, cassette, cartouche) qui fait partie intégrante de l'article."@fr,
        "Een fysieke drager waarop data, geluid, beeld etc. zijn opgeslagen. Voor bepaalde materiaalcategorieën bestaat de fysieke drager uit een opslagmedium (bijv. tape, film), soms verpakt in een plastic, metalen, enz. behuizing (bijv. cassette, cartridge) die een integraal onderdeel vormt van het item."@nl .

<https://data.hetarchief.be/ns/organization/ContentPartner> a rdfs:Class ;
    rdfs:label "Content partner"@en,
        "Partenaire de contenus"@fr,
        "Contentpartner"@nl ;
    rdfs:isDefinedBy <https://data.hetarchief.be/ns/organization/> ;
    rdfs:subClassOf org:Organization ;
    skos:definition "A content partner is an organization that has signed a collaboration agreement with meemoo for the long-term preservation and dissemination of their content."@en,
        "Un partenaire de contenu est une organisation qui a signé une convention de collaboration avec meemoo pour la préservation à long terme et la diffusion de leur contenu."@fr,
        "Een contentpartner is een organisatie die een samenwerkingovereenkomst heeft ondertekend met meemoo voor de langetermijnpreservatie en ontsluiting van hun materiaal."@nl .

<https://data.hetarchief.be/ns/organization/DigitizationPartner> a rdfs:Class ;
    rdfs:label "Digitization partner"@en,
        "Partenaire de digitalisation"@fr,
        "Digitaliseringspartner"@nl ;
    rdfs:isDefinedBy <https://data.hetarchief.be/ns/organization/> ;
    rdfs:subClassOf org:ServiceProvider ;
    skos:definition "An organization that provides digitisation services to meemoo."@en,
        "Une organisation qui fournit des services de digitalisation à meemoo."@fr,
        "Een organisatie die aan meemoo digitaliseringsdiensten levert."@nl .

<https://data.hetarchief.be/ns/organization/EducationalPartner> a rdfs:Class ;
    rdfs:label "Educational partner"@en,
        "Partenaire éducatif"@fr,
        "Educatieve partner"@nl ;
    rdfs:isDefinedBy <https://data.hetarchief.be/ns/organization/> ;
    rdfs:subClassOf org:Organization ;
    skos:definition "An educational partner is an organization that provides content on the 'Archief voor Onderwijs' platform and has signed the 'educational partner' collaboration agreement with meemoo (e.g. an educational publisher, KlasCement, Mediawijs, etc.)."@en,
        "Un partenaire éducatif est une organisation qui fournit du contenu sur la plateforme 'Archief voor Onderwijs' et a signé avec meemoo l'accord de collaboration 'partenaire éducatif' (par exemple, un éditeur scolaire, KlasCement, Mediawijs, etc.)."@fr,
        "Een educatieve partner is een organisatie die content aanbiedt op het 'Archief voor Onderwijs'-platform en met meemoo de samenwerkingsovereenkomst 'educatieve partner' heeft ondertekend (bv. een educatieve uitgeverij, KlasCement, Mediawijs, enz.)."@nl .

<https://data.hetarchief.be/ns/organization/Logo> a rdfs:Class ;
    rdfs:label "Logo"@en,
        "Logo"@fr,
        "Logo"@nl ;
    rdfs:isDefinedBy <https://data.hetarchief.be/ns/organization/> ;
    rdfs:subClassOf schema:ImageObject ;
    skos:definition "A logo is a graphic mark, emblem, or symbol of an organization."@en,
        "Un logo est une marque, un emblème ou un symbole graphique d'une organisation."@fr,
        "Een logo is een grafisch teken, embleem of symbool van een organisatie."@nl .

<https://data.hetarchief.be/ns/organization/OrganizationType> a rdfs:Class ;
    rdfs:label "Organization type"@en,
        "Type de organisation"@fr,
        "Organisatietype"@nl ;
    rdfs:isDefinedBy <https://data.hetarchief.be/ns/organization/> ;
    rdfs:subClassOf skos:Concept ;
    skos:definition "The type or classification of an organization."@en,
        "Le type ou la classification d'une organisation."@fr,
        "Het type of de classificatie van een organisatie."@nl .

<https://data.hetarchief.be/ns/organization/ProjectPartner> a rdfs:Class ;
    rdfs:label "Project partner"@en,
        "Partenaire de projet"@fr,
        "Projectpartner"@nl ;
    rdfs:isDefinedBy <https://data.hetarchief.be/ns/organization/> ;
    rdfs:subClassOf org:Organization ;
    skos:definition "An organization that collaborates with meemoo on projects formalized in an agreement or decision, such as projects within the Flemish cultural heritage decree, projects funded by the European Union, or other innovation and research projects."@en,
        "Une organisation qui collabore avec meemoo sur des projets formalisés dans un accord ou une décision, tels que des projets relevant du décret flamand sur le patrimoine culturel, des projets financés par l'Union européenne ou d'autres projets d'innovation et de recherche."@fr,
        "Een organisatie die samenwerkt met meemoo aan projecten die geformaliseerd zijn in een overeenkomst of besluit, zoals bijvoorbeeld projecten binnen het Vlaamse cultureelerfgoeddecreet, projecten onder financiering van de Europese Unie, of andere innovatie- en onderzoeksprojecten."@nl .

<https://data.hetarchief.be/ns/organization/ServiceConsumer> a rdfs:Class ;
    rdfs:label "Service consumer"@en,
        "Consomatteur de services"@fr,
        "Dienstenafnemer"@nl ;
    rdfs:isDefinedBy <https://data.hetarchief.be/ns/organization/> ;
    rdfs:subClassOf org:Organization ;
    skos:definition "An organization that consumes services from meemoo, with a contractual relationship with meemoo. This is not a content partner, but a private organization that stores digital content at meemoo (e.g. Plantentuin Meise)."@en,
        "Une organisation qui consomme des services de meemoo, avec une relation contractuelle avec meemoo. Ce n'est pas un partenaire de contenu, mais une organisation privée qui stocke du contenu numérique chez meemoo (par exemple Plantentuin Meise)."@fr,
        "Een organisatie die diensten bij meemoo afneemt, met contractuele relatie met meemoo. Het gaat hier niet over een contentpartner, maar over een particuliere organisatie die digitale opslag doet bij meemoo (bv. Plantentuin Meise)."@nl .

<https://data.hetarchief.be/ns/organization/ServiceProvider> a rdfs:Class ;
    rdfs:label "Service provider"@en,
        "Fournisseur de services"@fr,
        "Dienstenleverancier"@nl ;
    rdfs:isDefinedBy <https://data.hetarchief.be/ns/organization/> ;
    rdfs:subClassOf org:Organization ;
    skos:definition "An organization that provides services or goods to meemoo, for example related to IT, digitization, etc."@en,
        "Une organisation qui fournit des services ou des biens à meemoo, par exemple dans le domaine de l'informatique, de la numérisation, etc."@fr,
        "Een organisatie die aan meemoo diensten of goederen levert, bijvoorbeeld op het gebied van IT, digitalisering, enz."@nl .

schema:ArchiveComponent a rdfs:Class ;
    rdfs:label "Archive component"@en,
        "Composant d'archive"@fr,
        "Archiefcomponent"@nl ;
    rdfs:isDefinedBy schema: ;
    rdfs:subClassOf schema:CreativeWork ;
    skos:definition "An intangible type to be applied to any archive content, carrying with it a set of properties required to describe archival items and collections."@en,
        "Un type intangible à appliquer à tout contenu d'archives, portant avec lui un ensemble de propriétés nécessaires pour la description d'éléments d'archives et de collections."@fr,
        "Een immaterieel type dat toegepast moet worden op elke inhoud van het archief, met daarbij een set van eigenschappen die nodig zijn om archiefitems en -collecties te beschrijven."@nl .

schema:Collection a rdfs:Class ;
    rdfs:label "Collection"@en,
        "Collection"@fr,
        "Collectie"@nl ;
    rdfs:isDefinedBy schema: ;
    rdfs:subClassOf schema:CreativeWork ;
    skos:definition "A collection of items, e.g. creative works or products, typically but not necessarily of the same kind."@en,
        "Une collection d'articles, par exemple des œuvres créatives (creative works) ou des produits, généralement mais pas nécessairement de même type."@fr,
        "Een collectie van items, bv. creatieve werken (creative works) of producten, gewoonlijk maar niet altijd van dezelfde soort."@nl .

schema:ContactPoint a rdfs:Class ;
    rdfs:label "Contact point"@en,
        "Point de contact"@fr,
        "Aanspreek-/meldpunt"@nl ;
    rdfs:isDefinedBy schema: ;
    rdfs:subClassOf schema:StructuredValue ;
    skos:definition "A contact point, for example a Customer Complaints department."@en,
        "Un point de contact, par exemple un département des plaintes clients."@fr,
        "Een aanspreekpunt, zoals een afdeling voor klachten van klanten."@nl .

schema:Country a rdfs:Class ;
    rdfs:label "Country"@en,
        "Pays"@fr,
        "Land"@nl ;
    rdfs:comment "A country."@en,
        "Un pays."@fr,
        "Een land."@nl ;
    rdfs:isDefinedBy schema: ;
    rdfs:subClassOf schema:AdministrativeArea .

schema:CreativeWork a rdfs:Class ;
    rdfs:label "Creative work"@en,
        "Travail créatif"@fr,
        "Creatief werk"@nl ;
    rdfs:isDefinedBy schema: ;
    rdfs:subClassOf schema:Thing ;
    skos:definition "The most generic kind of creative work, including books, movies, photographs, software programs, etc."@en,
        "La plus générique des types de travail créatif (CreativeWork), y compris les livres, les films, les photos, les logiciels, etc."@fr,
        "De meest generieke soort van creatief werk (CreativeWork), zoals boeken, films, foto's, programma's, enz."@nl .

schema:CreativeWorkSeason a rdfs:Class ;
    rdfs:label "Creative work season"@en,
        "Saison du travail créatif"@fr,
        "Creatief werk seizoen"@nl ;
    rdfs:isDefinedBy schema: ;
    rdfs:subClassOf schema:CreativeWork ;
    skos:definition "A media season e.g. tv, radio, video game etc."@en,
        "Une saison médiatique, par exemple tv, radio, jeu vidéo etc."@fr,
        "Een mediaseizoen, bijvoorbeeld tv, radio, videogame etc."@nl .

schema:CreativeWorkSeries a rdfs:Class ;
    rdfs:label "Creative work series"@en,
        "Série du travail créatif"@fr,
        "Serie van het creatief werk"@nl ;
    rdfs:isDefinedBy schema: ;
    rdfs:subClassOf schema:CreativeWork ;
    skos:definition "A CreativeWorkSeries in schema.org is a group of related items, typically but not necessarily of the same kind. CreativeWorkSeries are usually organized into some order, often chronological. Unlike ItemList which is a general purpose data structure for lists of things, the emphasis with CreativeWorkSeries is on published materials (written e.g. books and periodicals, or media such as tv, radio and games)."@en,
        "Un CreativeWorkSeries dans schema.org est une série d'objets, typiquement mais pas forcément du même type. CreativeWorkSeries sont généralement organisées dans un certain ordre, souvent chronologique. Contrairement à ItemList, l'importance des CreativeWorkSeries est sur les matériaux publiés (par exemple des livres et des périodiques, ou des médias tels que tv, radio et jeux vidéo)."@fr,
        "Een CreativeWorkSeries in schema.org is een groep vergelijkbare items, meestal maar niet altijd van dezelfde soort. CreativeWorkSeries zijn meestal gegroepeerd in een bepaalde volgorde, vaak chronologisch. In tegenstelling tot ItemList, ligt de nadruk van CreativeWorkSeries op gepubliceerd materiaal (bijvoorbeeld boeken en periodieken, of media zoals tv, radio en games)."@nl .

schema:Episode a rdfs:Class ;
    rdfs:label "Episode"@en,
        "Épisode"@fr,
        "Aflevering"@nl ;
    rdfs:isDefinedBy schema: ;
    rdfs:subClassOf schema:CreativeWork ;
    skos:definition "A media episode (e.g. TV, radio, video game) which can be part of a series or season."@en,
        "Un épisode médiatique (par exemple tv, radio, jeu vidéo) qui peut faire partie d'une série ou d'une saison."@fr,
        "Een media aflevering (bijvoorbeeld tv, radio, videogame) die deel uitmaakt van een serie of seizoen."@nl .

schema:Event a rdfs:Class ;
    rdfs:label "Event"@en,
        "Événement"@fr,
        "Gebeurtenis"@nl ;
    rdfs:isDefinedBy schema: ;
    rdfs:subClassOf schema:Thing ;
    skos:definition "An event happening at a certain time and location, such as a concert, lecture, or festival."@en,
        "Un événement qui se déroule à un moment et dans un lieu donnés, comme un concert, une conférence ou un festival."@fr,
        "Een gebeurtenis die plaatsvindt op een gegeven moment en locatie, zoals een concert, een lezing of een festival."@nl .

schema:Organization a rdfs:Class ;
    rdfs:label "Organisation"@en,
        "Organisation"@fr,
        "Organisatie"@nl ;
    rdfs:isDefinedBy schema: ;
    rdfs:subClassOf schema:Thing ;
    skos:definition "An organization such as a school, NGO, corporation, club, etc."@en,
        "Une organisation telle que une école, une ONG, une société, un club, etc."@fr,
        "Een organisatie zoals een school, NGO, corporatie, club, enz."@nl .

schema:PerformanceRole a rdfs:Class ;
    rdfs:label "Performance role"@en,
        "Rôle de performance"@fr,
        "Uitvoeringsrol"@nl ;
    rdfs:isDefinedBy schema: ;
    rdfs:subClassOf schema:Role ;
    skos:definition "A PerformanceRole is a Role that some entity places with regard to a theatrical performance, e.g. in a Movie, TVSeries etc."@en,
        "Un PerformanceRole est un rôle qu'une entité remplit dans le cadre d'une représentation théâtrale, par exemple dans un film, une série télévisée etc."@fr,
        "Een PerformanceRole is een rol die een entiteit vertolkt met betrekking tot een theatrale uitvoering, bijvoorbeeld in een film, televisieserie etc."@nl .

schema:Person a rdfs:Class ;
    rdfs:label "Person"@en,
        "Personne"@fr,
        "Persoon"@nl ;
    rdfs:isDefinedBy schema: ;
    rdfs:subClassOf schema:Thing ;
    owl:equivalentClass <http://xmlns.com/foaf/0.1/Person> ;
    skos:definition "A person (alive, dead, undead, or fictional)."@en,
        "Une personne (vivante, morte, non-morte ou fictive)."@fr,
        "Een persoon (levend, dood, ondood, of fictief)."@nl .

schema:Place a rdfs:Class ;
    rdfs:label "Place"@en,
        "Lieu"@fr,
        "Plaats"@nl ;
    rdfs:isDefinedBy schema: ;
    rdfs:subClassOf schema:Thing ;
    skos:definition "Entities that have a somewhat fixed, physical extension."@en,
        "Entités qui ont une extension physique quelque peu fixée."@fr,
        "Entiteiten die een enigszins vastliggende, fysieke uitbreiding hebben."@nl .

schema:PostalAddress a rdfs:Class ;
    rdfs:label "Postal address"@en,
        "Adresse postale"@fr,
        "Postadres"@nl ;
    rdfs:isDefinedBy schema: ;
    rdfs:subClassOf schema:ContactPoint ;
    skos:definition "The mailing address."@en,
        "L'adresse postale."@fr,
        "Het postadres."@nl .

schema:QuantitativeValue a rdfs:Class ;
    rdfs:label "Quantitative Value"@en,
        "Valeur quantitative"@fr,
        "Kwantitatieve waarde"@nl ;
    rdfs:isDefinedBy schema: ;
    rdfs:subClassOf schema:Thing ;
    skos:definition "A point value or interval for product characteristics and other purposes."@en,
        "Une valeur ponctuelle ou un intervalle pour les caractéristiques d'un produit et d'autres fins."@fr,
        "Een puntwaarde of interval voor producteigenschappen en andere doeleinden."@nl .

schema:Role a rdfs:Class ;
    rdfs:label "Role"@en,
        "Rôle"@fr,
        "Rol"@nl ;
    rdfs:isDefinedBy schema: ;
    rdfs:subClassOf schema:Thing ;
    skos:definition """Represents additional information about a relationship or property.
        For example a Role can be used to say that a 'member' role linking some SportsTeam to a player occurred during a particular time period.
        Or that a Person's 'actor' role in a Movie was for some particular characterName.
        Such properties can be attached to a Role entity, which is then associated with the main entities using ordinary properties like 'member' or 'actor'.
        """@en,
        """Représente des informations supplémentaires sur une relation ou une propriété.
        Par exemple, un rôle peut être utilisé pour indiquer que une rôle 'membre' (member role) qui lie une équipe sportive à un joueur, a eu lieu durant une période particulière.
        Ou que le rôle d''acteur' (actor role) d'une personne dans un film correspond à un nom de personnage particulier.
        Ces propriétés peuvent être attachées à un rôle d'entité (entity role), qui est ensuite associée aux entités principales en utilisant des propriétés ordinaires comme 'membre' (member) ou 'acteur' (actor).
        """@fr,
        """Stelt bijkomende informatie voor over een relatie of eigenschap.
        Bijvoorbeeld: een rol kan worden gebruikt om aan te geven dat een 'lid'rol (member role) die een sportteam aan een speler verbond, tijdens een bepaalde periode voorviel.
        Of dat een persoons 'acteur'rol (actor role) in een film voor een bepaalde karakternaam was.
        Deze eigenschappen kunnen worden toegevoegd aan een rolentiteit, die dan geassocieerd wordt met de hoofdentiteiten via normale eigenschappen zoals 'lid' (member) of 'acteur' (actor).
        """@nl .

schema:Thing a rdfs:Class ;
    rdfs:label "Thing"@en,
        "Chose"@fr,
        "Ding"@nl ;
    rdfs:isDefinedBy schema: ;
    skos:definition "The most generic type of item."@en,
        "Le type d'élément le plus générique."@fr,
        "Het meest generieke type item."@nl .

<http://id.loc.gov/vocabulary/preservation/relationshipSubType/doc> a owl:ObjectProperty ;
    rdfs:label "documents"@en,
        "généralise"@fr,
        "documenteert"@nl ;
    rdfs:isDefinedBy <http://id.loc.gov/vocabulary/preservation/relationshipSubType> ;
    rdfs:subPropertyOf premis:relationship ;
    skos:definition "A relationship between information about an environment object and the environment object itself. For instance, a user manual has a “documents” relationship to the Open Office software application. Has a reciprocal relationship of isDocumentedIn."@en,
        "Une relation entre les informations sur un objet d'environnement et l'objet d'environnement lui-même. Par exemple, un manuel d'utilisation a une relation 'documents' avec l'application logicielle Open Office. A une relation réciproque avec isDocumentedIn."@fr,
        "Een relatie tussen informatie over een omgevingsobject en het omgevingsobject zelf. Bijvoorbeeld, een gebruikershandleiding heeft een 'documents'-relatie met de Open Office-softwareapplicatie. Heeft een wederkerige relatie met isDocumentedIn."@nl .

<http://id.loc.gov/vocabulary/preservation/relationshipSubType/gen> a owl:ObjectProperty ;
    rdfs:label "generalizes"@en,
        "généralise"@fr,
        "veralgemeent"@nl ;
    rdfs:isDefinedBy <http://id.loc.gov/vocabulary/preservation/relationshipSubType> ;
    rdfs:subPropertyOf premis:relationship ;
    skos:definition "A relationship between an environment object and another where the described object is a more general description than the more specific related environment. Has a reciprocal relationship of specializes."@en,
        "Une Relation entre un objet d'environnement et un autre objet où l'objet décrit a une description plus générale que l'environnement lié plus spécifique. A une relation réciproque avec specializes."@fr,
        "Een relatie tussen een omgevingsobject en een ander object, waarbij het beschreven object een algemenere beschrijving is dan de meer specifieke verwante omgeving. Heeft een wederkerige relatie met specializes."@nl .

<http://id.loc.gov/vocabulary/preservation/relationshipSubType/hsp> a owl:ObjectProperty ;
    rdfs:label "has Part"@en,
        "a partie"@fr,
        "heeft onderdeel"@nl ;
    rdfs:isDefinedBy <http://id.loc.gov/vocabulary/preservation/relationshipSubType> ;
    rdfs:subPropertyOf premis:relationship ;
    skos:definition "The object contains the related object when these are the same object category. For instance, a larger Intellectual Entity has another Intellectual Entity as a part, or a compound file (e.g. archive.tar) contains another file (e.g. text.xml). Has the reciprocal relationship of isPartOf."@en,
        "L'objet contient l'objet lié lorsqu'il s'agit de la même catégorie d'objet. Par exemple, une entité intellectuelle plus grande a une autre entité intellectuelle comme partie, ou un fichier composé (par exemple archive.tar) contient un autre fichier (par exemple text.xml). A une relation réciproque avec isPartOf."@fr,
        "Het object bevat het gerelateerde object wanneer ze tot dezelfde objectcategorie behoren. Bv. een grotere intellectuele entiteit bevat een andere intellectuele entiteit, of een samengesteld bestand (bv. archive.tar) bevat een ander bestand (bv. text.xml). Heeft een wederkerige relatie met isPartOf."@nl .

<http://id.loc.gov/vocabulary/preservation/relationshipSubType/hsr> a owl:ObjectProperty ;
    rdfs:label "has Root"@en,
        "est à la base de"@fr,
        "ligt aan de basis van"@nl ;
    rdfs:isDefinedBy <http://id.loc.gov/vocabulary/preservation/relationshipSubType> ;
    rdfs:subPropertyOf premis:relationship ;
    skos:definition "For a representation only, the related object is the file that must be processed first in order to render the representation. It implies that a compound object (i.e. one made up of multiple files) requires that one file be picked up first as its root to render it."@en,
        "Uniquement pour une représentation (representation), l'objet lié est le fichier (file) qui doit être traité en premier afin de rendre la représentation comme il faut. Cela implique qu'un objet composé (c'est-à-dire composé de plusieurs fichiers (files)) nécessite qu'un fichier (file) soit pris en premier comme racine/base pour le rendre."@fr,
        "Alleen voor een representatie (representation) is het gerelateerde object het bestand (file) dat als eerste moet worden verwerkt om de representatie (representation) te kunnen renderen. Dit impliceert dat een samengesteld object (d.w.z. een object dat uit meerdere bestanden (file) bestaat) vereist dat één bestand (file) als eerste als root/basis wordt verwerkt om het te renderen."@nl .

<http://id.loc.gov/vocabulary/preservation/relationshipSubType/hss> a owl:ObjectProperty ;
    rdfs:label "has Source"@en,
        "a une source"@fr,
        "heeft een bron"@nl ;
    rdfs:isDefinedBy <http://id.loc.gov/vocabulary/preservation/relationshipSubType> ;
    rdfs:subPropertyOf premis:relationship ;
    skos:definition "A relationship in which the object is derived from the related object as a result of a transformation. For instance, an HTML file that is the product of a migration from a file encoded in the WordStar format has that Wordstar file as its source. Also applies to the relationship between the original and a disk image. Has a reciprocal relationship of isSourceOf."@en,
        "Une relation dans laquelle l'objet est dérivé de l'objet lié à la suite d'une transformation. Par exemple, un fichier HTML qui est le produit d'une migration à partir d'un fichier codé au format WordStar a ce fichier Wordstar comme source. S'applique également à la relation entre l'original et une image disque. A une relation réciproque avec isSourceOf."@fr,
        "Een relatie waarbij het object is afgeleid van het verwante object als resultaat van een transformatie. Bijvoorbeeld, een HTML-bestand dat het product is van een migratie van een bestand dat gecodeerd is in het WordStar-formaat, heeft dat Wordstar-bestand als zijn bron. Geldt ook voor de relatie tussen het origineel en een schijfbestand. Heeft een wederkerige relatie met isSourceOf."@nl .

<http://id.loc.gov/vocabulary/preservation/relationshipSubType/idc> a owl:ObjectProperty ;
    rdfs:label "is Documented In"@en,
        "est documenté dans"@fr,
        "is gedocumenteerd in"@nl ;
    rdfs:isDefinedBy <http://id.loc.gov/vocabulary/preservation/relationshipSubType> ;
    rdfs:subPropertyOf premis:relationship ;
    skos:definition "A relationship between an environment object and the information that documents it. Has a reciprocal relationship with documents."@en,
        "Une relation entre un objet d'environnement et les informations qui le documentent. A une relation réciproque avec documents."@fr,
        "Een relatie tussen een omgevingsobject en de informatie die het documenteert. Heeft een wederkerige relatie met documents."@nl .

<http://id.loc.gov/vocabulary/preservation/relationshipSubType/inc> a owl:ObjectProperty ;
    rdfs:label "includes"@en,
        "inclut"@fr,
        "bevat"@nl ;
    rdfs:isDefinedBy <http://id.loc.gov/vocabulary/preservation/relationshipSubType> ;
    rdfs:subPropertyOf premis:relationship ;
    skos:definition "A relationship in which the described object includes the referenced object, when objects have different object categories. For instance, a representation includes files. Has a reciprocal relationship of isIncludedIn."@en,
        "Une relation dans laquelle l'objet décrit inclut l'objet référencé, lorsque les objets ont des catégories d'objets différentes. Par exemple, une représentation (representation) inclut des fichiers (files). A une relation réciproque avec isIncludedIn."@fr,
        "Een relatie waarbij het beschreven object het object bevat waarnaar wordt verwezen, wanneer objecten verschillende objectcategorieën hebben. Bijvoorbeeld, een representatie (representation) bevat bestanden (files). Heeft een wederkerige relatie met isIncludedIn."@nl .

<http://id.loc.gov/vocabulary/preservation/relationshipSubType/irq> a owl:ObjectProperty ;
    rdfs:label "is Required by"@en,
        "est requis par"@fr,
        "wordt vereist door"@nl ;
    rdfs:isDefinedBy <http://id.loc.gov/vocabulary/preservation/relationshipSubType> ;
    rdfs:subPropertyOf premis:relationship ;
    skos:definition "The relationship of an environment object to a file or representation, where the environment is required by the other objects to render or run. Has a reciprocal relationship of requires."@en,
        "La relation entre un objet d'environnement et un fichier (file) ou une représentation (representation), lorsque l'environnement est requis par les autres objets pour le rendu ou l'exécution. A une relation réciproque avec requires."@fr,
        "De relatie van een omgevingsobject tot een bestand (file) of representatie (representation), waarbij de omgeving door de andere objecten vereist wordt om te renderen of uit te voeren. Heeft een wederkerige relatie met requires."@nl .

<http://id.loc.gov/vocabulary/preservation/relationshipSubType/isi> a owl:ObjectProperty ;
    rdfs:label "is Included in"@en,
        "est inclus dans"@fr,
        "is inbegrepen in"@nl ;
    rdfs:isDefinedBy <http://id.loc.gov/vocabulary/preservation/relationshipSubType> ;
    rdfs:subPropertyOf premis:relationship ;
    skos:definition "A relationship in which the described object is included in the referenced object, when the objects have different object categories, for instance, a bitstream to a file, a file to a representation. Has a reciprocal relationship of includes."@en,
        "Une relation dans laquelle l'objet décrit est inclus dans l'objet référencé, lorsque les objets ont des catégories d'objets différentes, par exemple, un flux binaire (bitstream) dans un fichier (file), un fichier (file) dans une représentation (representation). A une relation réciproque avec includes."@fr,
        "Een relatie waarbij het beschreven object is inbegrepen in het object waarnaar wordt verwezen, wanneer de objecten verschillende objectcategorieën hebben, bijvoorbeeld een bitstream in een bestand (file), een bestand (file) in een representatie (representation). Heeft een wederkerige relatie met includes."@nl .

<http://id.loc.gov/vocabulary/preservation/relationshipSubType/iso> a owl:ObjectProperty ;
    rdfs:label "is Source of"@en,
        "est à la source de"@fr,
        "ligt aan de bron van"@nl ;
    rdfs:isDefinedBy <http://id.loc.gov/vocabulary/preservation/relationshipSubType> ;
    rdfs:subPropertyOf premis:relationship ;
    skos:definition "The related object is a version of the source object created by a transformation. For example, an HTML file that is the product of a migration from a file encoded in the WordStar format, the Wordstar file has a “isSourceOf” relationship to the HTML file. Also applies to the relationship between the original and a disk image. Has a reciprocal relationship of hasSource."@en,
        "L'objet lié est une version de l'objet source créée par une transformation. Par exemple, un fichier HTML qui est le produit d'une migration à partir d'un fichier codé au format WordStar, le fichier Wordstar a une relation 'isSourceOf' avec le fichier HTML. S'applique également à la relation entre l'original et une image disque. A une relation réciproque avec hasSource."@fr,
        "Het gerelateerde object is een versie van het bronobject gemaakt door een transformatie. Bijvoorbeeld, een HTML-bestand dat het product is van een migratie van een bestand dat is gecodeerd in het WordStar-formaat, het Wordstar-bestand heeft een 'isSourceOf'-relatie met het HTML-bestand. Geldt ook voor de relatie tussen het origineel en een schijfbestand. Heeft een wederkerige relatie met hasSource."@nl .

<http://id.loc.gov/vocabulary/preservation/relationshipSubType/isp> a owl:ObjectProperty ;
    rdfs:label "is Part Of"@en,
        "fait partie de"@fr,
        "maakt onderdeel uit van"@nl ;
    rdfs:isDefinedBy <http://id.loc.gov/vocabulary/preservation/relationshipSubType> ;
    rdfs:subPropertyOf premis:relationship ;
    skos:definition "A relationship in which the object is contained in the related object when these are the same object category. For instance a Web page intellectual entity is part of a larger Web site intellectual entity. Has a reciprocal relationship of hasPart."@en,
        "Une relation dans laquelle l'objet est contenu dans l'objet lié lorsque ceux-ci sont de la même catégorie d'objet. Par exemple, une entité intellectuelle de site Web fait partie d'une entité intellectuelle de site Web plus grande. A une relation réciproque avec hasPart."@fr,
        "Een relatie waarbij het object deel uitmaakt van het gerelateerde object wanneer ze behoren tot dezelfde objectcategorie. Bv. een webpagina intellectuele entiteit maakt onderdeel uit van een grotere webpagina intellectuele entiteit. Heeft een wederkerige relatie met hasPart."@nl .

<http://id.loc.gov/vocabulary/preservation/relationshipSubType/iss> a owl:ObjectProperty ;
    rdfs:label "is Superseded by"@en,
        "a été remplacé par"@fr,
        "werd vervangen door"@nl ;
    rdfs:isDefinedBy <http://id.loc.gov/vocabulary/preservation/relationshipSubType> ;
    rdfs:subPropertyOf premis:relationship ;
    skos:definition "A relationship between an environment object and another where the described object has been replaced by another. This allows for an audit trail of environments to be maintained. Has a reciprocal relationship of supersedes."@en,
        "Une relation entre un objet d'environnement et un autre objet où l'objet décrit a été remplacé par un autre. Cela permet de conserver une piste d'audit des environnements. A une relation réciproque avec supersedes."@fr,
        "Een relatie tussen een omgevingsobject en een ander object waarbij het beschreven object is vervangen door een ander. Hierdoor kan een controlespoor van omgevingen worden bijgehouden. Heeft een wederkerige relatie met supersedes."@nl .

<http://id.loc.gov/vocabulary/preservation/relationshipSubType/req> a owl:ObjectProperty ;
    rdfs:label "requires"@en,
        "nécessite"@fr,
        "vereist"@nl ;
    rdfs:isDefinedBy <http://id.loc.gov/vocabulary/preservation/relationshipSubType> ;
    rdfs:subPropertyOf premis:relationship ;
    skos:definition "The relationship of an object to another object, where it requires a particular environment or non-environment object to be rendered or to be run. For instance, a file of format Word 97, requires MS Word 1997 to render it. Has a reciprocal relationship of isRequiredBy."@en,
        "La relation d'un objet avec un autre objet, lorsqu'il nécessite un environnement particulier ou un objet non lié à l'environnement pour être rendu ou exécuté comme il faut. Par exemple, un fichier au format Word 97 nécessite MS Word 1997 pour être rendu. A une relation réciproque avec isRequiredBy."@fr,
        "De relatie van een object tot een ander object, waarbij het een bepaald omgevings- of niet-omgevingsobject nodig heeft om te worden weergegeven of om te worden uitgevoerd. Bijvoorbeeld, een bestand met de opmaak Word 97 vereist MS Word 1997 om het weer te geven. Heeft een wederkerige relatie met isRequiredBy."@nl .

<http://id.loc.gov/vocabulary/preservation/relationshipSubType/spe> a owl:ObjectProperty ;
    rdfs:label "specializes"@en,
        "spécialise"@fr,
        "specialiseert"@nl ;
    rdfs:isDefinedBy <http://id.loc.gov/vocabulary/preservation/relationshipSubType> ;
    rdfs:subPropertyOf premis:relationship ;
    skos:definition "A relationship between an environment object and another where the described object provides specific characteristics, while the related environment is more generic. Has a reciprocal relationship of generalizes."@en,
        "Une relation entre un objet d'environnement et un autre objet où l'objet décrit fournit des caractéristiques spécifiques, tandis que l'environnement lié est plus générique. A une relation réciproque avec generalizes."@fr,
        "Een relatie tussen een omgevingsobject en een ander object, waarbij het beschreven object specifieke kenmerken vertoont, terwijl de verwante omgeving meer generiek is. Heeft een wederkerige relatie met generalizes."@nl .

<http://id.loc.gov/vocabulary/preservation/relationshipSubType/sup> a owl:ObjectProperty ;
    rdfs:label "supersedes"@en,
        "remplace"@fr,
        "vervangt"@nl ;
    rdfs:isDefinedBy <http://id.loc.gov/vocabulary/preservation/relationshipSubType> ;
    rdfs:subPropertyOf premis:relationship ;
    skos:definition "A relationship between an environment object and another where the described object replaces another. This allows for an audit trail of environments to be maintained. Has a reciprocal relationship of isSupersededBy."@en,
        "Une relation entre un objet d'environnement et un autre objet où l'objet décrit en remplace un autre. Cela permet de conserver une piste d'audit des environnements. A une relation réciproque avec isSupersededBy."@fr,
        "Een relatie tussen een omgevingsobject en een ander object waarbij het beschreven object een ander object vervangt. Hierdoor kan een controlespoor van omgevingen worden bijgehouden. Heeft een wederkerige relatie met isSupersededBy."@nl .

dct:available a rdf:Property ;
    rdfs:label "date available"@en,
        "date de disponibilité"@fr,
        "beschikbaarheidsdatum"@nl ;
    rdfs:isDefinedBy dct: ;
    skos:definition "Date that the resource became or will become available."@en,
        "Date à laquelle la ressource devient ou deviendra disponible."@fr,
        "Datum waarop de bron beschikbaar is of zal zijn."@nl .

dct:format a rdf:Property ;
    rdfs:label "format"@en,
        "format"@fr,
        "formaat"@nl ;
    dct:description "Examples of dimensions include size and duration. Recommended best practice is to use a controlled vocabulary such as the list of Internet Media Types [MIME]."@en ;
    dct:hasVersion <http://dublincore.org/usage/terms/history/#formatT-001> ;
    dct:issued "2008-01-14"^^xsd:date ;
    dct:modified "2008-01-14"^^xsd:date ;
    rdfs:isDefinedBy dct: ;
    rdfs:range dct:MediaTypeOrExtent ;
    rdfs:subPropertyOf <http://purl.org/dc/elements/1.1/format> ;
    skos:definition "The file format, physical medium, or dimensions of the resource."@en,
        "Le format du fichier, le support physique ou les dimensions de la ressource."@fr,
        "Het bestandsformaat, fysiek medium of afmetingen van de bron."@nl .

<http://www.ebu.ch/metadata/ontologies/ebucore/ebucore#annotationConfidence> a rdf:Property ;
    rdfs:label "Annotation confidence"@en,
        "Fiabilité des annotations"@fr,
        "Annotatievertrouwen"@nl ;
    rdfs:domain <http://www.ebu.ch/metadata/ontologies/ebucore/ebucore#Annotation> ;
    rdfs:range xsd:string ;
    skos:definition "To estimate the confidence in an Annotation."@en,
        "Pour estimer la confiance dans une annotation."@fr,
        "Om het vertrouwen in een annotatie te schatten."@nl .

<http://www.ebu.ch/metadata/ontologies/ebucore/ebucore#annotationType> a rdf:Property ;
    rdfs:label "Annotation type"@en,
        "Type d'annotation"@fr,
        "Annotatietype"@nl ;
    rdfs:domain <http://www.ebu.ch/metadata/ontologies/ebucore/ebucore#Annotation> ;
    rdfs:range <http://www.ebu.ch/metadata/ontologies/ebucore/ebucore#Annotation_Type>,
        xsd:anyURI,
        xsd:string ;
    skos:definition "Range: string, anyURI or Concept."@en,
        "To define a type of Annotation."@en,
        "Pour définir un type d'annotation."@fr,
        "Om een type annotatie te definiëren."@nl .

<http://www.ebu.ch/metadata/ontologies/ebucore/ebucore#hasAnnotationRelatedArtefact> a rdf:Property ;
    rdfs:label "Annotation related artefact"@en,
        "Artefact lié à l'Annotation"@fr,
        "Artefact verbonden aan de Annotatie"@nl ;
    rdfs:domain <http://www.ebu.ch/metadata/ontologies/ebucore/ebucore#Annotation> ;
    rdfs:range xsd:anyURI,
        xsd:string ;
    rdfs:subPropertyOf <http://www.ebu.ch/metadata/ontologies/ebucore/ebucore#hasAnnotationPurpose> ;
    skos:definition "To identify an Artefact subject of the Annotation."@en,
        "Pour identifier un objet d'artefact de l'annotation."@fr,
        "Om een artefactonderwerp van de annotatie te identificeren."@nl .

<http://www.ebu.ch/metadata/ontologies/ebucore/ebucore#hasAnnotationTarget> a rdf:Property ;
    rdfs:label "Annotation target"@en,
        "Cible d'annotation"@fr,
        "Annotatiedoel"@nl ;
    rdfs:domain <http://www.ebu.ch/metadata/ontologies/ebucore/ebucore#Annotation> ;
    rdfs:range xsd:anyURI ;
    skos:definition "To define the target object to which the Annotation applies."@en,
        "Pour définir l'objet cible auquel s'applique l'annotation."@fr,
        "Om het doelobject te definiëren waarop de annotatie van toepassing is."@nl .

<http://www.ebu.ch/metadata/ontologies/ebucore/ebucore#hasCaptioning> a rdf:Property ;
    rdfs:label "captioning"@en,
        "sous-titrage"@fr,
        "ondertiteling"@nl ;
    rdfs:domain <http://www.ebu.ch/metadata/ontologies/ebucore/ebucore#Asset> ;
    rdfs:isDefinedBy <http://www.ebu.ch/metadata/ontologies/ebucore/ebucore#> ;
    rdfs:range <http://www.ebu.ch/metadata/ontologies/ebucore/ebucore#Captioning> ;
    skos:definition "To signal the presence of Captioning."@en,
        "Pour signaler la présence du sous-titrage."@fr,
        "Om de aanwezigheid van ondertiteling aan te duiden."@nl .

<http://www.ebu.ch/metadata/ontologies/ebucore/ebucore#hasCastMember> a rdf:Property ;
    rdfs:label "Cast member"@en,
        "Membre de la distribution"@fr,
        "Cast lid"@nl ;
    rdfs:comment "A member of the cast."@en,
        "Range: a string or a Cast"@en,
        "A member of the cast."@fr,
        "Een lid van de cast."@nl ;
    rdfs:domain <http://www.ebu.ch/metadata/ontologies/ebucore/ebucore#Asset> ;
    rdfs:range <http://www.ebu.ch/metadata/ontologies/ebucore/ebucore#Cast>,
        xsd:string .

<http://www.ebu.ch/metadata/ontologies/ebucore/ebucore#hasMediaFragment> a rdf:Property ;
    rdfs:label "fragment"@en,
        "a un fragment (de média)"@fr,
        "heeft (media)fragment"@nl ;
    rdfs:domain <http://www.ebu.ch/metadata/ontologies/ebucore/ebucore#MediaResource> ;
    rdfs:isDefinedBy <http://www.ebu.ch/metadata/ontologies/ebucore/ebucore#> ;
    rdfs:range <http://www.ebu.ch/metadata/ontologies/ebucore/ebucore#MediaFragment> ;
    owl:equivalentProperty <http://www.w3.org/ns/ma-ont#hasFragment> ;
    owl:inverseOf <http://www.ebu.ch/metadata/ontologies/ebucore/ebucore#isMediaFragmentOf> ;
    skos:definition "To define relation to MediaFragments within a MediaResource."@en,
        "Pour définir une relation entre des MediaFragments dans une MediaResource."@fr,
        "Om een relatie te definiëren tussen MediaFragments binnenin een MediaResource."@nl .

<http://www.ebu.ch/metadata/ontologies/ebucore/ebucore#hasMimeType> a rdf:Property ;
    rdfs:label "mime type"@en,
        "mime type"@fr,
        "mime type"@nl ;
    rdfs:domain <http://www.ebu.ch/metadata/ontologies/ebucore/ebucore#MediaResource> ;
    rdfs:isDefinedBy <http://www.ebu.ch/metadata/ontologies/ebucore/ebucore#> ;
    rdfs:range <http://www.ebu.ch/metadata/ontologies/ebucore/ebucore#MimeType>,
        xsd:string ;
    rdfs:subPropertyOf <http://www.ebu.ch/metadata/ontologies/ebucore/ebucore#hasFormat> ;
    skos:definition "To specify the Mime type of a Resource."@en,
        "Pour spécifier le type MIME d'une ressource."@fr,
        "Om het MIME type van een resource te specificeren."@nl .

<http://www.ebu.ch/metadata/ontologies/ebucore/ebucore#hasObjectType> a rdf:Property ;
    rdfs:label "object/asset type"@en,
        "type d'objet/de bien"@fr,
        "type object/activum"@nl ;
    rdfs:domain <http://www.ebu.ch/metadata/ontologies/ebucore/ebucore#EditorialObject> ;
    rdfs:isDefinedBy <http://www.ebu.ch/metadata/ontologies/ebucore/ebucore#> ;
    rdfs:range <http://www.ebu.ch/metadata/ontologies/ebucore/ebucore#ObjectType>,
        xsd:anyURI,
        xsd:string ;
    skos:definition "To define an ObjectType for the BusinessObject (e.g. book, report, programme, clip) if not defined as a subClass of BusinessObject."@en,
        "Pour définir un ObjectType pour un BusinessObject (par exemple un livre, rapport, programme, clip) s'il n'est pas défini comme une sous-classe de BusinessObject."@fr,
        "Om een ObjectType te definiëren voor een BusinessObject (bv. boek, rapport, programma, clip) indien dit niet gedefinieerd is als een subklasse van BusinessObject."@nl .

<http://www.ebu.ch/metadata/ontologies/ebucore/ebucore#isAnnotatedMediaResource> a rdf:Property ;
    rdfs:label "Media resource"@en,
        "Media resource"@fr,
        "Media resource"@nl ;
    rdfs:domain <http://www.ebu.ch/metadata/ontologies/ebucore/ebucore#Annotation> ;
    rdfs:range <http://www.ebu.ch/metadata/ontologies/ebucore/ebucore#MediaResource> ;
    skos:definition "To link an Annotation to a MediaResource."@en,
        "Pour lier une annotation à un MediaResource."@fr,
        "Om een annotatie te koppelen aan een mediaresource."@nl .

<http://www.ebu.ch/metadata/ontologies/ebucore/ebucore#synopsis> a rdf:Property ;
    rdfs:label "Synopsis"@en,
        "synopsis"@fr,
        "Korte inhoud"@nl ;
    rdfs:comment "To provide a summary."@en,
        "To provide a summary."@fr,
        "Om een samenvatting te geven."@nl ;
    rdfs:domain <http://www.ebu.ch/metadata/ontologies/ebucore/ebucore#Asset> ;
    rdfs:range xsd:string ;
    rdfs:subPropertyOf <http://www.ebu.ch/metadata/ontologies/ebucore/ebucore#description> .

<http://www.europeana.eu/schemas/edm/isNextInSequence> a owl:ObjectProperty ;
    rdfs:label "is next in sequence of"@en,
        "est le prochain dans la séquence de"@fr,
        "is de volgende in de reeks van"@nl ;
    rdfs:isDefinedBy <http://www.europeana.eu/schemas/edm/> ;
    rdfs:subPropertyOf <http://purl.org/dc/elements/1.1/relation> ;
    skos:definition "edm:isNextInSequence relates two resources S and R that are ordered parts of the same resource A, and such that S comes immediately after R in the order created by their being parts of A."@en,
        "edm:isNextInSequence met en relation deux ressources S et R qui sont des parties ordonnées de la même ressource A, et telles que S vient immédiatement après R dans l'ordre créé par leur appartenance à A."@fr,
        "edm:isNextInSequence relateert twee resources S en R die geordende onderdelen zijn van dezelfde resource A, en wel zodanig dat S onmiddellijk na R komt in de volgorde die ontstaat doordat zij onderdelen zijn van A."@nl .

premis:endDate a owl:DatatypeProperty ;
    rdfs:label "end date"@en,
        "date de fin"@fr,
        "einddatum"@nl ;
    rdfs:domain _:na87fcceb263b4ca493cedf23101c1dd8b1 ;
    rdfs:isDefinedBy premis: ;
    rdfs:subPropertyOf dct:date .

premis:fixity a owl:ObjectProperty ;
    rdfs:label "has fixity"@en,
        "a fixity"@fr,
        "heeft fixity"@nl ;
    rdfs:domain [ a owl:Class ;
            owl:unionOf ( premis:Bitstream premis:File ) ] ;
    rdfs:isDefinedBy premis: ;
    rdfs:range premis:Fixity .

premis:medium a owl:ObjectProperty ;
    rdfs:label "has medium"@en,
        "a un support"@fr,
        "heeft als medium"@nl ;
    rdfs:domain premis:StorageLocation ;
    rdfs:isDefinedBy premis: ;
    rdfs:range premis:StorageMedium .

premis:originalName a owl:DatatypeProperty ;
    rdfs:label "has original name"@en,
        "porte le nom d'origine"@fr,
        "heeft originele naam"@nl ;
    rdfs:domain [ a owl:Class ;
            owl:unionOf ( premis:File premis:IntellectualEntity premis:Representation ) ] ;
    rdfs:isDefinedBy premis: ;
    rdfs:range rdfs:Literal .

premis:size a owl:DatatypeProperty ;
    rdfs:label "has size"@en,
        "a une taille (du fichier)"@fr,
        "heeft (bestands)grootte"@nl ;
    rdfs:domain [ a owl:Class ;
            owl:unionOf ( premis:Bitstream premis:File ) ] ;
    rdfs:isDefinedBy premis: ;
    rdfs:range xsd:nonNegativeInteger ;
    skos:narrowMatch <http://www.ebu.ch/metadata/ontologies/ebucore/ebucore#fileSize> .

premis:startDate a owl:DatatypeProperty ;
    rdfs:label "start date"@en,
        "date de début"@fr,
        "startdatum"@nl ;
    rdfs:domain _:na87fcceb263b4ca493cedf23101c1dd8b17 ;
    rdfs:isDefinedBy premis: ;
    rdfs:subPropertyOf dct:date .

premis:storedAt a owl:ObjectProperty ;
    rdfs:label "stored at"@en,
        "stocké à"@fr,
        "opgeslagen te"@nl ;
    rdfs:domain [ a owl:Class ;
            owl:unionOf ( premis:Bitstream premis:File premis:Representation ) ] ;
    rdfs:isDefinedBy premis: ;
    rdfs:range premis:StorageLocation .

<http://www.ontologydesignpatterns.org/cp/owl/sequence.owl#directlyFollows> a owl:ObjectProperty ;
    rdfs:label "directly follows"@en,
        "suit directement"@fr,
        "volgt direct op"@nl ;
    rdfs:domain owl:Thing ;
    rdfs:isDefinedBy <http://www.ontologydesignpatterns.org/cp/owl/sequence.owl> ;
    rdfs:range owl:Thing ;
    rdfs:subPropertyOf <http://www.ontologydesignpatterns.org/cp/owl/sequence.owl#follows> ;
    owl:inverseOf <http://www.ontologydesignpatterns.org/cp/owl/sequence.owl#directlyPrecedes> ;
    skos:definition "The intransitive follows relation. For example, Thursday directly follows Wednesday. Directness of precedence depends on the designer conceptualization."@en,
        "La relation intransitive de 'suivre directement'. Par exemple, jeudi suit directement mercredi. Le caractère direct de la précédence dépend de la conceptualisation du concepteur."@fr,
        "De intransitieve 'volgt-direct-op' relatie. Bv. donderdag volgt direct op woensdag. De mate van 'directheid' bij het 'volgen-op' hangt af van het ontwerp van de bedenker."@nl .

rdf:value a rdf:Property ;
    rdfs:label "value"@en,
        "valeur"@fr,
        "waarde"@nl ;
    rdfs:domain rdfs:Resource ;
    rdfs:isDefinedBy rdf: ;
    rdfs:range xsd:string ;
    skos:definition "May be used in describing structured values."@en,
        "Peut être utilisé pour décrire des valeurs structurées."@fr,
        "Kan worden gebruikt om gestructureerde waardes te beschrijven."@nl .

skos:changeNote a rdf:Property,
        owl:AnnotationProperty ;
    rdfs:label "change note"@en,
        "note de changement"@fr,
        "wijzigingsnotitie"@nl ;
    rdfs:isDefinedBy <http://www.w3.org/2004/02/skos/core> ;
    rdfs:subPropertyOf skos:note ;
    skos:definition "A note about a modification to a concept."@en,
        "Une note à propos d'une modification d'un concept."@fr,
        "Een notitie over een wijziging aan een concept."@nl .

skos:definition a rdf:Property,
        owl:AnnotationProperty ;
    rdfs:label "definition"@en,
        "définition"@fr,
        "definitie"@nl ;
    rdfs:isDefinedBy <http://www.w3.org/2004/02/skos/core> ;
    rdfs:subPropertyOf skos:note ;
    skos:definition "A statement or formal explanation of the meaning of a concept."@en,
        "Une déclaration ou une explication formelle du sens d'un concept."@fr,
        "Een verklaring of formele uitleg van de betekenis van een concept."@nl .

skos:editorialNote a rdf:Property,
        owl:AnnotationProperty ;
    rdfs:label "editorial note"@en,
        "note éditoriale"@fr,
        "redactionele notitie"@nl ;
    rdfs:isDefinedBy <http://www.w3.org/2004/02/skos/core> ;
    rdfs:subPropertyOf skos:note ;
    skos:definition "A note for an editor, translator or maintainer of the vocabulary."@en,
        "Une note pour un éditeur, traducteur ou responsable de la terminologie."@fr,
        "Een notitie voor een redacteur, vertaler of beheerder van het vocabularium."@nl .

skos:exactMatch a rdf:Property,
        owl:ObjectProperty,
        owl:SymmetricProperty,
        owl:TransitiveProperty ;
    rdfs:label "has exact match"@en,
        "a une correspondance exacte"@fr,
        "heeft exacte overeenkomst"@nl ;
    rdfs:comment "skos:exactMatch is disjoint with each of the properties skos:broadMatch and skos:relatedMatch."@en,
        "skos:exactMatch est disjoints avec chacune des propriétés skos:broadMatch et skos:relatedMatch."@fr,
        "skos:exactMatch is disjunct met elk van de eigenschappen skos:broadMatch en skos:relatedMatch."@nl ;
    rdfs:isDefinedBy <http://www.w3.org/2004/02/skos/core> ;
    rdfs:subPropertyOf skos:closeMatch ;
    skos:definition "`skos:exactMatch` is used to link two concepts, indicating a high degree of confidence that the concepts can be used interchangeably across a wide range of information retrieval applications. `skos:exactMatch` is a transitive property, and is a sub-property of `skos:closeMatch`."@en,
        "`skos:exactMatch` est utilisé pour lier deux concepts, indiquant un haut degré de confiance que les concepts peuvent être utilisés de manière interchangeable dans un large éventail d'applications de recherche d'information. `skos:exactMatch` est une propriété transitive, et est une sous-propriété de `skos:closeMatch`."@fr,
        "`skos:exactMatch` wordt gebruikt om twee concepten te verbinden, waarbij een hoge mate van vertrouwen wordt uitgedrukt dat de concepten uitwisselbaar in een brede waaier van informatiezoektoepassingen kunnen worden gebruikt. `skos:exactMatch` is een transitieve eigenschap en is een sub-eigenschap van `skos:closeMatch`."@nl .

skos:example a rdf:Property,
        owl:AnnotationProperty ;
    rdfs:label "example"@en,
        "exemple"@fr,
        "voorbeeld"@nl ;
    rdfs:isDefinedBy <http://www.w3.org/2004/02/skos/core> ;
    rdfs:subPropertyOf skos:note ;
    skos:definition "An example of the use of a concept."@en,
        "Un exemple de l'utilisation d'un concept."@fr,
        "Een voorbeeld van het gebruik van een concept."@nl .

skos:historyNote a rdf:Property,
        owl:AnnotationProperty ;
    rdfs:label "history note"@en,
        "note historique"@fr,
        "historische notitie"@nl ;
    rdfs:isDefinedBy <http://www.w3.org/2004/02/skos/core> ;
    rdfs:subPropertyOf skos:note ;
    skos:definition "A note about the past state/use/meaning of a concept."@en,
        "Une note sur l'état/usage/sens passé d'un concept."@fr,
        "Een notitie over de vroegere staat/gebruik/betekenis van een concept."@nl .

skos:member a rdf:Property,
        owl:ObjectProperty ;
    rdfs:label "has member"@en,
        "a un membre"@fr,
        "heeft lid"@nl ;
    rdfs:domain skos:Collection ;
    rdfs:isDefinedBy <http://www.w3.org/2004/02/skos/core> ;
    rdfs:range _:n0eda34ab87e64af8be809e1d9077553ab1 ;
    skos:definition "Relates a collection to one of its members."@en,
        "Relie une collection à l'un de ses membres."@fr,
        "Verbindt een collectie met één van zijn leden."@nl .

skos:memberList a rdf:Property,
        owl:FunctionalProperty,
        owl:ObjectProperty ;
    rdfs:label "has member list"@en,
        "a une liste de membres"@fr,
        "heeft lijst van leden"@nl ;
    rdfs:comment """For any resource, every item in the list given as the value of the
      skos:memberList property is also a value of the skos:member property."""@en,
        """Pour toute ressource, chaque élément de la liste donnée comme valeur de la
        propriété skos:memberList est également une valeur de la propriété skos:member."""@fr,
        """Voor elke resource is elk item in de lijst die als waarde van de
        skos:memberList eigenschap wordt gegeven, ook een waarde van de skos:member eigenschap."""@nl ;
    rdfs:domain skos:OrderedCollection ;
    rdfs:isDefinedBy <http://www.w3.org/2004/02/skos/core> ;
    rdfs:range rdf:List ;
    skos:definition "Relates an ordered collection to the RDF list containing its members."@en,
        "Relie une collection ordonnée à la liste RDF contenant ses membres."@fr,
        "Verbindt een geordende collectie met de RDF lijst die zijn leden bevat."@nl .

skos:relatedMatch a rdf:Property,
        owl:ObjectProperty,
        owl:SymmetricProperty ;
    rdfs:label "has related match"@en,
        "a un match lié"@fr,
        "heeft gerelateerde match"@nl ;
    rdfs:isDefinedBy <http://www.w3.org/2004/02/skos/core> ;
    rdfs:subPropertyOf skos:mappingRelation,
        skos:related ;
    skos:definition "skos:relatedMatch is used to state an associative mapping link between two conceptual resources in different concept schemes."@en,
        "skos:relatedMatch est utilisé pour indiquer un lien de correspondance associative entre deux ressources conceptuelles dans des schémas de concepts différents."@fr,
        "skos:relatedMatch wordt gebruikt om een associatieve mapping link te geven tussen twee conceptuele resources in verschillende conceptenschema's."@nl .

skos:scopeNote a rdf:Property,
        owl:AnnotationProperty ;
    rdfs:label "scope note"@en,
        "note de portée"@fr,
        "scope notitie"@nl ;
    rdfs:isDefinedBy <http://www.w3.org/2004/02/skos/core> ;
    rdfs:subPropertyOf skos:note ;
    skos:definition "A note that helps to clarify the meaning and/or the use of a concept."@en,
        "Une note qui aide à clarifier le sens et/ou l'utilisation d'un concept."@fr,
        "Een notitie die helpt om de betekenis en/of het gebruik van een concept te verduidelijken."@nl .

<http://www.w3.org/2008/05/skos-xl#altLabel> a rdf:Property,
        owl:ObjectProperty ;
    rdfs:label "alternative label"@en,
        "étiquette alternative"@fr,
        "alternatief label"@nl ;
    rdfs:comment "If C skosxl:altLabel L and L skosxl:literalForm V, then X skos:altLabel V."@en ;
    rdfs:isDefinedBy <http://www.w3.org/2008/05/skos-xl> ;
    rdfs:range <http://www.w3.org/2008/05/skos-xl#Label> ;
    rdfs:seeAlso skos:altLabel ;
    skos:definition "The property skosxl:altLabel is used to associate an skosxl:Label with a skos:Concept. The property is analogous to skos:altLabel."@en,
        "La propriété skosxl:altLabel est utilisée pour associer une skosxl:Label avec un skos:Concept. La propriété est analogue à skos:altLabel."@fr,
        "De eigenschap skosxl:altLabel wordt gebruikt om een skosxl:Label te koppelen met een skos:Concept. De eigenschap is analoog aan skos:altLabel."@nl .

<http://www.w3.org/2008/05/skos-xl#hiddenLabel> a rdf:Property,
        owl:ObjectProperty ;
    rdfs:label "hidden label"@en,
        "étiquette cachée"@fr,
        "verborgen label"@nl ;
    rdfs:comment "If C skosxl:hiddenLabel L and L skosxl:literalForm V, then C skos:hiddenLabel V."@en ;
    rdfs:isDefinedBy <http://www.w3.org/2008/05/skos-xl> ;
    rdfs:range <http://www.w3.org/2008/05/skos-xl#Label> ;
    rdfs:seeAlso skos:hiddenLabel ;
    skos:definition "The property skosxl:hiddenLabel is used to associate an skosxl:Label with a skos:Concept. The property is analogous to skos:hiddenLabel."@en,
        "La propriété skosxl:hiddenLabel est utilisée pour associer une skosxl:Label avec un skos:Concept. La propriété est analogue à skos:hiddenLabel."@fr,
        "De eigenschap skosxl:hiddenLabel wordt gebruikt om een skosxl:Label te koppelen met een skos:Concept. De eigenschap is analoog aan skos:hiddenLabel."@nl .

<http://www.w3.org/2008/05/skos-xl#labelRelation> a rdf:Property,
        owl:ObjectProperty,
        owl:SymmetricProperty ;
    rdfs:label "label relation"@en,
        "relation de l'étiquette"@fr,
        "labelrelatie"@nl ;
    rdfs:domain <http://www.w3.org/2008/05/skos-xl#Label> ;
    rdfs:isDefinedBy <http://www.w3.org/2008/05/skos-xl> ;
    rdfs:range <http://www.w3.org/2008/05/skos-xl#Label> ;
    skos:definition "The property skosxl:labelRelation is used for representing binary ('direct') relations between instances of the class skosxl:Label."@en,
        "La propriété skosxl:labelRelation est utilisée pour représenter les relations binaires («directes») entre les instances de la classe skosxl:Label."@fr,
        "De eigenschap skosxl:labelRelation wordt gebruikt voor het weergeven van binaire ('directe') relaties tussen instanties van de klasse skosxl:Label."@nl ;
    skos:scopeNote "skosxl:labelRelation is not intended to be used directly, but rather as the basis for a design pattern which can be refined for more specific labeling scenarios."@en .

<http://www.w3.org/2008/05/skos-xl#prefLabel> a rdf:Property,
        owl:ObjectProperty ;
    rdfs:label "preferred label"@en,
        "étiquette préférée"@fr,
        "voorkeurslabel"@nl ;
    rdfs:comment "If C skosxl:prefLabel L and L skosxl:literalForm V, then X skos:prefLabel V."@en ;
    rdfs:isDefinedBy <http://www.w3.org/2008/05/skos-xl> ;
    rdfs:range <http://www.w3.org/2008/05/skos-xl#Label> ;
    rdfs:seeAlso skos:prefLabel ;
    skos:definition "The property skosxl:prefLabel is used to associate an skosxl:Label with a skos:Concept. The property is analogous to skos:prefLabel."@en,
        "La propriété skosxl:prefLabel est utilisée pour associer une skosxl:Label avec un skos:Concept. La propriété est analogue à skos:prefLabel."@fr,
        "De eigenschap skosxl:prefLabel wordt gebruikt om een skosxl:Label te koppelen met een skos:Concept. De eigenschap is analoog aan skos:prefLabel."@nl .

org:classification a rdf:Property,
        owl:ObjectProperty ;
    rdfs:label "classification"@en,
        "classification"@fr,
        "classificatie"@nl ;
    rdfs:domain org:Organization ;
    rdfs:isDefinedBy <http://www.w3.org/ns/org> ;
    rdfs:range skos:Concept ;
    skos:definition "Indicates a classification for this Organization within some classification scheme. Extension vocabularies may wish to specialize this property to have a range corresponding to a specific `skos:ConceptScheme`. This property is under discussion and may be revised or removed - in many cases organizations are best categorized by defining a sub-class hierarchy in an extension vocabulary."@en,
        "Indique une classification pour cette Organisation dans le cadre d'un schéma de classification. Il est possible de spécialiser cette propriété en utilisant un vocabulaire spécialisé pour que le champ corresponde à un concept spécifique `skos:ConceptScheme`. Cette propriété est en discussion est pourrait être révisée ou supprimée - dans de nombreux cas, les organisations sont mieux catégorisées par une hiérarchie de sous-classe dans un vocabulaire externe."@fr,
        "Duidt een classificatie van deze organisatie aan met een classificatieschema. Het is mogelijk om deze eigenschap verder te specificiëren met behulp van een gespecialiseerd vocabularium opdat het veld overeenkomt met een specifiek concept `skos:ConceptScheme`. In veel gevallen kunnen organisaties beter gecategoriseerd worden aan de hand van een hiërarchie met subklassen in een extern vocabularium."@nl .

org:hasPrimarySite a rdf:Property,
        owl:ObjectProperty ;
    rdfs:label "primary Site"@en,
        "site principal"@fr,
        "hoofdzetel"@nl ;
    rdfs:domain org:Organization ;
    rdfs:isDefinedBy <http://www.w3.org/ns/org> ;
    rdfs:range org:Site ;
    rdfs:subPropertyOf org:hasSite ;
    skos:definition "Indicates a primary site for the Organization, this is the default means by which an Organization can be contacted and is not necessarily the formal headquarters."@en,
        "Indique le site principal d'une Organisation, le moyen par défaut par lequel l'Organisation peut être contactée et pas nécessairement le siège social légal."@fr,
        "Duidt de hoofdzetel van een organisatie aan, dit is de standaard manier waarop de organisatie gecontacteerd kan worden en niet noodzakelijk de juridische zetel."@nl .

org:hasUnit a rdf:Property,
        owl:ObjectProperty ;
    rdfs:label "has Unit"@en,
        "possède une Unité"@fr,
        "heeft een eenheid"@nl ;
    rdfs:domain org:FormalOrganization ;
    rdfs:isDefinedBy <http://www.w3.org/ns/org> ;
    rdfs:range org:OrganizationalUnit ;
    rdfs:subPropertyOf org:hasSubOrganization ;
    skos:definition "Indicates a unit which is part of this Organization, e.g. a Department within a larger FormalOrganization. Inverse of `org:unitOf`."@en,
        "Indique une Unité qui fait partie d'une Organisation, par exemple un Départment au sein d'une Organisation Formelle plus large. Inverse de `org:unitOf`."@fr,
        "Duidt een eenheid aan die deel uitmaakt van een organisatie, zoals een departement in een grotere formele organisatie. Is het omgekeerde van `org:unitOf`."@nl .

org:identifier a rdf:Property,
        owl:DatatypeProperty ;
    rdfs:label "identifier"@en,
        "identifiant"@fr,
        "ID"@nl ;
    rdfs:domain org:Organization ;
    rdfs:isDefinedBy <http://www.w3.org/ns/org> ;
    rdfs:subPropertyOf skos:notation ;
    skos:definition "Gives an identifier, such as a company registration number, that can be used to used to uniquely identify the organization."@en,
        "Donne un identifiant, comme par exemple le numéro d'enregistrement d'une entreprise, qui peut être utilisé comme identifiant unique pour l'Organisation."@fr,
        "Geeft een ID, zoals een bedrijfsregistratienummer, dat gebruikt kan worden om de organisatie uniek te identificeren."@nl .

org:role a rdf:Property,
        owl:ObjectProperty ;
    rdfs:label "role"@en,
        "rôle"@fr,
        "rol"@nl ;
    rdfs:domain org:Post ;
    rdfs:isDefinedBy <http://www.w3.org/ns/org> ;
    rdfs:range org:Role ;
    skos:definition "Indicates the Role that the Agent plays in a Membership relationship with an Organization."@en,
        "Indique le Rôle de l'Agent dans son Engagement avec l'Organisation."@fr,
        "Duidt de rol aan die een Agent uitvoert in relatie met een organisatie."@nl .

org:siteAddress a rdf:Property,
        owl:ObjectProperty ;
    rdfs:label "site Address"@en,
        "adresse du Site"@fr,
        "adres van de zetel"@nl ;
    rdfs:domain org:Site ;
    rdfs:isDefinedBy <http://www.w3.org/ns/org> ;
    skos:definition "Indicates an address for the site in a suitable encoding. Use of vCard (using the http://www.w3.org/TR/vcard-rdf/ vocabulary) is encouraged but the range is left open to allow other encodings to be used. The address may include email, telephone, and geo-location information and is not restricted to a physical address."@en,
        "Indique une adresse pour le site dans un encodage approprié. L'usage du vocabulaire vCard ( http://www.w3.org/TR/vcard-rdf/) est encouragé, mais le range est ouvert pour permettre l'utilisation d'autres vocabulaires. L'adresse peut comporter le courriel, le téléphone, et l'information de géolocalisation; et n'est donc pas seulement limitée à une adresse physique."@fr,
        "Duidt het adres aan van de zetel in een geschikte encoding. Het gebruik van vCard (met de http://www.w3.org/TR/vcard-rdf/ vocabulary) wordt aangemoedigd, maar de range wordt open gelaten om andere encodings mogelijk te maken. Het adres kan de e-mail, het telefoonnummer en geo-locatie informatie bevatten. Het is niet beperkt tot een fysiek adres."@nl .

org:unitOf a rdf:Property,
        owl:ObjectProperty ;
    rdfs:label "unit Of"@en,
        "unité de"@fr,
        "organisatie-eenheid van"@nl ;
    rdfs:domain org:OrganizationalUnit ;
    rdfs:isDefinedBy <http://www.w3.org/ns/org> ;
    rdfs:range org:FormalOrganization ;
    rdfs:subPropertyOf org:subOrganizationOf ;
    skos:definition "Indicates an Organization of which this Unit is a part, e.g. a Department within a larger FormalOrganization. This is the inverse of `org:hasUnit`."@en,
        "Indique l'Organisation dont cette Organisation ou Unité fait partie, par exemple un Départment au sein d'une Organisation Formelle plus large. Inverse de `org:hasUnit`."@fr,
        "Duidt de Organisatie aan waarvan deze Organisatie of eenheid deel uitmaakt, bv. een departement binnen een grotere formele Organisatie. Omgekeerde van `org:hasUnit`."@nl .

prov:generatedAtTime a owl:DatatypeProperty ;
    rdfs:label "generated at time"@en,
        "a généré au moment"@fr,
        "genereerde op tijdstip"@nl ;
    rdfs:domain prov:Entity ;
    rdfs:isDefinedBy <http://www.w3.org/ns/prov-o#> ;
    rdfs:range xsd:dateTime .

prov:invalidatedAtTime a owl:DatatypeProperty ;
    rdfs:label "invalidated at time"@en,
        "invalidé au moment"@fr,
        "ongeldig gemaakt op tijdstip"@nl ;
    rdfs:domain prov:Entity ;
    rdfs:isDefinedBy <http://www.w3.org/ns/prov-o#> ;
    rdfs:range xsd:dateTime ;
    skos:definition "The time at which an entity was invalidated (i.e., no longer usable)."@en,
        "Le moment où une entité a été invalidée (c'est-à-dire n'est plus utilisable)."@fr,
        "Het tijdstip waarop een entiteit ongeldig werd gemaakt (d.w.z. niet langer bruikbaar)."@nl .

prov:wasAttributedTo a owl:ObjectProperty ;
    rdfs:label "was attributed to"@en,
        "a été attribué à"@fr,
        "is toegekend aan"@nl ;
    rdfs:domain prov:Entity ;
    rdfs:isDefinedBy <http://www.w3.org/ns/prov-o#> ;
    rdfs:range prov:Agent ;
    rdfs:subPropertyOf prov:wasInfluencedBy ;
    owl:propertyChainAxiom ( prov:qualifiedAttribution prov:agent ) ;
    skos:definition "Attribution is the ascribing of an entity to an agent."@en,
        "Attribution est l'attribution d'une entité à un agent."@fr,
        "Toekenning is het toekennen van een entiteit aan een agent."@nl .

<http://xmlns.com/foaf/0.1/homepage> a rdf:Property ;
    rdfs:label "homepage"@en,
        "page d'accueil"@fr,
        "homepagina"@nl ;
    rdfs:domain owl:Thing ;
    rdfs:isDefinedBy <http://xmlns.com/foaf/0.1/> ;
    rdfs:range <http://xmlns.com/foaf/0.1/Document> ;
    skos:definition "A homepage for some thing. "@en,
        "Une page d'accueil pour quelque chose"@fr,
        "Een homepagina van/voor iets"@nl .

<https://data.hetarchief.be/ns/description/audioNoiseReduction> a rdf:Property ;
    rdfs:label "audio noise reduction"@en,
        "réduction du bruit audio"@fr,
        "audio ruisonderdrukking"@nl ;
    rdfs:domain <https://data.hetarchief.be/ns/object/PhysicalCarrier> ;
    rdfs:isDefinedBy <https://data.hetarchief.be/ns/description/> ;
    rdfs:range rdf:Literal ;
    skos:definition "The technology used for noise reduction in audio."@en,
        "La technologie utilisée pour la réduction du bruit de l'audio."@fr,
        "De techniek die gebruikt wordt voor ruisonderdrukking bij audio."@nl .

<https://data.hetarchief.be/ns/description/audioRecordingSpeed> a rdf:Property ;
    rdfs:label "audio recording speed"@en,
        "vitesse d'enregistrement audio"@fr,
        "audio-opnamesnelheid"@nl ;
    rdfs:domain <https://data.hetarchief.be/ns/object/PhysicalCarrier> ;
    rdfs:isDefinedBy <https://data.hetarchief.be/ns/description/> ;
    rdfs:range skos:Concept ;
    skos:definition "The speed with which open reel audio or a gramophone record is recorded."@en,
        "La vitesse à laquelle l'audio à bobine ouverte ou un enregistrement de gramophone est enregistré."@fr,
        "De snelheid waarmee openspoelaudio of een grammofoonplaat wordt opgenomen."@nl .

<https://data.hetarchief.be/ns/description/chapterNumber> a rdf:Property ;
    rdfs:label "DVD chapter number"@en,
        "Numéro de chapitre DVD"@fr,
        "Dvd-hoofdstuknummer"@nl ;
    rdfs:domain <https://data.hetarchief.be/ns/description/DVDChapter> ;
    rdfs:isDefinedBy <https://data.hetarchief.be/ns/description/> ;
    rdfs:range xsd:integer ;
    rdfs:subPropertyOf schema:position ;
    skos:definition "The sequence number of the DVD chapter in relation to the other chapters that are part of the same DVD."@en,
        "Le numéro de série du chapitre du DVD par rapport aux autres chapitres qui font partie du même DVD."@fr,
        "Het volgnummer van het dvd-hoofdstuk ten opzichte van de andere hoofstukken die deel uitmaken van dezelfde dvd."@nl .

<https://data.hetarchief.be/ns/description/coloringType> a rdf:Property ;
    rdfs:label "type of coloring image reel"@en,
        "type de coloration bobine d'image"@fr,
        "type kleuring filmspoel"@nl ;
    rdfs:domain <https://data.hetarchief.be/ns/description/ImageReel> ;
    rdfs:isDefinedBy <https://data.hetarchief.be/ns/description/> ;
    rdfs:range skos:Concept ;
    rdfs:subPropertyOf <http://dbpedia.org/ontology/filmColourType> ;
    skos:definition "The type of coloring of the image reel."@en,
        "Le type de coloration de la bobine d’image."@fr,
        "Het soort kleuring van de beeldrol/-spoel."@nl .

<https://data.hetarchief.be/ns/description/hasMissingAudioReels> a rdf:Property ;
    rdfs:label "missing audio reels"@en,
        "bobines audio manquantes"@fr,
        "ontbrekende audiospoelen"@nl ;
    rdfs:domain <https://data.hetarchief.be/ns/object/CarrierRepresentation> ;
    rdfs:isDefinedBy <https://data.hetarchief.be/ns/description/> ;
    rdfs:range rdfs:Literal ;
    skos:definition "Indicates for a film if audio reels are missing, preceding any digitization process."@en,
        "Indique pour un film si des bobines audio sont manquantes, avant toute opération de numérisation."@fr,
        "Duidt aan voor een film of er audiorollen/-spoelen ontbreken, voorafgaand aan enig digitaliseringsproces."@nl .

<https://data.hetarchief.be/ns/description/hasMissingImageReels> a rdf:Property ;
    rdfs:label "missing image reels"@en,
        "bobines d'image manquantes"@fr,
        "ontbrekende beeldspoelen"@nl ;
    rdfs:domain <https://data.hetarchief.be/ns/object/CarrierRepresentation> ;
    rdfs:isDefinedBy <https://data.hetarchief.be/ns/description/> ;
    rdfs:range rdfs:Literal ;
    skos:definition "Indicates for a film if image reels are missing, preceding any digitization process."@en,
        "Indique pour un film si des bobines d'image sont manquantes, avant toute opération de numérisation."@fr,
        "Duidt aan voor een film of er beeldrollen/-spoelen ontbreken, voorafgaand aan enig digitaliseringsproces."@nl .

<https://data.hetarchief.be/ns/description/iec60094Type> a rdf:Property ;
    rdfs:label "iec-60094 type"@en,
        "iec-60094 type"@fr,
        "iec-60094 type"@nl ;
    rdfs:domain <https://data.hetarchief.be/ns/object/PhysicalCarrier> ;
    rdfs:isDefinedBy <https://data.hetarchief.be/ns/description/> ;
    rdfs:range skos:Concept ;
    skos:definition "The IEC-60094 Type of the compact cassette that indicates the magnetic material used as a binder on top of the polyester bottom layer of the cassette."@en,
        "Le type IEC-60094 de la cassette compacte qui indique le matériau magnétique utilisé comme liant sur le dessus de la couche inférieure en polyester de la cassette."@fr,
        "Het iec-60094 type van de compact cassette die duidt op het magnetisch materiaal dat als bindmiddel werd gebruikt bovenop de polyester onderlaag van de cassette."@nl .

<https://data.hetarchief.be/ns/description/numberOfAudioChannels> a rdf:Property ;
    rdfs:label "number of audio channels"@en,
        "nombre de canaux audio"@fr,
        "aantal audiokanalen"@nl ;
    rdfs:domain <https://data.hetarchief.be/ns/object/CarrierRepresentation> ;
    rdfs:isDefinedBy <https://data.hetarchief.be/ns/description/> ;
    rdfs:range rdfs:Literal ;
    skos:definition "The number of parallel audio channels that the audio track contains."@en,
        "Le nombre de canaux audio parallèles que contient la piste audio."@fr,
        "Het aantal audiokanalen die een audiospoor bevat."@nl .

<https://data.hetarchief.be/ns/description/numberOfAudioTracks> a rdf:Property ;
    rdfs:label "number of audio tracks"@en,
        "nombre de pistes audio"@fr,
        "aantal audiosporen"@nl ;
    rdfs:domain <https://data.hetarchief.be/ns/object/CarrierRepresentation> ;
    rdfs:isDefinedBy <https://data.hetarchief.be/ns/description/> ;
    rdfs:range rdfs:Literal ;
    skos:definition "The number of audio tracks that the representation contains."@en,
        "Le nombre de pistes audio que la représentation contient."@fr,
        "Het aantal audio sporen die de representatie bevat."@nl .

<https://data.hetarchief.be/ns/description/numberOfMissingAudioReels> a rdf:Property ;
    rdfs:label "number of missing audio reels"@en,
        "nombre de bobines audio manquantes"@fr,
        "aantal ontbrekende audiospoelen"@nl ;
    rdfs:domain <https://data.hetarchief.be/ns/object/CarrierRepresentation> ;
    rdfs:isDefinedBy <https://data.hetarchief.be/ns/description/> ;
    rdfs:range rdfs:Literal ;
    skos:definition "Indicates for a film how many audio reels are missing, preceding any digitization process."@en,
        "Indique pour un film combien des bobines audio sont manquantes, avant toute opération de numérisation."@fr,
        "Duidt aan voor een film hoeveel audiorollen/-spoelen ontbreken, voorafgaand aan enig digitaliseringsproces."@nl .

<https://data.hetarchief.be/ns/description/numberOfMissingImageReels> a rdf:Property ;
    rdfs:label "number of missing image reels"@en,
        "nombre de bobines d'image manquantes"@fr,
        "aantal ontbrekende beeldspoelen"@nl ;
    rdfs:domain <https://data.hetarchief.be/ns/object/CarrierRepresentation> ;
    rdfs:isDefinedBy <https://data.hetarchief.be/ns/description/> ;
    rdfs:range rdfs:Literal ;
    skos:definition "Indicates for a film how many image reels are missing, preceding any digitization process."@en,
        "Indique pour un film combien des bobines d'image sont manquantes, avant toute opération de numérisation."@fr,
        "Duidt aan voor een film hoeveel beeldrollen/-spoelen ontbreken, voorafgaand aan enig digitaliseringsproces."@nl .

<https://data.hetarchief.be/ns/description/numberOfPages> a rdf:Property ;
    rdfs:label "number of pages"@en,
        "nombre de pages"@fr,
        "aantal pagina's"@nl ;
    rdfs:domain <https://data.hetarchief.be/ns/description/NewspaperIssue> ;
    rdfs:isDefinedBy <https://data.hetarchief.be/ns/description/> ;
    rdfs:range rdfs:Literal ;
    skos:definition "The number of pages that a particular work consists of."@en,
        "Le nombre de pages qui composent une œuvre particulière."@fr,
        "Het aantal pagina's waaruit een bepaald werk bestaat."@nl ;
    skos:related schema:numberOfPages .

<https://data.hetarchief.be/ns/description/numberOfReels> a rdf:Property ;
    rdfs:label "number of film reels"@en,
        "nombre de bobines de film"@fr,
        "aantal filmrollen/-spoelen"@nl ;
    rdfs:domain <https://data.hetarchief.be/ns/object/CarrierRepresentation> ;
    rdfs:isDefinedBy <https://data.hetarchief.be/ns/description/> ;
    rdfs:range rdfs:Literal ;
    skos:definition "The number of film reels (regardless of type) that make up a digitized film."@en,
        "Le nombre de bobines de film (quel que soit le type) qui composent un film numérisé."@fr,
        "Het aantal filmrollen/-spoelen (ongeacht het type) waaruit een gedigitaliseerde film bestaat."@nl .

<https://data.hetarchief.be/ns/description/pageNumber> a rdf:Property ;
    rdfs:label "page number"@en,
        "numéro de page"@fr,
        "paginanummer"@nl ;
    rdfs:domain <https://data.hetarchief.be/ns/description/NewspaperIssuePage> ;
    rdfs:isDefinedBy <https://data.hetarchief.be/ns/description/> ;
    rdfs:range rdfs:Literal ;
    rdfs:subPropertyOf schema:position ;
    skos:definition "The sequence number of a page within its larger whole (e.g. a newspaper edition, a book, etc.)."@en,
        "Le numéro de séquence d'une page dans son ensemble plus grand (par exemple, une édition de journal, un livre, etc.)."@fr,
        "Het volgnummer van een pagina binnen zijn groter geheel (bv. een kranteneditie, een boek, etc.)."@nl .

<https://data.hetarchief.be/ns/event> a owl:Ontology ;
    dct:author [ schema:email "milan.valadou@meemoo.be" ;
            schema:name "Milan Valadou" ],
        [ schema:email "miel.vandersande@meemoo.be" ;
            schema:name "Miel Vander Sande" ],
        [ schema:email "lennert.vandevelde@meemoo.be" ;
            schema:name "Lennert Van de Velde" ] ;
    dct:created "2022-06-08" ;
    dct:description "Data model to describe events."@en,
        "Modèle de données pour décrire des événements."@fr,
        "Datamodel voor het beschrijven van gebeurtenissen."@nl ;
    dct:modified "2023-01-12" ;
    dct:title "Data model Events"@en,
        "Modèle de données Events"@fr,
        "Datamodel Events"@nl ;
    pav:version "0.0.1" ;
    vann:preferredNamespacePrefix "haEvt" ;
    vann:preferredNamespaceUri "http://data.hetarchief.be/ns/events/" ;
    owl:imports <http://id.loc.gov/vocabulary/preservation/eventOutcome>,
        <http://id.loc.gov/vocabulary/preservation/eventRelatedAgentRole>,
        <http://id.loc.gov/vocabulary/preservation/eventRelatedObjectRole>,
        <http://id.loc.gov/vocabulary/preservation/eventType>,
        premis: .

<https://data.hetarchief.be/ns/event#ActivityShape> a sh:NodeShape ;
    sh:property [ a sh:PropertyShape ;
            sh:description "The generated object."@en,
                "L'objet généré."@fr,
                "Het gegenereerde object."@nl ;
            sh:maxCount 1 ;
            sh:message "prov:generated occurs more than once or its value is not an IRI"@en,
                "prov:generated apparaît plus d'une fois ou sa valeur n'est pas un IRI"@fr,
                "prov:generated komt meer dan eens voor of de waarde is geen IRI"@nl ;
            sh:minCount 0 ;
            sh:name "has generated"@en,
                "a généré"@fr,
                "heeft gegenereerd"@nl ;
            sh:nodeKind sh:IRI ;
            sh:path prov:generated ;
            sh:severity sh:Violation ],
        [ a sh:PropertyShape ;
            sh:datatype xsd:dateTime ;
            sh:description "The start date of the activity."@en,
                "La date de début de l'activité."@fr,
                "De startdatum van de activiteit."@nl ;
            sh:maxCount 1 ;
            sh:message "prov:startedAtTime is absent, occurs more than once or its value is not of type xsd:dateTime"@en,
                "prov:startedAtTime est absent, apparaît plus d'une fois ou sa valeur n'est pas de type xsd:dateTime"@fr,
                "prov:startedAtTime ontbreekt, komt meer dan eens voor of de waarde is niet van het type xsd:dateTime"@nl ;
            sh:minCount 1 ;
            sh:name "has start date"@en,
                "a date de début"@fr,
                "heeft startdatum"@nl ;
            sh:path prov:startedAtTime ;
            sh:severity sh:Violation ],
        [ a sh:PropertyShape ;
            sh:datatype xsd:dateTime ;
            sh:description "The end date of the activity."@en,
                "La date de fin de l'activité."@fr,
                "De einddatum van de activiteit."@nl ;
            sh:maxCount 1 ;
            sh:message "prov:endedAtTime is absent, occurs more than once or its value is not of type xsd:dateTime"@en,
                "prov:endedAtTime est absent, apparaît plus d'une fois ou sa valeur n'est pas de type xsd:dateTime"@fr,
                "prov:endedAtTime ontbreekt, komt meer dan eens voor of de waarde is niet van het type xsd:dateTime"@nl ;
            sh:minCount 1 ;
            sh:name "has end date"@en,
                "a date de fin"@fr,
                "heeft einddatum"@nl ;
            sh:path prov:endedAtTime ;
            sh:severity sh:Violation ],
        [ a sh:PropertyShape ;
            rdfs:label "was associated with"@en,
                "a été associé à"@fr,
                "is geassocieerd met"@nl ;
            skos:definition "An agent that had some (unspecified) responsibility for the occurrence of this activity."@en,
                "Un agent qui avait une responsabilité (non spécifiée) avant la survenue de cette activité."@fr,
                "Een agent die enige (niet-gespecificeerde) verantwoordelijkheid had voor het optreden van deze activiteit."@nl ;
            sh:maxCount 1 ;
            sh:message "prov:wasAssociatedWith is absent, occurs more than once or its value is not an instance of classes schema:Person/org/Organization/premis:SoftwareAgent/premis:HardwareAgent"@en,
                "prov:wasAssociatedWith est absent, apparaît plus d'une fois ou sa valeur n'est pas une instance de classes schema:Person/org/Organization/premis:SoftwareAgent/premis:HardwareAgent"@fr,
                "prov:wasAssociatedWith ontbreekt, komt meer dan eens voor of de waarde is geen instantie van de klassen schema:Person/org/Organization/premis:SoftwareAgent/premis:HardwareAgent"@nl ;
            sh:minCount 1 ;
            sh:or ( [ sh:class schema:Person ] [ sh:class org:Organization ] [ sh:class premis:SoftwareAgent ] [ sh:class premis:HardwareAgent ] ) ;
            sh:path prov:wasAssociatedWith ;
            sh:severity sh:Violation ] ;
    sh:targetClass prov:Activity .

<https://data.hetarchief.be/ns/event#BrandShape> a sh:NodeShape ;
    sh:property [ a sh:PropertyShape ;
            sh:datatype rdf:langString ;
            sh:maxCount 1 ;
            sh:message "schema:name is missing or not of type string "@en,
                "schema:name est manquant ou n'est pas de type string"@fr,
                "schema:name ontbreekt of is niet van het type string"@nl ;
            sh:minCount 1 ;
            sh:name "name"@en,
                "nom"@fr,
                "naam"@nl ;
            sh:nodeKind sh:Literal ;
            sh:path schema:name ;
            sh:severity sh:Violation ] ;
    sh:targetClass schema:Brand .

<https://data.hetarchief.be/ns/event#EventShape> a sh:NodeShape ;
    sh:property [ a sh:PropertyShape ;
            sh:class premis:OutcomeStatus ;
            sh:description "The outcome status of the event."@en,
                "Statut du résultat de l'événement (Event)."@fr,
                "De uitkomststatus van de gebeurtenis (Event)."@nl ;
            sh:in ( evtOutcome:fai evtOutcome:suc evtOutcome:war ) ;
            sh:maxCount 1 ;
            sh:message "premis:outcome is absent, occurs more than once or its value is not in the list (evtOutcome:fai evtOutcome:suc evtOutcome:war)"@en,
                "premis:outcome est absent, apparaît plus d'une fois ou sa valeur n'est pas dans la liste (evtOutcome:fai evtOutcome:suc evtOutcome:war)"@fr,
                "premis:outcome ontbreekt, komt meer dan eens voor of de waarde maakt geen deel uit van de lijst (evtOutcome:fai evtOutcome:suc evtOutcome:war)"@nl ;
            sh:minCount 0 ;
            sh:name "has outcome"@en,
                "a résultat"@fr,
                "heeft uitkomst"@nl ;
            sh:path premis:outcome ;
            sh:severity sh:Violation ],
        [ a sh:PropertyShape ;
            sh:datatype xsd:string ;
            sh:description "A note about the outcome of the event."@en,
                "Une note sur le résultat de l'événement (Event)."@fr,
                "Een opmerking over de uitkomst van de gebeurtenis (Event)."@nl ;
            sh:maxCount 1 ;
            sh:message "premis:outcomeNote occurs more than once or its value is not of type string"@en,
                "premis:outcomeNote apparaît plus d'une seule fois ou sa valeur n'est pas de type string"@fr,
                "premis:outcomeNote komt meer dan eens voor of de waarde is niet van het type string"@nl ;
            sh:minCount 0 ;
            sh:name "has outcome note"@en,
                "a une note de résultat"@fr,
                "heeft uitkomstopmerking"@nl ;
            sh:path premis:outcomeNote ;
            sh:severity sh:Violation ],
        [ a sh:PropertyShape ;
            sh:datatype xsd:string ;
            sh:description "A note about the event."@en,
                "Une note sur l'événement (Event)"@fr,
                "Een opmerking over de gebeurtenis (Event)."@nl ;
            sh:maxCount 1 ;
            sh:message "premis:note occurs more than once or its value is not of type string"@en,
                "premis:note apparaît plus d'une seule fois ou sa valeur n'est pas de type string"@fr,
                "premis:note komt meer dan eens voor of de waarde is niet van het type string"@nl ;
            sh:minCount 0 ;
            sh:name "has note"@en,
                "a une note"@fr,
                "heeft opmerking"@nl ;
            sh:path premis:note ;
            sh:severity sh:Violation ],
        [ a sh:PropertyShape ;
            sh:class premis:Object ;
            sh:description "The object that was generated by the event."@en,
                "L'objet généré par l'événement (Event)."@fr,
                "Het object dat door de gebeurtenis (Event) gegenereerd is."@nl ;
            sh:message "evtObjRole:out occurs more than once or its value is no instance of class premis:Object"@en,
                "evtObjRole:out apparaît plus d'une seule fois ou sa valeur n'est pas une instance de la classe premis:Object"@fr,
                "evtObjRole:out komt meer dan eens voor of de waarde is geen instantie van de klasse premis:Object"@nl ;
            sh:name "result"@en,
                "résultat"@fr,
                "resultaat"@nl ;
            sh:path evtObjRole:out ;
            sh:severity sh:Violation ],
        [ a sh:PropertyShape ;
            sh:class premis:Object ;
            sh:description "The object that was used as a source for the event."@en,
                "L'object utilisé comme source pour l'événement (Event)"@fr,
                "Het object dat als bron gebruikt is voor de gebeurtenis (Event)."@nl ;
            sh:message "evtObjRole:sou occurs more than once or its value is no instance of class premis:Object"@en,
                "evtObjRole:sou apparaît plus d'une seule fois ou sa valeur n'est pas une instance de la classe premis:Object"@fr,
                "evtObjRole:sou komt meer dan eens voor of de waarde is geen instantie van de klasse premis:Object"@nl ;
            sh:name "has source"@en,
                "a une source"@fr,
                "heeft bron"@nl ;
            sh:path evtObjRole:sou ;
            sh:severity sh:Violation ],
        [ a sh:PropertyShape ;
            sh:class org:Organization ;
            sh:description "The organization that implemented the event."@en,
                "L'organisation qui a implementé l'événement (Event)."@fr,
                "De organisatie die de gebeurtenis (Event) heeft geimplementeerd."@nl ;
            sh:maxCount 1 ;
            sh:message "evtAgRole:imp is absent, occurs more than once or its value is no instance of class org:Organization"@en,
                "evtAgRole:imp est absent, apparaît plus d'une seule fois ou sa valeur n'est pas une instance de la classe org:Organization"@fr,
                "evtAgRole:imp ontbreekt, komt meer dan eens voor of de waarde is geen instantie van de klasse org:Organization"@nl ;
            sh:minCount 1 ;
            sh:name "implemented by"@en,
                "implementé par"@fr,
                "geimplementeerd door"@nl ;
            sh:path evtAgRole:imp ;
            sh:severity sh:Violation ],
        [ a sh:PropertyShape ;
            sh:class premis:SoftwareAgent ;
            sh:description "The software that executed the event."@en,
                "Le logiciel qui a exécuté l'événement (Event)."@fr,
                "De software die de gebeurtenis (Event) heeft uitgevoerd."@nl ;
            sh:maxCount 1 ;
            sh:message "evtAgRole:exe occurs more than once or its value is no instance of classes premis:SoftwareAgent"@en,
                "evtAgRole:exe apparaît plus d'une seule fois ou sa valeur n'est pas une instance de classes premis:SoftwareAgent"@fr,
                "evtAgRole:exe komt meer dan eens voor of de waarde is geen instantie van de klassen premis:SoftwareAgent"@nl ;
            sh:minCount 0 ;
            sh:name "executed by"@en,
                "exécuté par"@fr,
                "uitgevoerd door"@nl ;
            sh:path evtAgRole:exe ;
            sh:severity sh:Violation ],
        [ a sh:PropertyShape ;
            sh:class premis:HardwareAgent ;
            sh:description "The hardware that was used to execute the event."@en,
                "Le matériel qui a été utilisé pour exécuter l'événement (Event)."@fr,
                "De hardware die gebruikt is voor het uitvoeren van de gebeurtenis (Event)."@nl ;
            sh:message "schema:instrument's value is no instance of classes premis:HardwareAgent"@en,
                "schema:instrument sa valeur n'est pas une instance de classes premis:HardwareAgent"@fr,
                "schema:instrument's waarde is geen instantie van de klassen premis:HardwareAgent"@nl ;
            sh:minCount 0 ;
            sh:name "instrument"@en,
                "instrument"@fr,
                "instrument"@nl ;
            sh:path schema:instrument ;
            sh:severity sh:Violation ] ;
    sh:targetClass premis:Event .

<https://data.hetarchief.be/ns/event#HardwareAgentShape> a sh:NodeShape ;
    sh:property <https://data.hetarchief.be/ns/event#NameShape>,
        <https://data.hetarchief.be/ns/event#brandShape>,
        <https://data.hetarchief.be/ns/event#modelShape>,
        <https://data.hetarchief.be/ns/event#serialNumberShape>,
        <https://data.hetarchief.be/ns/event#versionShape> ;
    sh:targetClass premis:HardwareAgent .

<https://data.hetarchief.be/ns/event#ObjectShape> a sh:NodeShape ;
    sh:property [ a sh:PropertyShape ;
            sh:class premis:Event ;
            sh:description "The time at which the object was completely created and is available for use."@en,
                "Heure à laquelle l'objet a été complètement créé et est disponible pour utilisation."@fr,
                "De tijd waarop het object volledig is aangemaakt en beschikbaar is voor gebruik."@nl ;
            sh:maxCount 1 ;
            sh:message "prov:wasGeneratedBy occurs more than once or its value is no instance of premis:Event"@en,
                "prov:wasGeneratedBy apparaît plus d'une seule fois ou sa valeur n'est pas une instance de premis:Event"@fr,
                "prov:wasGeneratedBy komt meer dan eens voor of de waarde is geen instantie van premis:Event"@nl ;
            sh:minCount 0 ;
            sh:name "was generated by"@en,
                "généré par"@fr,
                "is gegenereerd door"@nl ;
            sh:path prov:wasGeneratedBy ;
            sh:severity sh:Violation ] ;
    sh:targetClass premis:Object .

<https://data.hetarchief.be/ns/event#SoftwareAgentShape> a sh:NodeShape ;
    sh:property <https://data.hetarchief.be/ns/event#NameShape>,
        <https://data.hetarchief.be/ns/event#brandShape>,
        <https://data.hetarchief.be/ns/event#modelShape>,
        <https://data.hetarchief.be/ns/event#serialNumberShape>,
        <https://data.hetarchief.be/ns/event#versionShape> ;
    sh:targetClass premis:SoftwareAgent .

<https://data.hetarchief.be/ns/mediahaven/record> a rdf:Property ;
    rdfs:label "record"@en,
        "enregistrement"@fr,
        "record"@nl ;
    rdfs:domain <https://data.hetarchief.be/ns/mediahaven/Fragment> ;
    rdfs:isDefinedBy <https://data.hetarchief.be/ns/mediahaven/> ;
    rdfs:range <https://data.hetarchief.be/ns/mediahaven/Record> ;
    skos:definition "The record in the Mediahaven asset management system."@en,
        "L'enregistrement dans le système de gestion d'actifs Mediahaven."@fr,
        "Het fragment in het Mediahaven asset management systeem."@nl .

<https://data.hetarchief.be/ns/mediahaven/tenantName> a rdf:Property ;
    rdfs:label "tenant name"@en,
        "nom du locataire"@fr,
        "tenant naam"@nl ;
    rdfs:domain org:Organization ;
    rdfs:isDefinedBy <https://data.hetarchief.be/ns/mediahaven/> ;
    rdfs:range xsd:string ;
    skos:definition "The Mediahaven tenant name of the organization."@en,
        "Le nom du locataire Mediahaven de l'organisation."@fr,
        "De Mediahaven tenant naam van de organisatie."@nl .

<https://data.hetarchief.be/ns/object/preservationProblem> a rdf:Property ;
    rdfs:label "preservation problem"@en,
        "problème de préservation"@fr,
        "preservatieprobleem"@nl ;
    rdfs:isDefinedBy <https://data.hetarchief.be/ns/object/> .

<https://data.hetarchief.be/ns/object/primaryIdentifier> a rdf:Property ;
    rdfs:label "has primary identifier"@en,
        "a identifiant principal"@fr,
        "heeft primaire identificatiecode"@nl ;
    rdfs:isDefinedBy <https://data.hetarchief.be/ns/object/> ;
    rdfs:range <https://data.hetarchief.be/ns/object/LocalIdentifier> ;
    rdfs:subPropertyOf premis:identifier .

<https://data.hetarchief.be/ns/organization/hasLogo> a rdf:Property ;
    rdfs:label "has a logo"@en,
        "a un logo"@fr,
        "heeft een logo"@nl ;
    rdfs:domain org:Organization ;
    rdfs:isDefinedBy <https://data.hetarchief.be/ns/organization/> ;
    rdfs:range <https://data.hetarchief.be/ns/organization/Logo> ;
    skos:definition "A logo for an organization."@en,
        "Un logo pour une organisation."@fr,
        "Een logo voor een organisatie."@nl .

<https://data.hetarchief.be/ns/organization/hasPreference> a rdf:Property ;
    rdfs:label "prefers"@en,
        "préfère"@fr,
        "verkiest"@nl ;
    rdfs:domain org:Organization ;
    rdfs:isDefinedBy <https://data.hetarchief.be/ns/organization/> ;
    rdfs:range skos:Concept ;
    skos:definition "Expresses the wish of an organization regarding whether or not to perform a certain service in collaboration with/by meemoo."@en,
        "Exprime le souhait d'une organisation quant à la réalisation ou non d'un certain service en collaboration avec/par meemoo."@fr,
        "Drukt de wens uit van een organisatie met betrekking tot het al dan niet uitvoeren van een bepaalde service in samenwerking met/door meemoo."@nl .

<https://data.hetarchief.be/ns/organization/requestForm> a rdf:Property ;
    rdfs:label "request form"@en,
        "formulaire de demande"@fr,
        "aanvraagformulier"@nl ;
    rdfs:domain <https://data.hetarchief.be/ns/organization/ContentPartner> ;
    rdfs:isDefinedBy <https://data.hetarchief.be/ns/organization/> ;
    rdfs:range rdfs:Literal ;
    skos:definition "A link to a form with which a user can request content from the content partner."@en,
        "Un lien vers un formulaire avec lequel un utilisateur peut demander du contenu au partenaire de contenu."@fr,
        "Een link naar een formulier waarmee een gebruiker materiaal kan aanvragen bij de contentpartner "@nl .

<https://data.hetarchief.be/ns/organization/sector> a rdf:Property ;
    rdfs:label "sector"@en,
        "secteur"@fr,
        "sector"@nl ;
    rdfs:domain org:Organization ;
    rdfs:isDefinedBy <https://data.hetarchief.be/ns/organization/> ;
    rdfs:range rdfs:Literal ;
    skos:definition "The sector the organisation is active in."@en,
        "Le secteur dans lequel l'organisation est active."@fr,
        "De sector waarin de organisatie actief is."@nl .

schema:about a rdf:Property ;
    rdfs:label "about"@en,
        "sur"@fr,
        "over"@nl ;
    rdfs:domain schema:CreativeWork ;
    rdfs:isDefinedBy schema: ;
    rdfs:range schema:Thing ;
    skos:definition "The subject matter of the content."@en,
        "Le sujet du contenu."@fr,
        "Het onderwerp van de inhoud."@nl .

schema:abstract a rdf:Property ;
    rdfs:label "abstract"@en,
        "résumé"@fr,
        "abstract"@nl ;
    rdfs:domain schema:CreativeWork ;
    rdfs:isDefinedBy schema: ;
    rdfs:range xsd:string ;
    owl:equivalentProperty dct:abstract ;
    skos:definition "An abstract is a short description that summarizes a CreativeWork."@en,
        "Un résumé est une description courte qui résume un CreativeWork."@fr,
        "Een abstract is een korte beschrijving die een CreativeWork samenvat."@nl .

schema:actor a rdf:Property ;
    rdfs:label "actor"@en,
        "acteur"@fr,
        "acteur"@nl ;
    rdfs:domain schema:CreativeWork ;
    rdfs:isDefinedBy schema: ;
    rdfs:range schema:Person ;
    skos:definition "An actor, e.g. in tv, radio, movie, video games etc., or in an event. Actors can be associated with individual items or with a series, episode, clip."@en,
        "Un acteur, par exemple à la télévision, à la radio, au cinéma, dans les jeux vidéo, etc. ou dans un événement. Les acteurs peuvent être associés à des éléments individuels ou à une série, un épisode, un clip."@fr,
        "Een acteur, bv. in tv, radio, film, videogames etc. of in een evenement. Acteurs kunnen geassocieerd worden met met individuele items of met een serie, aflevering, clip."@nl .

schema:addressCountry a rdf:Property ;
    rdfs:label "addressCountry"@en,
        "partie de l'adresse concernant le pays"@fr,
        "deel van het adres met betrekking tot het land"@nl ;
    rdfs:isDefinedBy schema: ;
    skos:definition "The country. For example, USA. You can also provide the two-letter [ISO 3166-1 alpha-2 country code](http://en.wikipedia.org/wiki/ISO_3166-1)."@en,
        "Le pays."@fr,
        "Het land."@nl ;
    schema:domainIncludes schema:DefinedRegion,
        schema:GeoCoordinates,
        schema:GeoShape,
        schema:PostalAddress ;
    schema:rangeIncludes schema:Country,
        schema:Text .

schema:addressLocality a rdf:Property ;
    rdfs:label "addressLocality"@en,
        "localitéAdresse"@fr,
        "adresPlaats"@nl ;
    rdfs:isDefinedBy schema: ;
    skos:definition "The locality in which the street address is, and which is in the region. For example, Mountain View."@en,
        "La localité dans laquelle se trouve l'adresse de rue, et qui se trouve dans la région."@fr,
        "De plaats waar het straatadres zich bevindt, en de plaats van de regio."@nl ;
    schema:domainIncludes schema:PostalAddress ;
    schema:rangeIncludes schema:Text .

schema:addressRegion a rdf:Property ;
    rdfs:label "addressRegion"@en,
        "addresseRegion"@fr,
        "adresRegio"@nl ;
    rdfs:isDefinedBy schema: ;
    skos:definition "The region in which the locality is, and which is in the country. For example, California or another appropriate first-level [Administrative division](https://en.wikipedia.org/wiki/List_of_administrative_divisions_by_country)."@en,
        "La région dans laquelle se trouve la localité, et qui se trouve dans le pays. Par exemple, la Californie ou [une autre division administrative appropriée de premier niveau](https://fr.wikipedia.org/wiki/Liste_des_subdivisions_par_pays)."@fr,
        "De regio waarin de plaats zich bevindt, en die in het land ligt. Bijvoorbeeld, Californië of een ander geschikte [administratieve afdeling van het eerste niveau](https://nl.wikipedia.org/wiki/Bestuurslagen_per_land)."@nl ;
    schema:domainIncludes schema:DefinedRegion,
        schema:PostalAddress ;
    schema:rangeIncludes schema:Text .

schema:alternateName a rdf:Property ;
    rdfs:label "alternate name"@en,
        "nom alternatif"@fr,
        "alternatieve naam"@nl ;
    rdfs:domain schema:Thing ;
    rdfs:isDefinedBy schema: ;
    rdfs:range xsd:string ;
    owl:equivalentProperty dct:alternative ;
    skos:definition "An alias for the item"@en,
        "Un alias pour l'élément"@fr,
        "Een alias voor het item"@nl .

schema:artMedium a rdf:Property ;
    rdfs:label "art medium"@en,
        "médium artistique"@fr,
        "kunst medium"@nl ;
    rdfs:domain schema:CreativeWork ;
    rdfs:isDefinedBy schema: ;
    rdfs:range xsd:string ;
    owl:equivalentProperty dct:medium ;
    skos:definition "The material used. (e.g. Oil, Watercolour, Acrylic, Linoprint, Marble, Cyanotype, Digital, Lithograph, DryPoint, Intaglio, Pastel, Woodcut, Pencil, Mixed Media, etc.)"@en,
        "Le matériau utilisé. (par exemple Huile, Aquarelle, Acrylique, Linoprint, Marbre, Cyanotype, Numérique, Lithographie, Point sec, Intaglio, Pastel, Gravure sur bois, Crayon, Médias mixtes, etc.)"@fr,
        "Het gebruikte materiaal. (bv. Olie, Aquarel, Acryl, Linoprint, Marmer, Cyanotype, Digitaal, Lithografie, Droogpunt, Intaglio, Pastel, Houtsnede, Potlood, Gemengde media, etc.)"@nl .

schema:artform a rdf:Property ;
    rdfs:label "artform"@en,
        "forme artistique"@fr,
        "kunstvorm"@nl ;
    rdfs:domain schema:CreativeWork ;
    rdfs:isDefinedBy schema: ;
    rdfs:range xsd:string ;
    skos:definition "The artform, medium, or mode of this creative work for example Painting, Drawing, Sculpture, Print, Photograph, Assemblage, Collage, etc."@en,
        "La forme artistique, le support ou le mode de ce travail créatif, par exemple Peinture, Dessin, Sculpture, Impression, Photographie, Assemblage, Collage, etc."@fr,
        "De kunstvorm, het medium of de vorm van dit creatieve werk, bijvoorbeeld Schilderij, Tekening, Beeldhouwwerk, Print, Foto, Assemblage, Collage, etc."@nl .

schema:birthDate a rdf:Property ;
    rdfs:label "birth date"@en,
        "date de naissance"@fr,
        "geboortedatum"@nl ;
    rdfs:domain schema:Person ;
    rdfs:isDefinedBy schema: ;
    rdfs:range xsd:date ;
    skos:definition "Date of birth"@en,
        "Date de naissance"@fr,
        "Geboortedatum"@nl .

schema:caption a rdf:Property ;
    rdfs:label "caption"@en,
        "sous-titrage"@fr,
        "ondertiteling"@nl ;
    rdfs:domain schema:CreativeWork ;
    rdfs:isDefinedBy schema: ;
    rdfs:range xsd:string ;
    skos:definition "The caption for this object."@en,
        "Les sous-titres de cet objet."@fr,
        "De ondertiteling voor dit object."@nl .

schema:contactPoint a rdf:Property ;
    rdfs:label "contactPoint"@en,
        "pointDeContact"@fr,
        "aanspreekpunt"@nl ;
    rdfs:isDefinedBy schema: ;
    skos:definition "A contact point for a person or organization."@en,
        "Un point de contact pour une personne ou une organisation."@fr,
        "Een aanspreekpunt voor een persoon of een organisatie."@nl ;
    schema:domainIncludes schema:HealthInsurancePlan,
        schema:Organization,
        schema:Person ;
    schema:rangeIncludes schema:ContactPoint .

schema:contactType a rdf:Property ;
    rdfs:label "contactType"@en,
        "typePointContact"@fr,
        "contactType"@nl ;
    rdfs:isDefinedBy schema: ;
    skos:definition "A person or organization can have different contact points, for different purposes. For example, a sales contact point, a PR contact point and so on. This property is used to specify the kind of contact point."@en,
        "Une personne ou une organisation peut avoir différents points de contact, à des fins différentes. Par exemple, un point de contact pour les ventes, un point de contact pour les relations publiques, etc. Cette propriété est utilisée pour spécifier le type de point de contact."@fr,
        "Een persoon of organisatie kan verschillende contactpunten hebben, voor verschillende doeleinden. Bijvoorbeeld een verkoopcontactpunt, een PR-contactpunt enzovoort. Deze eigenschap wordt gebruikt om het soort contactpunt te specificeren."@nl ;
    schema:domainIncludes schema:ContactPoint ;
    schema:rangeIncludes schema:Text .

schema:contributor a rdf:Property ;
    rdfs:label "contributor"@en,
        "contributeur"@fr,
        "bijdrager"@nl ;
    rdfs:domain schema:CreativeWork ;
    rdfs:isDefinedBy schema: ;
    rdfs:range [ owl:unionOf ( schema:Person org:Organization schema:Role ) ] ;
    owl:equivalentProperty dct:contributor ;
    skos:definition "A secondary contributor to the CreativeWork or Event."@en,
        "Un contributeur secondaire à la CreativeWork ou à le Event."@fr,
        "Een tweede bijdrager aan het CreativeWork of Event."@nl .

schema:copyrightHolder a rdf:Property ;
    rdfs:label "copyright holder"@en,
        "titulaire du droit d'auteur"@fr,
        "auteursrechthebbende"@nl ;
    rdfs:domain schema:CreativeWork ;
    rdfs:isDefinedBy schema: ;
    rdfs:range [ owl:unionOf ( schema:Person org:Organization schema:Role ) ] ;
    owl:equivalentProperty dct:rightsHolder ;
    skos:definition "The party holding the legal copyright to the CreativeWork."@en,
        "La partie qui détient le droit d'auteur légal de l'œuvre créative (CreativeWork)."@fr,
        "De partij die de auteursrechten heeft op het CreativeWork."@nl .

schema:copyrightNotice a rdf:Property ;
    rdfs:label "copyright notice"@en,
        "avis de droit d'auteur"@fr,
        "auteursrechtvermelding"@nl ;
    rdfs:domain schema:CreativeWork ;
    rdfs:isDefinedBy schema: ;
    rdfs:range xsd:string ;
    owl:equivalentProperty dct:rights ;
    skos:definition "Text of a notice appropriate for describing the copyright aspects of this Creative Work, ideally indicating the owner of the copyright for the Work."@en,
        "Texte d'une notice appropriée pour décrire les aspects du droit d'auteur de cette CreativeWork, indiquant idéalement le propriétaire du droit d'auteur de l'oeuvre."@fr,
        "Tekst van een mededeling die geschikt is om de auteursrechtelijke aspecten van dit CreativeWork te beschrijven, idealiter met vermelding van de auteursrechthebbende van het werk."@nl .

schema:copyrightYear a rdf:Property ;
    rdfs:label "copyright year"@en,
        "année des droits d'auteur"@fr,
        "auteursrechtjaar"@nl ;
    rdfs:domain schema:CreativeWork ;
    rdfs:isDefinedBy schema: ;
    owl:equivalentProperty dct:dateCopyrighted ;
    skos:definition "The year during which the claimed copyright for the CreativeWork was first asserted."@en,
        "L'année durant laquelle le droit d'auteur revendiqué pour l'œuvre créative a été revendiqué pour la première fois."@fr,
        "Het jaar waarin het auteursrecht voor het CreativeWork voor het eerst gold/geldend gemaakt werd."@nl .

schema:creator a rdf:Property ;
    rdfs:label "creator"@en,
        "créateur"@fr,
        "maker"@nl ;
    rdfs:domain schema:CreativeWork ;
    rdfs:isDefinedBy schema: ;
    rdfs:range [ owl:unionOf ( schema:Person org:Organization schema:Role ) ] ;
    owl:equivalentProperty dct:creator ;
    skos:definition "The creator/author of this CreativeWork."@en,
        "Le créateur / auteur de ce travail créatif."@fr,
        "De maker/auteur van dit creatief werk."@nl .

schema:creditText a rdf:Property ;
    rdfs:label "credit text"@en,
        "texte du crédit"@fr,
        "credittekst"@nl ;
    rdfs:domain schema:CreativeWork ;
    rdfs:isDefinedBy schema: ;
    rdfs:range xsd:string ;
    skos:definition "Text that can be used to credit person(s) and/or organization(s) associated with a published Creative Work."@en,
        "Texte qui peut être utilisé pour créditer la ou les personne(s) et/ou organisation(s) associée(s) à une oeuvre créative (CreativeWork) publiée."@fr,
        "Tekst die gebruikt kan worden om personen en/of organisaties aan te geven die met een gepubliceerd CreativeWork zijn verbonden."@nl .

schema:dateCreated a rdf:Property ;
    rdfs:label "date created"@en,
        "date de création"@fr,
        "creatiedatum"@nl ;
    rdfs:domain schema:CreativeWork ;
    rdfs:isDefinedBy schema: ;
    owl:equivalentProperty dct:created ;
    skos:definition "The date on which the CreativeWork was created."@en,
        "La date à laquelle le CreativeWork a été créé."@fr,
        "De datum waarin het CreativeWork werd gemaakt."@nl .

schema:dateDeleted a rdf:Property ;
    rdfs:label "date deleted" ;
    rdfs:domain schema:DataFeedItem ;
    rdfs:isDefinedBy schema: ;
    rdfs:range xsd:dateTime ;
    skos:definition "The datetime the item was removed from the DataFeed."@en,
        "De DateTime Het item is verwijderd uit de DataFeed."@fr,
        "L'élément DateTime a été supprimé du DataFeed."@nl .

schema:dateModified a rdf:Property ;
    rdfs:label "date modified" ;
    rdfs:domain schema:CreativeWork,
        schema:DataFeedItem ;
    rdfs:isDefinedBy schema: ;
    rdfs:range xsd:dateTime ;
    skos:definition "The date on which the CreativeWork was most recently modified or when the item's entry was modified within a DataFeed."@en,
        "La date à laquelle le Creativework a été récemment modifié ou lorsque l'entrée de l'élément a été modifiée dans une DataFeed."@fr,
        "De datum waarop het creatieve werk het meest recent werd gewijzigd of wanneer de invoer van het item binnen een DataFeed werd gewijzigd."@nl .

schema:datePublished a rdf:Property ;
    rdfs:label "date published"@en,
        "date de publication"@fr,
        "publicatiedatum"@nl ;
    rdfs:domain schema:CreativeWork ;
    rdfs:isDefinedBy schema: ;
    owl:equivalentProperty dct:issued ;
    skos:definition "Date of first broadcast/publication."@en,
        "La date de la première diffusion ou publication."@fr,
        "De datum waarop de eerste uitzending/publicatie plaatsvond."@nl .

schema:deathDate a rdf:Property ;
    rdfs:label "death date"@en,
        "date de décès"@fr,
        "sterfdatum"@nl ;
    rdfs:domain schema:Person ;
    rdfs:isDefinedBy schema: ;
    rdfs:range xsd:date ;
    skos:definition "Date of death."@en,
        "Date de décès."@fr,
        "Datum van overlijden."@nl .

schema:depth a rdf:Property ;
    rdfs:label "depth"@en,
        "profondeur"@fr,
        "diepte"@nl ;
    rdfs:domain schema:CreativeWork ;
    rdfs:isDefinedBy schema: ;
    rdfs:range schema:QuantitativeValue ;
    skos:definition "The depth of the item."@en,
        "La profondeur de l'objet."@fr,
        "De diepte van het item."@nl .

schema:description a rdf:Property ;
    rdfs:label "description"@en,
        "description"@fr,
        "beschrijving"@nl ;
    rdfs:domain schema:Thing ;
    rdfs:isDefinedBy schema: ;
    rdfs:range xsd:string ;
    owl:equivalentProperty dct:description ;
    skos:definition "A description of the item."@en,
        "Une description de l'objet."@fr,
        "Een beschrijving van het item."@nl .

schema:duration a rdf:Property ;
    rdfs:label "duration"@en,
        "durée"@fr,
        "duur"@nl ;
    rdfs:domain schema:CreativeWork ;
    rdfs:isDefinedBy schema: ;
    owl:equivalentProperty dct:extent ;
    skos:definition "The duration of the item (movie, audio recording, event, etc.) in ISO 8601 date format."@en,
        "La durée de l'objet (film, enregistrement audio, événement, etc.) au format de date ISO 8601."@fr,
        "De duur van het item (film, opname audio, evenement, enz.) in ISO 8601 datumformaat."@nl .

schema:email a rdf:Property ;
    rdfs:label "email address"@en,
        "adresse e-mail"@fr,
        "e-mailadres"@nl ;
    rdfs:domain schema:ContactPoint,
        schema:Organization,
        schema:Person ;
    rdfs:isDefinedBy schema: ;
    rdfs:range xsd:string ;
    skos:definition "Email address."@en,
        "Adresse e-mail."@fr,
        "E-mailadres."@nl .

schema:endDate a rdf:Property ;
    rdfs:label "end date"@en,
        "date de fin"@fr,
        "einddatum"@nl ;
    rdfs:isDefinedBy schema: ;
    skos:definition "The end date and time of the item (in [ISO 8601 date format](http://en.wikipedia.org/wiki/ISO_8601))."@en,
        "La date de fin et l'heure de l'article (en [ISO 8601 date format](http://en.wikipedia.org/wiki/ISO_8601))."@fr,
        "De einddatum en tijd van het item (in [ISO 8601 date format](http://en.wikipedia.org/wiki/ISO_8601))."@nl ;
    schema:domainIncludes schema:CreativeWorkSeason,
        schema:CreativeWorkSeries,
        schema:DatedMoneySpecification,
        schema:Event,
        schema:MerchantReturnPolicySeasonalOverride,
        schema:Role ;
    schema:rangeIncludes schema:Date,
        schema:DateTime .

schema:endTime a rdf:Property ;
    rdfs:label "endTime"@en,
        "heure de fin"@fr,
        "eindtijd"@nl ;
    rdfs:isDefinedBy schema: ;
    skos:definition """
    The endTime of something. For a reserved event or service (e.g. FoodEstablishmentReservation), the time that it is expected to end. For actions that span a period of time, when the action was performed. E.g. John wrote a book from January to *December*. For media, including audio and video, it's the time offset of the end of a clip within a larger file.
    Note that Event uses startDate/endDate instead of startTime/endTime, even when describing dates with times. This situation may be clarified in future revisions."""@en,
        "La fin de quelque chose.Pour un événement ou un service réservé (par exemple.Pour les actions qui s'étendent sur un certain temps, lorsque l'action a été effectuée.Par exemple.John a écrit un livre de janvier à * décembre *.Pour les médias, y compris l'audio et la vidéo, c'est le décalage de temps de la fin d'un clip dans un fichier plus grand."@fr,
        "De eindtijd van iets. Voor een gereserveerd evenement of service (bijvoorbeeld FoodestablishmentReservation), de tijd dat het naar verwachting zal eindigen. Voor acties die een periode van tijd omvatten, wanneer de actie werd uitgevoerd. Bijv.John schreef een boek van januari tot *december*.Voor media, inclusief audio en video, is dit de tijdoffset van het einde van een clip binnen een groter bestand. "@nl .

schema:episodeNumber a rdf:Property ;
    rdfs:label "episode number"@en,
        "numéro d'épisode"@fr,
        "afleveringnummer"@nl ;
    rdfs:domain schema:Episode ;
    rdfs:isDefinedBy schema: ;
    skos:definition "Position of the episode within an ordered group of episodes."@en,
        "Position de l'épisode dans un groupe d'épisodes ordonnés."@fr,
        "De positie van de aflevering binnen een geordende groep van afleveringen."@nl .

schema:familyName a rdf:Property ;
    rdfs:label "family name"@en,
        "nom de famille"@fr,
        "familienaam"@nl ;
    rdfs:domain schema:Person ;
    rdfs:isDefinedBy schema: ;
    rdfs:range xsd:string ;
    skos:definition "Family name. In the U.S., the last name of a Person."@en,
        "Nom de famille. Aux États-Unis, le dernier nom d'une Personne."@fr,
        "Familienaam. In de V.S., de achternaam van een Persoon."@nl .

schema:genre a rdf:Property ;
    rdfs:label "genre"@en,
        "genre"@fr,
        "genre"@nl ;
    rdfs:domain schema:CreativeWork ;
    rdfs:isDefinedBy schema: ;
    rdfs:range xsd:string ;
    skos:definition "Genre of the creative work, broadcast channel or group."@en,
        "Genre de l'œuvre créative (CreativeWork), de la chaîne de télévision/diffusion ou du groupe."@fr,
        "Genre van het CreativeWork, uitzendkanaal of groep."@nl .

schema:givenName a rdf:Property ;
    rdfs:label "given name"@en,
        "prénom"@fr,
        "voornaam"@nl ;
    rdfs:domain schema:Person ;
    rdfs:isDefinedBy schema: ;
    skos:definition "Given name. In the U.S., the first name of a Person."@en,
        "Prénom. Aux États-Unis, le premier nom d'une Personne."@fr,
        "Voornaam. In de V.S., de eerste naam van een Persoon."@nl .

schema:height a rdf:Property ;
    rdfs:label "height"@en,
        "hauteur"@fr,
        "hoogte"@nl ;
    rdfs:domain schema:CreativeWork ;
    rdfs:isDefinedBy schema: ;
    rdfs:range schema:QuantitativeValue ;
    skos:definition "The height of the item."@en,
        "La hauteur de l'objet."@fr,
        "De hoogte van het item."@nl .

schema:inLanguage a rdf:Property ;
    rdfs:label "in language"@en,
        "en langue"@fr,
        "in taal"@nl ;
    rdfs:domain schema:CreativeWork ;
    rdfs:isDefinedBy schema: ;
    rdfs:range xsd:string ;
    skos:definition "The language of the content or performance or used in an action. Please use one of the language codes from the IETF BCP 47 standard."@en,
        "La langue du contenu ou de la performance ou utilisée dans une action. Veuillez utiliser l'un des codes de langue de la norme IETF BCP 47."@fr,
        "De taal van de inhoud of de uitvoering of gebruikt in een actie. Gebruik bij voorkeur één van de taalcodes uit de IETF BCP 47 standaard."@nl .

schema:isPartOf a rdf:Property ;
    rdfs:label "is part of"@en,
        "fait partie de"@fr,
        "is onderdeel van"@nl ;
    rdfs:domain schema:CreativeWork ;
    rdfs:isDefinedBy schema: ;
    skos:definition "Indicates an item or CreativeWork that this item, or CreativeWork (in some sense), is part of."@en,
        "Indique un élément ou un CreativeWork qui fait partie de cet élément, ou de ce CreativeWork (dans un certain sens)."@fr,
        "Geeft een item of CreativeWork aan waarvan dit item, of CreativeWork (in een bepaald opzicht), een onderdeel is."@nl .

schema:keywords a rdf:Property ;
    rdfs:label "keywords"@en,
        "mots-clés"@fr,
        "trefwoorden"@nl ;
    rdfs:domain schema:CreativeWork ;
    rdfs:isDefinedBy schema: ;
    rdfs:range xsd:string ;
    owl:equivalentProperty dct:subject ;
    skos:definition "Keywords or tags used to describe some item. Multiple textual entries in a keywords list are typically delimited by commas, or by repeating the property."@en,
        "Mots-clés ou balises utilisés pour décrire un élément. Des entrées textuelles multiples dans une liste de mots-clés sont généralement séparées par des virgules, ou par répétition de la propriété (Property)."@fr,
        "Trefwoorden of tags die gebruikt worden om een item te beschrijven. Meerdere tekstuele elementen in een trefwoordenlijst worden meestal gescheiden door komma's, of door het herhaling van de eigenschap (Property)."@nl .

schema:license a rdf:Property ;
    rdfs:label "license"@en,
        "licence"@fr,
        "licentie"@nl ;
    rdfs:domain schema:CreativeWork ;
    rdfs:isDefinedBy schema: ;
    rdfs:range [ owl:unionOf ( schema:Thing skos:Concept ) ] ;
    owl:equivalentProperty dct:accessRights ;
    skos:definition "A license document that applies to this content, typically indicated by URL."@en,
        "Un document de licence qui s'applique à ce contenu, généralement indiqué par URL."@fr,
        "Een licentiedocument dat geldig is voor deze inhoud, meestal gekenmerkt door een URL."@nl .

schema:maintainer a rdf:Property ;
    rdfs:label "maintainer"@en,
        "mainteneur/responsable"@fr,
        "beheerder"@nl ;
    rdfs:isDefinedBy schema: ;
    skos:definition "A maintainer is a Person or Organization that manages contributions to, and/or publication of, some (typically complex) artifact."@en,
        "Un mainteneur est une personne ou une organisation qui gère les contributions à, et/ou la publication de, un (généralement complexe) artefact."@fr,
        "Een beheerder is een Persoon of Organisatie die bijdragen beheert aan, en/of publicatie van, een (meestal complex) artefact."@nl .

schema:mentions a rdf:Property ;
    rdfs:label "mentions"@en,
        "mentionne"@fr,
        "vermeldt"@nl ;
    rdfs:isDefinedBy schema: ;
    skos:definition "Indicates that the CreativeWork contains a reference to, but is not necessarily about a concept."@en,
        "Indique que le Creative Work contient une référence à, mais ne concerne pas nécessairement un concept."@fr,
        "Geeft aan dat het Creative Work een verwijzing bevat naar, maar niet noodzakelijkerwijs over een concept."@nl .

schema:postOfficeBoxNumber a rdf:Property ;
    rdfs:label "postOfficeBoxNumber"@en,
        "numéroBoîtePostale"@fr,
        "postbusnummer"@nl ;
    rdfs:isDefinedBy schema: ;
    skos:definition "The post office box number for PO box addresses."@en,
        "Le numéro de la boîte postale pour les adresses de type boîte postale."@fr,
        "Het postbusnummer voor postbusadressen."@nl ;
    schema:domainIncludes schema:PostalAddress ;
    schema:rangeIncludes schema:Text .

schema:postalCode a rdf:Property ;
    rdfs:label "postalCode"@en,
        "codePostale"@fr,
        "postCode"@nl ;
    rdfs:isDefinedBy schema: ;
    skos:definition "The postal code. For example, 94043."@en,
        "Le code postale."@fr,
        "De postcode."@nl ;
    schema:domainIncludes schema:DefinedRegion,
        schema:GeoCoordinates,
        schema:GeoShape,
        schema:PostalAddress ;
    schema:rangeIncludes schema:Text .

schema:publisher a rdf:Property ;
    rdfs:label "publisher"@en,
        "éditeur"@fr,
        "uitgever"@nl ;
    rdfs:domain schema:CreativeWork ;
    rdfs:isDefinedBy schema: ;
    owl:equivalentProperty dct:publisher ;
    skos:definition "The publisher of the creative work."@en,
        "L'éditeur du travail créatif."@fr,
        "De uitgever van het creatief werk."@nl .

schema:roleName a rdf:Property ;
    rdfs:label "role name"@en,
        "nom du rôle"@fr,
        "rolnaam"@nl ;
    rdfs:domain schema:PerformanceRole ;
    rdfs:isDefinedBy schema: ;
    rdfs:range skos:Concept ;
    skos:definition "A role played, performed or filled by a person or organization."@en,
        "Un rôle joué ou rempli par une personne ou une organisation."@fr,
        "Een rol gespeeld of vertolkt door een persoon of organisatie."@nl .

schema:seasonNumber a rdf:Property ;
    rdfs:label "season number"@en,
        "numéro de saison"@fr,
        "seizoen nummer"@nl ;
    rdfs:domain schema:CreativeWorkSeason ;
    rdfs:isDefinedBy schema: ;
    skos:definition "Position of the season within an ordered group of seasons."@en,
        "Position de la saison dans un groupe ordonné de saisons."@fr,
        "Positie van het seizoen in een geordende groep van seizoenen."@nl .

schema:spatial a rdf:Property ;
    rdfs:label "spatial coverage"@en,
        "couverture spatiale/géographique"@fr,
        "geografische dekking; aflijning binnen de ruimte"@nl ;
    rdfs:domain schema:CreativeWork ;
    rdfs:isDefinedBy schema: ;
    rdfs:range schema:Place ;
    owl:equivalentProperty dct:spatial ;
    skos:definition "The spatialCoverage of a CreativeWork indicates the place(s) which are the focus of the content."@en,
        "La couverture spatiale d'un travail créatif (CreativeWork) indique où se situe le contenu."@fr,
        "De geografische dekking van een CreativeWork geeft aan waar de focus van de inhoud ligt."@nl .

schema:startDate a rdf:Property ;
    rdfs:label "start date"@en,
        "date de début"@fr,
        "begindatum"@nl ;
    rdfs:isDefinedBy schema: ;
    skos:definition "The start date and time of the item (in [ISO 8601 date format](http://en.wikipedia.org/wiki/ISO_8601))."@en,
        "La date et l'heure de la date de la statistique par l'item (en [ISO 8601 date format](http://en.wikipedia.org/wiki/ISO_8601))"@fr,
        "De startdatum en tijd van de status van het item (in [ISO 8601 date format](http://en.wikipedia.org/wiki/ISO_8601))"@nl ;
    schema:domainIncludes schema:CreativeWorkSeason,
        schema:CreativeWorkSeries,
        schema:DatedMoneySpecification,
        schema:Event,
        schema:MerchantReturnPolicySeasonalOverride,
        schema:Role ;
    schema:rangeIncludes schema:Date,
        schema:DateTime .

schema:startTime a rdf:Property ;
    rdfs:label "startTime"@en,
        "heure de départ"@fr,
        "starttijd"@nl ;
    rdfs:isDefinedBy schema: ;
    skos:definition "The startTime of something. For a reserved event or service (e.g. FoodEstablishmentReservation), the time that it is expected to start. For actions that span a period of time, when the action was performed. E.g. John wrote a book from *January* to December. For media, including audio and video, it's the time offset of the start of a clip within a larger file.\\n\\nNote that Event uses startDate/endDate instead of startTime/endTime, even when describing dates with times. This situation may be clarified in future revisions."@en,
        "Le début du temps de quelque chose. Pour un événement ou un service réservé (par exemple.Pour les actions qui s'étendent sur un certain temps, lorsque l'action a été effectuée.Par exemple. John a écrit un livre de * janvier * à décembre.Pour les médias, y compris l'audio et la vidéo, c'est le décalage de temps du début d'un clip dans un fichier plus grand. \\ n \\ nnote que l'événement utilise StartDate / EndDate au lieu de démarrage / fin de fin, même lors de la description des dates avec les temps. Cette situation peut être clarifiée dans les révisions futures."@fr,
        "De starttijd van iets. Voor een gereserveerd evenement of service (bijvoorbeeld FoodestablishmentReservation), de tijd die naar verwachting zal beginnen.Voor acties die een periode van tijd omvatten, wanneer de actie werd uitgevoerd.Bijv.John schreef een boek van * januari * tot december.Voor media, inclusief audio en video, is dit de tijdoffset van het begin van een clip binnen een groter bestand. \\ n \\ nnote die gebeurtenis gebruikt startdate/enddate in plaats van starttijd/eindtijd, zelfs bij het beschrijven van datums met tijden. Deze situatie kan worden verduidelijkt in toekomstige herzieningen."@nl .

schema:streetAddress a rdf:Property ;
    rdfs:label "streetAddress"@en,
        "adresseDeRue"@fr,
        "straatAdres"@nl ;
    rdfs:isDefinedBy schema: ;
    skos:definition "The street address. For example, 1600 Amphitheatre Pkwy."@en,
        "L'adresse de rue."@fr,
        "Het adres van de straat."@nl ;
    schema:domainIncludes schema:PostalAddress ;
    schema:rangeIncludes schema:Text .

schema:telephone a rdf:Property ;
    rdfs:label "telephone"@en,
        "téléphone"@fr,
        "telefoon"@nl ;
    rdfs:isDefinedBy schema: ;
    skos:definition "The telephone number."@en,
        "Le numéro de téléphone."@fr,
        "Het telefoonnummer."@nl ;
    schema:domainIncludes schema:ContactPoint,
        schema:Organization,
        schema:Person,
        schema:Place ;
    schema:rangeIncludes schema:Text .

schema:temporal a rdf:Property ;
    rdfs:label "temporal coverage"@en,
        "couverture temporelle"@fr,
        "temporele dekking; aflijning binnen de tijd"@nl ;
    rdfs:domain schema:CreativeWork ;
    rdfs:isDefinedBy schema: ;
    rdfs:range xsd:string ;
    owl:equivalentProperty dct:temporal ;
    skos:definition "The temporalCoverage of a CreativeWork indicates the period that the content applies to, i.e. that it describes, either as a `DateTime` or as a textual string indicating a time period in ISO 8601 time interval format."@en,
        "La couverture temporelle d'un travail créatif (CreativeWork) indique la période à laquelle s'applique le contenu, c'est-à-dire qu'il décrit soit par une date et heure (`DateTime`), soit par une série de caractères indiquant une période de temps en format ISO 8601."@fr,
        "De dekking in de tijd van een CreativeWork geeft aan over welke periode de inhoud handelt, bijvoorbeeld als een `xsd:dateTime` of als een tekstuele string die een tijdsinterval in ISO 8601 formaat aanduidt."@nl .

schema:thumbnailUrl a rdf:Property ;
    rdfs:label "thumbnailUrl"@en,
        "URL miniature"@fr,
        "miniatuur-url"@nl ;
    rdfs:isDefinedBy schema: ;
    skos:definition "A thumbnail image relevant to the Thing."@en,
        "Une image miniature pertinente pour la chose."@fr,
        "Een miniatuurafbeelding relevant voor het ding."@nl .

schema:transcript a rdf:Property ;
    rdfs:label "transcript"@en,
        "transcription"@fr,
        "transcriptie"@nl ;
    rdfs:domain schema:CreativeWork ;
    rdfs:isDefinedBy schema: ;
    rdfs:range xsd:string ;
    skos:definition "If this MediaObject is an AudioObject or VideoObject, the transcript of that object."@en,
        "Si cet MediaObject est un AudioObject ou VideoObject, la transcription de cet objet."@fr,
        "Als dit MediaObject een AudioObject of VideoObject is, de transcriptie van dat object."@nl .

schema:unitCode a rdf:Property ;
    rdfs:label "unit code"@en,
        "code d'unité"@fr,
        "eenheid code"@nl ;
    rdfs:domain schema:QuantitativeValue ;
    rdfs:isDefinedBy schema: ;
    rdfs:range xsd:string ;
    skos:definition "The unit of measurement given using the UN/CEFACT Common Code (3 characters)."@en,
        "L'unité de mesure donnée en utilisant le code commun UN/CEFACT (3 caractères)."@fr,
        "De eenheid van de meting, gegeven met behulp van de UN/CEFACT Common Code (3 karakters)."@nl .

schema:unitText a rdf:Property ;
    rdfs:label "unit text"@en,
        "texte d'unité"@fr,
        "eenheid tekst"@nl ;
    rdfs:domain schema:QuantitativeValue ;
    rdfs:isDefinedBy schema: ;
    rdfs:range xsd:string ;
    skos:definition "A string or text indicating the unit of measurement. Useful if you cannot provide a standard unit code for `schema:unitCode`."@en,
        "Une chaîne de caractères ou un texte indiquant l'unité de mesure. Utile si vous ne pouvez pas fournir de code d'unité standard pour `schema:unitCode`."@fr,
        "Een string of tekst die de eenheid van de meting aangeeft. Handig als je geen standaard eenheidcode kunt geven voor `schema:unitCode`."@nl .

schema:value a rdf:Property ;
    rdfs:label "value"@en,
        "valeur"@fr,
        "waarde"@nl ;
    rdfs:domain schema:QuantitativeValue ;
    rdfs:isDefinedBy schema: ;
    rdfs:range xsd:float ;
    skos:definition "The value of the quantitative value."@en,
        "La valeur de la valeur quantitative."@fr,
        "De waarde van de kwantitatieve waarde."@nl .

schema:width a rdf:Property ;
    rdfs:label "width"@en,
        "largeur"@fr,
        "breedte"@nl ;
    rdfs:domain schema:CreativeWork ;
    rdfs:isDefinedBy schema: ;
    rdfs:range schema:QuantitativeValue ;
    skos:definition "The width of the item."@en,
        "La largeur de l'élément."@fr,
        "De breedte van het item."@nl .

evtObjRole:out a owl:ObjectProperty ;
    rdfs:label "outcome"@en,
        "résultat"@fr,
        "uitkomst"@nl ;
    rdfs:domain premis:Event ;
    rdfs:isDefinedBy evtObjRole: ;
    rdfs:range premis:Object ;
    rdfs:subPropertyOf prov:generated ;
    skos:definition "The object in relation to the described event is the outcome of that event."@en,
        "L'objet dans la relation à l'événement (Event) décrit est le résultat de cet événement (Event)."@fr,
        "Het object in relatie tot de beschreven gebeurtenis (Event) is het resultaat van die gebeurtenis (Event)."@nl .

evtObjRole:sou a owl:ObjectProperty ;
    rdfs:label "source"@en,
        "source"@fr,
        "bron"@nl ;
    rdfs:domain premis:Event ;
    rdfs:isDefinedBy evtObjRole: ;
    rdfs:range premis:Object ;
    rdfs:subPropertyOf prov:used ;
    skos:definition "The object in relation to the described event that existed prior to that event and was used by it."@en,
        "L'objet dans la relation à l'événement (Event) décrit et qui existait avant cet événement (Event) et qui a été utilisé par celui-ci."@fr,
        "Het object in relatie tot de beschreven gebeurtenis (Event) dat bestond voor die gebeurtenis (Event) en die erdoor gebruikt werd."@nl .

dct:medium a rdf:Property ;
    rdfs:label "medium"@en,
        "médium"@fr,
        "medium"@nl ;
    rdfs:isDefinedBy dct: ;
    rdfs:range xsd:string ;
    skos:definition "The material or physical carrier of the resource"@en,
        "Le support matériel ou physique de la ressource"@fr,
        "Het materiaal of fysieke drager van de bron"@nl .

dct:rights a rdf:Property ;
    rdfs:label "Rights"@en,
        "Droits"@fr,
        "Rechten"@nl ;
    dct:description "Typically, rights information includes a statement about various property rights associated with the resource, including intellectual property rights.  Recommended practice is to refer to a rights statement with a URI.  If this is not possible or feasible, a literal value (name, label, or short text) may be provided."@en,
        "En règle générale, les informations sur les droits comprennent une déclaration sur les différents droits de propriété associés à la ressource, y compris les droits de propriété intellectuelle.La pratique recommandée est de se référer à une déclaration de droits avec un URI.Si cela n'est pas possible ou possible, une valeur littérale (nom, étiquette ou texte court) peut être fourni."@fr,
        "Doorgaans bevat rechteninformatie een verklaring over verschillende eigendomsrechten die verband houden met de bron, inclusief intellectuele eigendomsrechten.Aanbevolen praktijk is om te verwijzen naar een rechtenverklaring met een URI.Als dit niet mogelijk of haalbaar is, kan een letterlijke waarde (naam, label of korte tekst) worden verstrekt."@nl ;
    dct:issued "2008-01-14"^^xsd:date ;
    rdfs:isDefinedBy dct: ;
    rdfs:range xsd:string ;
    rdfs:subPropertyOf <http://purl.org/dc/elements/1.1/rights> ;
    skos:definition "Information about rights held in and over the resource."@en,
        "Informations sur les droits maintenus dans et au-dessus de la ressource."@fr,
        "Informatie over rechten in en over de bron."@nl .

<http://www.ebu.ch/metadata/ontologies/ebucore/ebucore#isMediaFragmentOf> a rdf:Property ;
    rdfs:label "media fragment source"@en,
        "source du fragment de média (MediaFragment)"@fr,
        "bron van het mediafragment (MediaFragment)"@nl ;
    rdfs:domain <http://www.ebu.ch/metadata/ontologies/ebucore/ebucore#MediaFragment> ;
    rdfs:isDefinedBy <http://www.ebu.ch/metadata/ontologies/ebucore/ebucore#> ;
    rdfs:range <http://www.ebu.ch/metadata/ontologies/ebucore/ebucore#MediaResource> ;
    skos:definition "To identify the Media Resource to which a Media Fragment belongs to."@en,
        "Pour identifier la MediaResource à laquelle appartient un MediaFragment."@fr,
        "Om de MediaResource te identificeren waartoe een MediaFragment behoort."@nl .

premis:identifier a owl:ObjectProperty ;
    rdfs:label "has identifier"@en,
        "a identifiant"@fr,
        "heeft identificatiecode"@nl ;
    rdfs:isDefinedBy premis: ;
    rdfs:range premis:Identifier .

premis:outcome a owl:ObjectProperty ;
    rdfs:label "has outcome"@en,
        "a résultat"@fr,
        "heeft resultaat"@nl ;
    rdfs:domain premis:Event ;
    rdfs:isDefinedBy premis: ;
    rdfs:range premis:OutcomeStatus .

premis:outcomeNote a owl:DatatypeProperty ;
    rdfs:label "has outcome note"@en,
        "a note de résultat"@fr,
        "heeft resultaatnota"@nl ;
    rdfs:domain premis:Event ;
    rdfs:isDefinedBy premis: ;
    rdfs:range rdfs:Literal ;
    rdfs:subPropertyOf premis:note .

<http://www.ontologydesignpatterns.org/cp/owl/sequence.owl#directlyPrecedes> a owl:ObjectProperty ;
    rdfs:label "directly precedes"@en,
        "précède directement"@fr,
        "gaat direct vooraf aan"@nl ;
    rdfs:domain owl:Thing ;
    rdfs:isDefinedBy <http://www.ontologydesignpatterns.org/cp/owl/sequence.owl> ;
    rdfs:range owl:Thing ;
    rdfs:subPropertyOf <http://www.ontologydesignpatterns.org/cp/owl/sequence.owl#precedes> ;
    skos:definition "The intransitive precedes relation. For example, Monday directly precedes Tuesday. Directness of precedence depends on the designer conceptualization."@en,
        "La relation intransitive de 'préceder'. Par exemple, lundi précède directement mardi. Le caractère direct de la précédence dépend de la conceptualisation du concepteur."@fr,
        "De intransitieve 'gaat-vooraf-aan' relatie. Bv. maandag gaat direct vooraf aan dinsdag. De mate van 'direct-vooraf-gaan-aan' hangt af van het ontwerp van de bedenker."@nl .

<http://www.ontologydesignpatterns.org/cp/owl/sequence.owl#precedes> a owl:ObjectProperty,
        owl:TransitiveProperty ;
    rdfs:label "precedes"@en,
        "précède"@fr,
        "gaat vooraf aan"@nl ;
    rdfs:domain owl:Thing ;
    rdfs:isDefinedBy <http://www.ontologydesignpatterns.org/cp/owl/sequence.owl> ;
    rdfs:range owl:Thing ;
    owl:inverseOf <http://www.ontologydesignpatterns.org/cp/owl/sequence.owl#follows> ;
    skos:definition "A relation between entities, expressing a 'sequence' schema. E.g. 'year 1999 precedes 2000', 'deciding what coffee to use' precedes 'preparing coffee', 'World War II follows World War I', 'in the Milan to Rome autoroute, Bologna precedes Florence', etc. It can then be used between tasks, processes, time intervals, spatially locate objects, situations, etc. Subproperties can be defined in order to distinguish the different uses."@en,
        "Une relation entre entités, exprimant une 'séquence'. Par exemple, 'l'année 1999 précède l'année 2000', 'décider quel café à utiliser' précède 'préparer du café', 'sur l'autoroute de Milan à Rome, Bologne précède Florence', etc. Il peut être utilisé avec des tâches, des processus, des intervalles de temps, des objets dans l'espace, des situations, etc. Des sous-propriétés (subproperties) peuvent être définies pour distinguer les différentes utilisations."@fr,
        "Een relatie tussen entiteiten, die een 'sequentie' uitdrukt. Bv. 'het jaar 1999 gaat vooraf aan het jaar 2000', 'beslissen welke koffie te gebruiken' gaat vooraf aan 'koffie klaarmaken', 'op de autoweg van Milaan naar Rome, gaat Bologna vooraf aan Florence', etc. Het kan gebruikt worden bij taken, processen, tijdsintervallen, objecten in de ruimte, situaties, etc. Subeigenschappen (subproperties) kunnen gedefinieerd worden om de verschillende gebruiken te onderscheiden."@nl .

skos:altLabel a rdf:Property,
        owl:AnnotationProperty ;
    rdfs:label "alternative label"@en,
        "label alternatif"@fr,
        "alternatief label"@nl ;
    rdfs:comment "The range of skos:altLabel is the class of RDF plain literals."@en,
        "skos:prefLabel, skos:altLabel and skos:hiddenLabel are pairwise disjoint properties."@en,
        "Le domaine de skos:altLabel est la classe des littéraux RDF."@fr,
        "skos:prefLabel, skos:altLabel et skos:hiddenLabel sont des propriétés disjoints."@fr,
        "Het domein van skos:altLabel is de klasse van RDF literals."@nl,
        "skos:prefLabel, skos:altLabel en skos:hiddenLabel zijn disjuncte eigenschappen."@nl ;
    rdfs:isDefinedBy <http://www.w3.org/2004/02/skos/core> ;
    rdfs:subPropertyOf rdfs:label ;
    skos:definition "An alternative lexical label for a resource."@en,
        "Un label lexical alternatif pour une ressource."@fr,
        "Een alternatief lexicaal label voor een resource."@nl ;
    skos:example "Acronyms, abbreviations, spelling variants, and irregular plural/singular forms may be included among the alternative labels for a concept. Mis-spelled terms are normally included as hidden labels (see skos:hiddenLabel)."@en,
        "Les acronymes, abréviations, variantes orthographiques et formes plurielles/singulières irrégulières peuvent être incluses parmi les labels alternatifs pour un concept. Les termes mal orthographiés sont normalement inclus comme labels cachés (voir skos:hiddenLabel)."@fr,
        "Acroniemen, afkortingen, spellingvarianten en onregelmatige meervoudsvormen/ enkelvoudsvormen kunnen onder de alternatieve labels voor een concept worden opgenomen. Fout gespelde termen worden normaal gesproken opgenomen als verborgen labels (zie skos:hiddenLabel)."@nl .

skos:broadMatch a rdf:Property,
        owl:ObjectProperty ;
    rdfs:label "has broader match"@en,
        "a un match plus large"@fr,
        "heeft bredere overeenkomst"@nl ;
    rdfs:isDefinedBy <http://www.w3.org/2004/02/skos/core> ;
    rdfs:subPropertyOf skos:broader,
        skos:mappingRelation ;
    owl:inverseOf skos:narrowMatch ;
    skos:definition "`skos:broadMatch` is used to state a hierarchical mapping link between two conceptual resources in different concept schemes."@en,
        "`skos:broadMatch` est utilisé pour indiquer un lien de correspondance hiérarchique entre deux ressources conceptuelles dans des schémas de concepts différents."@fr,
        "`skos:broadMatch` wordt gebruikt om een hiërarchische mapping link te geven tussen twee conceptuele resources in verschillende conceptenschema's."@nl .

skos:closeMatch a rdf:Property,
        owl:ObjectProperty,
        owl:SymmetricProperty ;
    rdfs:label "has close match"@en,
        "a un match proche"@fr,
        "heeft nauwe overeenkomst"@nl ;
    rdfs:isDefinedBy <http://www.w3.org/2004/02/skos/core> ;
    rdfs:subPropertyOf skos:mappingRelation ;
    skos:definition "`skos:closeMatch` is used to link two concepts that are sufficiently similar that they can be used interchangeably in some information retrieval applications. In order to avoid the possibility of \"compound errors\" when combining mappings across more than two concept schemes, `skos:closeMatch` is not declared to be a transitive property."@en,
        "`skos:closeMatch` est utilisé pour lier deux concepts qui sont suffisamment similaires pour pouvoir être utilisés de manière interchangeable dans certaines applications de recherche d'information. Afin d'éviter la possibilité d'\"erreurs combinées\" lors de l'utilisation de correspondances entre plus de deux schémas de concepts, `skos:closeMatch` n'est pas déclaré comme une propriété transitive."@fr,
        "`skos:closeMatch` wordt gebruikt om twee concepten te linken die voldoende gelijkwaardig zijn dat ze in sommige informatie-uitwisselingsapplicaties uitwisselbaar kunnen worden gebruikt. Om de mogelijkheid van \"samengestelde fouten\" te vermijden bij het combineren van mappings over meer dan twee conceptenschema's, is `skos:closeMatch` niet gedefinieerd als een transitieve eigenschap."@nl .

skos:hasTopConcept a rdf:Property,
        owl:ObjectProperty ;
    rdfs:label "has top concept"@en,
        "a un concept supérieur"@fr,
        "heeft bovenste concept"@nl ;
    rdfs:domain skos:ConceptScheme ;
    rdfs:isDefinedBy <http://www.w3.org/2004/02/skos/core> ;
    rdfs:range skos:Concept ;
    owl:inverseOf skos:topConceptOf ;
    skos:definition "Relates, by convention, a concept scheme to a concept which is topmost in the broader/narrower concept hierarchies for that scheme, providing an entry point to these hierarchies."@en,
        "Relie, par convention, un schéma de concepts à un concept qui est le plus haut dans les hiérarchies de concepts plus large/plus restreint pour ce schéma, fournissant un point d'entrée pour ces hiérarchies."@fr,
        "Verbindt, bij conventie, een conceptenschema met een concept dat bovenaan staat in de bredere/nauwere concept hiërarchieën voor dat schema, en die een ingang vormt voor deze hiërarchieën."@nl .

skos:hiddenLabel a rdf:Property,
        owl:AnnotationProperty ;
    rdfs:label "hidden label"@en,
        "étiquette cachée"@fr,
        "verborgen label"@nl ;
    rdfs:comment "The range of skos:hiddenLabel is the class of RDF plain literals."@en,
        "skos:prefLabel, skos:altLabel and skos:hiddenLabel are pairwise disjoint properties."@en,
        "The range of skos:hiddenLabel is the class of RDF plain literals."@fr,
        "skos:prefLabel, skos:altLabel et skos:hiddenLabel sont des propriétés disjoints."@fr,
        "The range of skos:hiddenLabel is the class of RDF plain literals."@nl,
        "skos:prefLabel, skos:altLabel en skos:hiddenLabel zijn disjuncte eigenschappen."@nl ;
    rdfs:isDefinedBy <http://www.w3.org/2004/02/skos/core> ;
    rdfs:subPropertyOf rdfs:label ;
    skos:definition "A lexical label for a resource that should be hidden when generating visual displays of the resource, but should still be accessible to free text search operations."@en,
        "Une étiquette lexicale pour une ressource qui doit être cachée lors de la génération d'affichages visuels de la ressource, mais qui doit toujours être accessible aux opérations de recherche de texte libre."@fr,
        "Een lexicaal label voor een resource dat verborgen moet worden bij het genereren van visuele weergaven van de resource, maar dat nog steeds toegankelijk moet zijn voor vrije tekst zoekoperaties."@nl .

skos:inScheme a rdf:Property,
        owl:ObjectProperty ;
    rdfs:label "is in scheme"@en,
        "est dans le schéma"@fr,
        "is in schema"@nl ;
    rdfs:isDefinedBy <http://www.w3.org/2004/02/skos/core> ;
    rdfs:range skos:ConceptScheme ;
    skos:definition "Relates a resource (for example a concept) to a concept scheme in which it is included."@en,
        "Relie une ressource (par exemple un concept) à un schéma de concepts dans lequel elle est incluse."@fr,
        "Verbindt een resource (bijvoorbeeld een concept) met een conceptenschema waarin het is opgenomen."@nl ;
    skos:scopeNote "A concept may be a member of more than one concept scheme."@en,
        "Un concept peut être membre de plus d'un schéma de concepts."@fr,
        "Een concept kan lid zijn van meer dan één conceptenschema."@nl .

skos:narrowMatch a rdf:Property,
        owl:ObjectProperty ;
    rdfs:label "has narrower match"@en,
        "a un match plus restreint"@fr,
        "heeft nauwere overeenkomst"@nl ;
    rdfs:isDefinedBy <http://www.w3.org/2004/02/skos/core> ;
    rdfs:subPropertyOf skos:mappingRelation,
        skos:narrower ;
    owl:inverseOf skos:broadMatch ;
    skos:definition "`skos:narrowMatch` is used to state a hierarchical mapping link between two conceptual resources in different concept schemes."@en,
        "`skos:narrowMatch` est utilisé pour indiquer un lien de correspondance hiérarchique entre deux ressources conceptuelles dans des schémas de concepts différents."@fr,
        "`skos:narrowMatch` wordt gebruikt om een hiërarchische mapping link te geven tussen twee conceptuele resources in verschillende conceptenschema's."@nl .

skos:notation a rdf:Property,
        owl:DatatypeProperty ;
    rdfs:label "notation"@en,
        "notation"@fr,
        "notatie"@nl ;
    rdfs:isDefinedBy <http://www.w3.org/2004/02/skos/core> ;
    skos:definition "A notation, also known as classification code, is a string of characters such as \"T58.5\" or \"303.4833\" used to uniquely identify a concept within the scope of a given concept scheme."@en,
        "Une notation, également connue sous le nom de code de classification, est une chaîne de caractères telle que «T58.5» ou «303.4833» utilisée pour identifier de manière unique un concept dans le cadre d'un schéma de concepts donné."@fr,
        "Een notatie, ook wel classificatiecode genoemd, is een reeks tekens zoals \"T58.5\" of \"303.4833\" die gebruikt wordt om een concept uniek te identificeren binnen de context van een gegeven conceptenschema."@nl ;
    skos:scopeNote "By convention, skos:notation is used with a typed literal in the object position of the triple."@en,
        "Par convention, skos:notation est utilisé avec un littéral typé dans la position objet du triplet."@fr,
        "Volgens conventie wordt skos:notation gebruikt met een typed literal in de objectpositie van de triple."@nl .

skos:prefLabel a rdf:Property,
        owl:AnnotationProperty ;
    rdfs:label "preferred label"@en,
        "étiquette préférée"@fr,
        "voorkeurslabel"@nl ;
    rdfs:comment "A resource has no more than one value of skos:prefLabel per language tag, and no more than one value of skos:prefLabel without language tag."@en,
        "The range of skos:prefLabel is the class of RDF plain literals."@en,
        "skos:prefLabel, skos:altLabel and skos:hiddenLabel are pairwise disjoint properties."@en,
        "La portée de skos:prefLabel est la classe des littéraux RDF."@fr,
        "Une ressource n'a pas plus d'une valeur de skos:prefLabel par balise de langue, et pas plus d'une valeur de skos:prefLabel sans balise de langue."@fr,
        "skos:prefLabel, skos:altLabel et skos:hiddenLabel sont des propriétés disjoints par paires."@fr,
        "De range van skos:prefLabel is de klasse van RDF plain literals."@nl,
        "Een resource heeft niet meer dan één waarde van skos:prefLabel per taaltag, en niet meer dan één waarde van skos:prefLabel zonder taaltag."@nl,
        "skos:prefLabel, skos:altLabel en skos:hiddenLabel zijn onderling disjuncte eigenschappen."@nl ;
    rdfs:isDefinedBy <http://www.w3.org/2004/02/skos/core> ;
    rdfs:subPropertyOf rdfs:label ;
    skos:definition "The preferred lexical label for a resource, in a given language."@en,
        "L'étiquette lexical préférée pour une ressource, dans une langue donnée."@fr,
        "Het verkozen lexicale label voor een resource, in een gegeven taal."@nl .

skos:topConceptOf a rdf:Property,
        owl:ObjectProperty ;
    rdfs:label "is top concept in scheme"@en,
        "est un concept supérieur dans le schéma"@fr,
        "is bovenste concept in schema"@nl ;
    rdfs:domain skos:Concept ;
    rdfs:isDefinedBy <http://www.w3.org/2004/02/skos/core> ;
    rdfs:range skos:ConceptScheme ;
    rdfs:subPropertyOf skos:inScheme ;
    owl:inverseOf skos:hasTopConcept ;
    skos:definition "Relates a concept to the concept scheme that it is a top level concept of."@en,
        "Associe un concept au schéma de concepts dont il s'agit d'un concept de niveau supérieur."@fr,
        "Verbindt een concept met het conceptenschema waarvan het een bovenste niveau concept (top concept) is."@nl .

<http://www.w3.org/2008/05/skos-xl#literalForm> a rdf:Property,
        owl:DatatypeProperty ;
    rdfs:label "literal form"@en,
        "forme littérale"@fr,
        "letterlijke vorm"@nl ;
    rdfs:comment "If two instances of the class skosxl:Label have the same literal form, they are not necessarily the same resource."@en,
        "The range of skosxl:literalForm is the class of RDF plain literals."@en ;
    rdfs:domain <http://www.w3.org/2008/05/skos-xl#Label> ;
    rdfs:isDefinedBy <http://www.w3.org/2008/05/skos-xl> ;
    skos:definition "The property skosxl:literalForm is used to give the literal form of an skosxl:Label."@en,
        "La propriété skosxl:literalForm est utilisée pour donner la forme littérale d'une skosxl:Label."@fr,
        "De eigenschap skosxl:literalForm wordt gebruikt om de letterlijke vorm van een skosxl:Label te geven."@nl .

org:hasPost a rdf:Property,
        owl:ObjectProperty ;
    rdfs:label "post"@en,
        "possède un poste"@fr,
        "positie"@nl ;
    rdfs:domain org:Organization ;
    rdfs:isDefinedBy <http://www.w3.org/ns/org> ;
    rdfs:range org:Post ;
    owl:inverseOf org:postIn ;
    skos:definition "Indicates a Post which exists within the Organization."@en,
        "Indique un Poste qui existe dans l'Organisation."@fr,
        "Duidt een positie aan die bestaat binnen de organisatie."@nl .

org:hasSite a rdf:Property,
        owl:ObjectProperty ;
    rdfs:label "has site"@en,
        "a un site"@fr,
        "heeft een zetel"@nl ;
    rdfs:domain org:Organization ;
    rdfs:isDefinedBy <http://www.w3.org/ns/org> ;
    rdfs:range org:Site ;
    skos:definition "Indicates a site at which the Organization has some presence even if only indirect (e.g. virtual office or a professional service which is acting as the registered address for a company). Inverse of `org:siteOf`."@en,
        "Indique un site sur lequel l'Organisation possède une présence, même indirecte (domiciliation, boite postale). Inverse de `org:siteOf`."@fr,
        "Duidt de zetel aan waarop de organisatie aanwezig is, zelfs indien indirect (bv. via domiciliëring of postbus). Omgekeerde van `org:siteOf`."@nl .

org:heldBy a rdf:Property,
        owl:ObjectProperty ;
    rdfs:label "held by"@en,
        "occupé par"@fr,
        "bezet door"@nl ;
    rdfs:domain org:Post ;
    rdfs:isDefinedBy <http://www.w3.org/ns/org> ;
    rdfs:range <http://xmlns.com/foaf/0.1/Agent> ;
    owl:inverseOf org:holds ;
    skos:definition "Indicates an Agent which holds a Post."@en,
        "Indique un Agent qui occupe le Poste."@fr,
        "Duidt een Agent aan die een positie heeft."@nl .

org:holds a rdf:Property,
        owl:ObjectProperty ;
    rdfs:label "holds"@en,
        "occupe"@fr,
        "heeft positie"@nl ;
    rdfs:domain <http://xmlns.com/foaf/0.1/Agent> ;
    rdfs:isDefinedBy <http://www.w3.org/ns/org> ;
    rdfs:range org:Post ;
    owl:inverseOf org:heldBy ;
    skos:definition "Indicates a Post held by some Agent."@en,
        "Indicate un Poste occupé par un Agent."@fr,
        "Duidt een positie aan die ingevuld wordt door een Agent."@nl .

org:postIn a rdf:Property,
        owl:ObjectProperty ;
    rdfs:label "post in"@en,
        "poste chez"@fr,
        "positie in"@nl ;
    rdfs:domain org:Post ;
    rdfs:isDefinedBy <http://www.w3.org/ns/org> ;
    rdfs:range org:Organization ;
    owl:inverseOf org:hasPost ;
    skos:definition "Indicates the Organization in which the Post exists."@en,
        "Indicate l'Organisation dans laquelle le Poste existe."@fr,
        "Duidt de organisatie aan waarbij de positie bestaat."@nl .

prov:startedAtTime a owl:DatatypeProperty ;
    rdfs:label "started at time"@en,
        "démarré à l'heure"@fr,
        "gestart op tijdstip"@nl ;
    rdfs:domain prov:Activity ;
    rdfs:isDefinedBy <http://www.w3.org/ns/prov-o#> ;
    rdfs:range xsd:dateTime ;
    skos:definition "The time at which an activity started. See also `prov:endedAtTime`."@en,
        "Le moment où une activité a commencé. Voir aussi `prov:endedAtTime`."@fr,
        "Het tijdstip waarop een activiteit begon. Zie ook `prov:endedAtTime`."@nl .

prov:used a owl:ObjectProperty ;
    rdfs:label "used"@en,
        "a utilisé"@fr,
        "gebruikte"@nl ;
    rdfs:domain prov:Activity ;
    rdfs:isDefinedBy <http://www.w3.org/ns/prov-o#> ;
    rdfs:range prov:Entity ;
    rdfs:subPropertyOf prov:wasInfluencedBy ;
    owl:propertyChainAxiom ( prov:qualifiedUsage prov:entity ) ;
    skos:definition "A `prov:Entity` that was used by this `prov:Activity`. For example, `:baking prov:used :spoon, :egg, :oven .`"@en,
        "Une `prov:Entity` qui a été utilisée par cette `prov:Activity`. Par exemple , `:baking prov:used :cuillère , :œuf , :four.`"@fr,
        "Een `prov:Entity` die door deze `prov:Activity` werd gebruikt. Bijvoorbeeld: `:bakken prov:used :lepel ,:ei, :oven.`"@nl .

prov:wasAssociatedWith a owl:ObjectProperty ;
    rdfs:label "was associated with"@en,
        "a été associé à"@fr,
        "is geassocieerd met"@nl ;
    rdfs:domain prov:Activity ;
    rdfs:isDefinedBy <http://www.w3.org/ns/prov-o#> ;
    rdfs:range prov:Agent ;
    rdfs:subPropertyOf prov:wasInfluencedBy ;
    owl:propertyChainAxiom ( prov:qualifiedAssociation prov:agent ) ;
    skos:definition "An `prov:Agent` that had some (unspecified) responsibility for the occurrence of this `prov:Activity`."@en,
        "Un `prov:Agent` qui avait une responsabilité (non spécifiée) avant la survenue de cette `prov:Activity`."@fr,
        "Een `prov:Agent` die enige (niet-gespecificeerde) verantwoordelijkheid had voor het optreden van deze `prov:Activity`."@nl .

<https://data.hetarchief.be/ns/object/hasAccessCopy> a rdf:Property ;
    rdfs:label "has access copy"@en,
        "a copie d'accès"@fr,
        "heeft toegangskopie"@nl ;
    rdfs:isDefinedBy <https://data.hetarchief.be/ns/object/> ;
    rdfs:subPropertyOf <http://id.loc.gov/vocabulary/preservation/relationshipSubType/isr> ;
    owl:inverseOf <https://data.hetarchief.be/ns/object/isAccessCopyOf> .

<https://data.hetarchief.be/ns/object/hasIIIFCopy> a rdf:Property ;
    rdfs:label "has IIIF copy"@en,
        "a copie IIIF"@fr,
        "heeft IIIF-kopie"@nl ;
    rdfs:isDefinedBy <https://data.hetarchief.be/ns/object/> ;
    rdfs:subPropertyOf <http://id.loc.gov/vocabulary/preservation/relationshipSubType/isr> ;
    owl:inverseOf <https://data.hetarchief.be/ns/object/isIIIFCopyOf> .

<https://data.hetarchief.be/ns/object/hasMasterCopy> a rdf:Property ;
    rdfs:label "has archiving master"@en,
        "a copie principale"@fr,
        "heeft archiefmaster"@nl ;
    rdfs:isDefinedBy <https://data.hetarchief.be/ns/object/> ;
    rdfs:subPropertyOf <http://id.loc.gov/vocabulary/preservation/relationshipSubType/isr> ;
    owl:inverseOf <https://data.hetarchief.be/ns/object/isMasterCopyOf> .

<https://data.hetarchief.be/ns/object/hasMezzanineCopy> a rdf:Property ;
    rdfs:label "has mezzanine format"@en,
        "a format mezzanine"@fr,
        "heeft mezzanineformaat"@nl ;
    rdfs:isDefinedBy <https://data.hetarchief.be/ns/object/> ;
    rdfs:subPropertyOf <http://id.loc.gov/vocabulary/preservation/relationshipSubType/isr> ;
    owl:inverseOf <https://data.hetarchief.be/ns/object/isMezzanineCopyOf> .

<https://data.hetarchief.be/ns/object/hasTranscriptionCopy> a rdf:Property ;
    rdfs:label "has transcription copy"@en,
        "a copie de transcription"@fr,
        "heeft transcriptiekopie"@nl ;
    rdfs:isDefinedBy <https://data.hetarchief.be/ns/object/> ;
    rdfs:subPropertyOf <http://id.loc.gov/vocabulary/preservation/relationshipSubType/isr> ;
    owl:inverseOf <https://data.hetarchief.be/ns/object/isTranscriptionCopyOf> .

<https://data.hetarchief.be/ns/object/isAccessCopyOf> a rdf:Property ;
    rdfs:label "is access copy of"@en,
        "est copie d'accès de"@fr,
        "is toegangskopie van"@nl ;
    rdfs:isDefinedBy <https://data.hetarchief.be/ns/object/> ;
    rdfs:subPropertyOf <http://id.loc.gov/vocabulary/preservation/relationshipSubType/rep> ;
    owl:inverseOf <https://data.hetarchief.be/ns/object/hasAccessCopy> .

<https://data.hetarchief.be/ns/object/isIIIFCopyOf> a rdf:Property ;
    rdfs:label "is IIIF copy of"@en,
        "est copie IIIF de"@fr,
        "is IIIF-kopie van"@nl ;
    rdfs:isDefinedBy <https://data.hetarchief.be/ns/object/> ;
    rdfs:subPropertyOf <http://id.loc.gov/vocabulary/preservation/relationshipSubType/rep> ;
    owl:inverseOf <https://data.hetarchief.be/ns/object/hasIIIFCopy> .

<https://data.hetarchief.be/ns/object/isMasterCopyOf> a rdf:Property ;
    rdfs:label "is archiving master of"@en,
        "est la copie principale de"@fr,
        "is archiefmaster van"@nl ;
    rdfs:isDefinedBy <https://data.hetarchief.be/ns/object/> ;
    rdfs:subPropertyOf <http://id.loc.gov/vocabulary/preservation/relationshipSubType/rep> ;
    owl:inverseOf <https://data.hetarchief.be/ns/object/hasMasterCopy> .

<https://data.hetarchief.be/ns/object/isMezzanineCopyOf> a rdf:Property ;
    rdfs:label "is mezzanine format of"@en,
        "est format mezzanine de"@fr,
        "is mezzanineformaat van"@nl ;
    rdfs:isDefinedBy <https://data.hetarchief.be/ns/object/> ;
    rdfs:subPropertyOf <http://id.loc.gov/vocabulary/preservation/relationshipSubType/rep> ;
    owl:inverseOf <https://data.hetarchief.be/ns/object/hasMezzanineCopy> .

<https://data.hetarchief.be/ns/object/isTranscriptionCopyOf> a rdf:Property ;
    rdfs:label "is transcription copy of"@en,
        "est copie transcription de"@fr,
        "is transcriptiekopie van"@nl ;
    rdfs:isDefinedBy <https://data.hetarchief.be/ns/object/> ;
    rdfs:subPropertyOf <http://id.loc.gov/vocabulary/preservation/relationshipSubType/rep> ;
    owl:inverseOf <https://data.hetarchief.be/ns/object/hasTranscriptionCopy> .

<https://data.hetarchief.be/ns/organization/hasAccountManager> a rdf:Property ;
    rdfs:label "has an account manager"@en,
        "a un gestionnaire de comptes"@fr,
        "heeft een accountmanager"@nl ;
    rdfs:domain org:Organization ;
    rdfs:isDefinedBy <https://data.hetarchief.be/ns/organization/> ;
    rdfs:range schema:Person ;
    owl:inverseOf <https://data.hetarchief.be/ns/organization/isAccountManagerOf> ;
    skos:definition "A person that is the account manager of an organization."@en,
        "Une personne qui est le gestionnaire de comptes d'une organisation."@fr,
        "Een persoon die de accountmanager is van een organisatie."@nl .

<https://data.hetarchief.be/ns/organization/isAccountManagerOf> a rdf:Property ;
    rdfs:label "is account manager of"@en,
        "est gestionnaire de comptes de"@fr,
        "is account manager van"@nl ;
    rdfs:domain schema:Person ;
    rdfs:isDefinedBy <https://data.hetarchief.be/ns/organization/> ;
    rdfs:range org:Organization ;
    owl:inverseOf <https://data.hetarchief.be/ns/organization/hasAccountManager> ;
    skos:definition "An organization that a person is the account manager of."@en,
        "Une organisation dont une personne est le gestionnaire de comptes."@fr,
        "Een organisatie waarvan een persoon de accountmanager is."@nl .

<https://data.hetarchief.be/ns/terms/higherPriority> a rdf:Property ;
    rdfs:label "has higher priority than"@en,
        "a une priorité plus grande que"@fr,
        "heeft een hogere prioriteit dan"@nl ;
    rdfs:domain skos:Concept ;
    rdfs:isDefinedBy <https://data.hetarchief.be/ns/terms/> ;
    rdfs:range skos:Concept ;
    rdfs:subPropertyOf skos:related ;
    owl:inverseOf <https://data.hetarchief.be/ns/terms/lowerPriority> ;
    skos:definition "Relates a concept to a concept that has a higher priority."@en,
        "Relie un concept à un concept qui a une priorité plus élevée."@fr,
        "Relateert een concept aan een ander concept dat een hogere prioriteit heeft."@nl ;
    skos:example "File format XML1.1 is a more recent and thus preferable format over XML1.0; XML1.1 thus holds a higher priority than XML1.0."@en,
        "Le format de fichier XML1.1 est un format plus récent et donc préférable à XML1.0; XML1.1 a donc une priorité plus élevée que XML1.0."@fr,
        "Het bestandsformaat XML1.1 is een recenter en dus verkieslijker formaat dan XML1.0; XML1.1 heeft dus een hogere prioriteit dan XML1.0."@nl .

<https://data.hetarchief.be/ns/terms/lowerPriority> a rdf:Property ;
    rdfs:label "has lower priority than"@en,
        "a une priorité inférieure à"@fr,
        "heeft een lagere prioriteit dan"@nl ;
    rdfs:domain skos:Concept ;
    rdfs:isDefinedBy <https://data.hetarchief.be/ns/terms/> ;
    rdfs:range skos:Concept ;
    rdfs:subPropertyOf skos:related ;
    owl:inverseOf <https://data.hetarchief.be/ns/terms/higherPriority> ;
    skos:definition "Relates a concept to a concept that has a lower priority."@en,
        "Relie un concept à un concept qui a une priorité inférieure."@fr,
        "Relateert een concept aan een ander concept dat een lagere prioriteit heeft."@nl ;
    skos:example "File format XML1.1 is a more recent and thus preferable format over XML1.0; XML1.0 thus holds a lower priority than XML1.1."@en,
        "Le format de fichier XML1.1 est un format plus récent et donc préférable à XML1.0; XML1.0 a donc une priorité inférieure à XML1.1."@fr,
        "Het bestandsformaat XML1.1 is een recenter en dus verkieslijker formaat dan XML1.0; XML1.0 heeft dus een lagere prioriteit dan XML1.1."@nl .

schema:brand a rdf:Property ;
    rdfs:label "brand"@en,
        "marque"@fr,
        "merk"@nl ;
    rdfs:isDefinedBy schema: ;
    skos:definition "The brand(s) associated with a product or service, or the brand(s) maintained by an organization or business person."@en,
        "La (s) marque (s) associée à un produit ou à un service, ou la (s) marque (s) entretenue par une organisation ou un homme d'affaires."@fr,
        "Het merk (en) geassocieerd met een product of service, of het merk (en) dat wordt onderhouden door een organisatie of ondernemer."@nl .

schema:identifier a rdf:Property ;
    rdfs:label "identifier"@en,
        "identifiant"@fr,
        "identifier"@nl ;
    rdfs:domain schema:Thing ;
    rdfs:isDefinedBy schema: ;
    rdfs:range xsd:string ;
    owl:equivalentProperty dct:identifier ;
    skos:definition "The identifier property represents any kind of identifier for any kind of Thing, such as ISBNs, GTIN codes, UUIDs etc."@en,
        "La propriété 'identifier' représente n'importe quel type d'identifiant pour n'importe quel type d'objet (Thing), tels que les ISBNs, les codes GTIN, les UUIDs etc."@fr,
        "De identifier-eigenschap representeert elk soort identifier voor elk soort ding (Thing), zoals ISBNs, GTIN codes, UUIDs enz."@nl .

schema:instrument a rdf:Property ;
    rdfs:label "instrument"@en,
        "instrument"@fr,
        "instrument"@nl ;
    rdfs:isDefinedBy schema: ;
    skos:definition "The object that helped the agent perform the action. E.g. John wrote a book with *a pen*."@en,
        "L'objet qui a aidé l'agent à effectuer l'action. Par exemple: John a écrit un livre avec *un stylo*."@fr,
        "Het object dat de agent heeft geholpen de actie uit te voeren. Bijv. John schreef een boek met *een pen*."@nl .

schema:model a rdf:Property ;
    rdfs:label "model"@en,
        "modèle"@fr,
        "model"@nl ;
    rdfs:isDefinedBy schema: ;
    skos:definition "The model of the product. Use with the URL of a ProductModel or a textual representation of the model identifier. The URL of the ProductModel can be from an external source. It is recommended to additionally provide strong product identifiers via the gtin8/gtin13/gtin14 and mpn properties."@en,
        "Le modèle du produit.Utilisez avec l'URL d'un produit de produit ou une représentation textuelle de l'identifiant du modèle. L'URL du ProductModel peut provenir d'une source externe.Il est recommandé de fournir en outre des identificateurs de produits solides via les propriétés GTIN8 / GTIN13 / GTIN14 et MPN."@fr,
        "Het model van het product.Gebruik met de URL van een productmodel of een tekstuele weergave van de model-ID. De URL van het productmodel kan uit een externe bron zijn.Het wordt aanbevolen om bovendien sterke productidentifiers te bieden via de eigenschappen GTIN8/GTIN13/GTIN14 en MPN."@nl .

schema:serialNumber a rdf:Property ;
    rdfs:label "serialNumber"@en,
        "numéro de série"@fr,
        "serienummer"@nl ;
    rdfs:isDefinedBy schema: ;
    rdfs:subPropertyOf schema:identifier ;
    skos:definition "The serial number or any alphanumeric identifier of a particular product. When attached to an offer, it is a shortcut for the serial number of the product included in the offer."@en,
        "Le numéro de série ou tout identifiant alphanumérique d'un produit particulier. Lorsqu'il est attaché à une offre, il s'agit d'un raccourci pour le numéro de série du produit inclus dans l'offre."@fr,
        "Het serienummer of een alfanumerieke identificatie van een bepaald product. Wanneer het wordt bevestigd aan een aanbieding, is het een snelkoppeling voor het serienummer van het product dat in het aanbod is opgenomen."@nl .

schema:version a rdf:Property ;
    rdfs:label "version"@en,
        "version"@fr,
        "versie"@nl ;
    rdfs:isDefinedBy schema: ;
    skos:definition "The version of the CreativeWork embodied by a specified resource."@en,
        "La version du Creativework incarné par une ressource spécifiée."@fr,
        "De versie van het Creative Work dat is belichaamd door een opgegeven item."@nl .

dct:description a rdfs:Property ;
    rdfs:label "description"@en,
        "description"@fr,
        "beschrijving"@nl ;
    rdfs:isDefinedBy dct: ;
    skos:definition "An account of the resource."@en,
        "Un compte rendu de la ressource."@fr,
        "Een verslag van de resource"@nl .

premis:note a owl:DatatypeProperty ;
    rdfs:label "has note"@en,
        "a note"@fr,
        "heeft nota"@nl ;
    rdfs:isDefinedBy premis: ;
    rdfs:range rdfs:Literal ;
    rdfs:subPropertyOf dct:description .

<http://www.ontologydesignpatterns.org/cp/owl/sequence.owl#follows> a owl:ObjectProperty,
        owl:TransitiveProperty ;
    rdfs:label "follows"@en,
        "suit"@fr,
        "volgt op"@nl ;
    rdfs:domain owl:Thing ;
    rdfs:isDefinedBy <http://www.ontologydesignpatterns.org/cp/owl/sequence.owl> ;
    rdfs:range owl:Thing ;
    skos:definition "A relation between entities, expressing a 'sequence' schema. E.g. 'year 2000 follows 1999', 'preparing coffee' follows 'deciding what coffee to use', 'II World War follows I World War', etc. It can be used between tasks, processes or time intervals, and subproperties would fit best in order to distinguish the different uses."@en,
        "Une relation entre entités, exprimant une 'séquence'. Par exemple, 'l'année 2000 suit l'année 1999', 'préparer du café' suit 'décider quel café à utiliser', 'la Seconde Guerre mondiale suit la Première Guerre mondiale', etc. Il peut être utilisé avec des tâches, des processus ou des intervalles de temps, et des sous-propriétés seraient les meilleures adaptées pour distinguer les différentes utilisations."@fr,
        "Een relatie tussen entiteiten, die een 'sequentie' uitdrukt. Bv. 'het jaar 2000 volgt op het jaar 1999', 'koffie klaarmaken' volgt op 'beslissen welke koffie te gebruiken', 'WO II volgt op WO I', etc. Het kan gebruikt worden bij taken, processen, of tijdsintervallen, en subeigenschappen (subproperties) zouden het best passen om de verschillende gebruiken te onderscheiden."@nl .

skos:broader a rdf:Property,
        owl:ObjectProperty ;
    rdfs:label "has broader"@en,
        "a un concept plus large"@fr,
        "heeft breder concept"@nl ;
    rdfs:comment "Broader concepts are typically rendered as parents in a concept hierarchy (tree)."@en,
        "Les concepts plus larges sont généralement représentés comme des parents dans une hiérarchie de concepts (arbre)."@fr,
        "Bredere concepten worden meestal weergegeven als parents in een concept hiërarchie (boom)."@nl ;
    rdfs:isDefinedBy <http://www.w3.org/2004/02/skos/core> ;
    rdfs:subPropertyOf skos:broaderTransitive ;
    owl:inverseOf skos:narrower ;
    skos:definition "Relates a concept to a concept that is more general in meaning."@en,
        "Relie un concept à un concept qui est plus général dans son sens."@fr,
        "Verbindt een concept met een concept dat in betekenis algemener is."@nl ;
    skos:scopeNote "By convention, skos:broader is only used to assert an immediate (i.e. direct) hierarchical link between two conceptual resources."@en,
        "Par convention, skos:broader est utilisé uniquement pour indiquer un lien hiérarchique direct entre deux ressources conceptuelles."@fr,
        "Volgens conventie wordt skos:broader alleen gebruikt om een directe (dus niet transitieve) hiërarchische link tussen twee conceptuele resources aan te geven."@nl .

skos:broaderTransitive a rdf:Property,
        owl:ObjectProperty,
        owl:TransitiveProperty ;
    rdfs:label "has broader transitive"@en,
        "a un concept plus large (transitive)"@fr,
        "heeft breder concept (transitief)"@nl ;
    rdfs:isDefinedBy <http://www.w3.org/2004/02/skos/core> ;
    rdfs:subPropertyOf skos:semanticRelation ;
    owl:inverseOf skos:narrowerTransitive ;
    skos:definition "`skos:broaderTransitive` is a transitive superproperty of `skos:broader`."@en,
        "`skos:broaderTransitive` est une superpropriété transitive de `skos:broader`."@fr,
        "`skos:broaderTransitive` is een transitieve superproperty van `skos:broader`."@nl ;
    skos:scopeNote "By convention, skos:broaderTransitive is not used to make assertions. Rather, the properties can be used to draw inferences about the transitive closure of the hierarchical relation, which is useful e.g. when implementing a simple query expansion algorithm in a search application."@en,
        "Par convention, skos:broaderTransitive n'est pas utilisé pour faire des assertions. A la place, les propriétés peuvent être utilisées pour tirer des inferences sur la fermeture transitive de la relation hiérarchique, ce qui est utile par exemple lors de l'implémentation d'un algorithme simple d'expansion de requête dans une application de recherche."@fr,
        "Volgens conventie wordt skos:broaderTransitive niet gebruikt om beweringen te doen. De eigenschappen kunnen wel gebruikt worden om inferenties te trekken over de transitieve sluiting van de hiërarchische relatie, wat bijvoorbeeld handig is bij het implementeren van een eenvoudige queryexpansie-algoritme in een zoekapplicatie."@nl .

skos:narrower a rdf:Property,
        owl:ObjectProperty ;
    rdfs:label "has narrower"@en,
        "a un concept plus restreint"@fr,
        "heeft nauwer concept"@nl ;
    rdfs:comment "Narrower concepts are typically rendered as children in a concept hierarchy (tree)."@en,
        "Les concepts plus restreints sont généralement représentés comme des enfants dans une hiérarchie de concepts (arbre)."@fr,
        "Nauwere concepten worden meestal weergegeven als kinderen in een concepthiërarchie (boom)."@nl ;
    rdfs:isDefinedBy <http://www.w3.org/2004/02/skos/core> ;
    rdfs:subPropertyOf skos:narrowerTransitive ;
    owl:inverseOf skos:broader ;
    skos:definition "Relates a concept to a concept that is more specific in meaning."@en,
        "Relie un concept à un concept qui est plus spécifique dans son sens."@fr,
        "Verbindt een concept met een concept dat in betekenis meer specifiek is."@nl ;
    skos:scopeNote "By convention, skos:broader is only used to assert an immediate (i.e. direct) hierarchical link between two conceptual resources."@en,
        "Par convention, skos:broader est utilisé uniquement pour indiquer un lien hiérarchique direct entre deux ressources conceptuelles."@fr,
        "Volgens conventie wordt skos:broader alleen gebruikt om een directe (dus niet transitieve) hiërarchische link tussen twee conceptuele resources aan te geven."@nl .

skos:narrowerTransitive a rdf:Property,
        owl:ObjectProperty,
        owl:TransitiveProperty ;
    rdfs:label "has narrower transitive"@en,
        "a un concept plus restreint (transitive)"@fr,
        "heeft nauwer concept (transitief)"@nl ;
    rdfs:isDefinedBy <http://www.w3.org/2004/02/skos/core> ;
    rdfs:subPropertyOf skos:semanticRelation ;
    owl:inverseOf skos:broaderTransitive ;
    skos:definition "`skos:narrowerTransitive` is a transitive superproperty of `skos:narrower`."@en,
        "`skos:narrowerTransitive` est une superpropriété transitive de `skos:narrower`."@fr,
        "`skos:narrowerTransitive` is een transitieve superproperty van `skos:narrower`."@nl ;
    skos:scopeNote "By convention, skos:narrowerTransitive is not used to make assertions. Rather, the properties can be used to draw inferences about the transitive closure of the hierarchical relation, which is useful e.g. when implementing a simple query expansion algorithm in a search application."@en,
        "Par convention, skos:narrowerTransitive n'est pas utilisé pour faire des assertions. A la place, les propriétés peuvent être utilisées pour tirer des inferences sur la fermeture transitive de la relation hiérarchique, ce qui est utile par exemple lors de l'implémentation d'un algorithme simple d'expansion de requête dans une application de recherche."@fr,
        "Volgens conventie wordt skos:narrowerTransitive niet gebruikt om beweringen te doen. De eigenschappen kunnen wel gebruikt worden om inferenties te trekken over de transitieve sluiting van de hiërarchische relatie, wat bijvoorbeeld handig is bij het implementeren van een eenvoudig queryexpansie-algoritme in een zoekapplicatie."@nl .

prov:generated a owl:ObjectProperty ;
    rdfs:label "generated"@en,
        "a généré"@fr,
        "genereerde"@nl ;
    rdfs:domain prov:Activity ;
    rdfs:isDefinedBy <http://www.w3.org/ns/prov-o#> ;
    rdfs:range prov:Entity ;
    rdfs:subPropertyOf prov:influenced ;
    owl:inverseOf prov:wasGeneratedBy .

prov:wasGeneratedBy a owl:ObjectProperty ;
    rdfs:label "was generated by"@en,
        "a été généré par"@fr,
        "is gegenereerd door"@nl ;
    rdfs:domain prov:Entity ;
    rdfs:isDefinedBy <http://www.w3.org/ns/prov-o#> ;
    rdfs:range prov:Activity ;
    rdfs:subPropertyOf prov:wasInfluencedBy ;
    owl:propertyChainAxiom ( prov:qualifiedGeneration prov:activity ) .

<https://data.hetarchief.be/ns/event#NameShape> a sh:PropertyShape ;
    sh:datatype rdf:langString ;
    sh:maxCount 1 ;
    sh:message "schema:name is missing or not of type string "@en,
        "schema:name est manquant ou n'est pas de type string"@fr,
        "schema:name ontbreekt of is niet van het type string"@nl ;
    sh:minCount 1 ;
    sh:name "name"@en,
        "nom"@fr,
        "naam"@nl ;
    sh:nodeKind sh:Literal ;
    sh:path schema:name ;
    sh:severity sh:Violation .

<https://data.hetarchief.be/ns/event#brandShape> a sh:PropertyShape ;
    sh:class schema:Brand ;
    sh:description "The particular brand of the Agent."@en,
        "La marque particulière de l'agent."@fr,
        "Het specifieke merk van de agent."@nl ;
    sh:maxCount 1 ;
    sh:message "schema:brand occurs more than once or its value is no instance of schema:Brand"@en ;
    sh:minCount 0 ;
    sh:name "brand"@en,
        "marque"@fr,
        "merk"@nl ;
    sh:path schema:brand ;
    sh:severity sh:Violation .

<https://data.hetarchief.be/ns/event#modelShape> a sh:PropertyShape ;
    sh:datatype xsd:string ;
    sh:description "The particular model of the Agent."@en,
        "La modèle particulière de l'agent."@fr,
        "Het specifieke model van de agent."@nl ;
    sh:maxCount 1 ;
    sh:message "schema:model occurs more than once or its value is no string"@en ;
    sh:minCount 0 ;
    sh:name "model"@en,
        "modèle"@fr,
        "model"@nl ;
    sh:path schema:model ;
    sh:severity sh:Violation .

<https://data.hetarchief.be/ns/event#serialNumberShape> a sh:PropertyShape ;
    sh:datatype xsd:string ;
    sh:description "The serial number or any alphanumeric identifier of a particular agent."@en,
        "Le numéro de série ou tout identifiant alphanumérique d'un agent particulier."@fr,
        "Het serienummer of een alfanumerieke identificatie van een bepaald middel."@nl ;
    sh:maxCount 1 ;
    sh:message "schema:serialNumber occurs more than once or its value is no string"@en ;
    sh:minCount 0 ;
    sh:name "serialNumber"@en,
        "numéro de série"@fr,
        "serienummer"@nl ;
    sh:path schema:serialNumber ;
    sh:severity sh:Violation .

<https://data.hetarchief.be/ns/event#versionShape> a sh:PropertyShape ;
    sh:datatype xsd:string ;
    sh:description "The agent's version number or version name."@en,
        "Le numéro de version de l'agent ou le nom de la version."@fr,
        "Het versienummer of versienaam van de agent."@nl ;
    sh:maxCount 1 ;
    sh:message "schema:version occurs more than once or its value is no string"@en ;
    sh:minCount 0 ;
    sh:name "version"@en,
        "version"@fr,
        "versie"@nl ;
    sh:path schema:version ;
    sh:severity sh:Violation .

schema:name a rdf:Property ;
    rdfs:label "name"@en,
        "nom"@fr,
        "naam"@nl ;
    rdfs:domain schema:Thing ;
    rdfs:isDefinedBy schema: ;
    rdfs:range xsd:string ;
    owl:equivalentProperty dct:title ;
    skos:definition "The name of the item."@en,
        "Le nom de l'article."@fr,
        "De naam van het item."@nl .

skos:related a rdf:Property,
        owl:ObjectProperty,
        owl:SymmetricProperty ;
    rdfs:label "has related"@en,
        "a un concept lié"@fr,
        "heeft gerelateerd concept"@nl ;
    rdfs:comment "skos:related is disjoint with skos:broaderTransitive"@en,
        "skos:related est disjoint avec skos:broaderTransitive"@fr,
        "skos:related is disjunct met skos:broaderTransitive"@nl ;
    rdfs:isDefinedBy <http://www.w3.org/2004/02/skos/core> ;
    rdfs:subPropertyOf skos:semanticRelation ;
    skos:definition "Relates a concept to a concept with which there is an associative semantic relationship."@en,
        "Relie un concept à un concept avec lequel il existe une relation sémantique associative."@fr,
        "Verbindt een concept met een concept waarmee er een associatieve semantische relatie is."@nl .

skos:mappingRelation a rdf:Property,
        owl:ObjectProperty ;
    rdfs:label "is in mapping relation with"@en,
        "est en relation de correspondance avec"@fr,
        "heeft een mappingrelatie met"@nl ;
    rdfs:comment "These concept mapping relations mirror semantic relations, and the data model defined below is similar (with the exception of skos:exactMatch) to the data model defined for semantic relations. A distinct vocabulary is provided for concept mapping relations, to provide a convenient way to differentiate links within a concept scheme from links between concept schemes. However, this pattern of usage is not a formal requirement of the SKOS data model, and relies on informal definitions of best practice."@en,
        "Ces relations de correspondance de concepts reflètent les relations sémantiques, et le modèle de données défini ci-dessous est similaire (à l'exception de skos:exactMatch) au modèle de données défini pour les relations sémantiques. Un vocabulaire distinct est fourni pour les relations de correspondance de concepts, pour fournir un moyen pratique de différencier les liens à l'intérieur d'un schéma de concepts des liens entre les schémas de concepts. Cependant, ce modèle d'utilisation n'est pas une exigence formelle du modèle de données SKOS, et repose sur des définitions informelles des meilleures pratiques."@fr,
        "Deze conceptmappingrelaties spiegelen semantische relaties, en het datamodel hieronder is vergelijkbaar (met uitzondering van skos:exactMatch) met het datamodel gedefinieerd voor semantische relaties. Een apart vocabularium is voorzien voor conceptmappingrelaties, om een handige manier te bieden om het onderscheid te maken tussen links binnen een conceptenschema en links tussen conceptenschema's. Deze manier van gebruik is echter geen formele vereiste van het SKOS datamodel, en is afhankelijk van informele definities van best practices."@nl ;
    rdfs:isDefinedBy <http://www.w3.org/2004/02/skos/core> ;
    rdfs:subPropertyOf skos:semanticRelation ;
    skos:definition "Relates two concepts coming, by convention, from different schemes, and that have comparable meanings"@en,
        "Relie deux concepts provenant, par convention, de schémas différents, et qui ont des sens comparables"@fr,
        "Verbindt twee concepten die, door conventie, uit verschillende schema's komen en vergelijkbare betekenissen hebben"@nl .

skos:semanticRelation a rdf:Property,
        owl:ObjectProperty ;
    rdfs:label "is in semantic relation with"@en,
        "est en relation sémantique avec"@fr,
        "heeft een semantische relatie met"@nl ;
    rdfs:domain skos:Concept ;
    rdfs:isDefinedBy <http://www.w3.org/2004/02/skos/core> ;
    rdfs:range skos:Concept ;
    skos:definition "Links a concept to a concept related by meaning."@en,
        "Liaison d'un concept à un concept lié par sens."@fr,
        "Verbindt een concept met een concept dat op basis van de betekenis gerelateerd is."@nl ;
    skos:scopeNote "This property should not be used directly, but as a super-property for all properties denoting a relationship of meaning between concepts."@en,
        "Cette propriété ne doit pas être utilisée directement, mais comme super-propriété pour toutes les propriétés désignant une relation de sens entre concepts."@fr,
        "Deze eigenschap moet niet direct gebruikt worden, maar als super-eigenschap voor alle eigenschappen die een betekenisrelatie tussen concepten aanduiden."@nl .

<http://id.loc.gov/vocabulary/preservation/relationshipSubType/isr> a owl:ObjectProperty ;
    rdfs:label "is Represented by"@en,
        "est représenté par"@fr,
        "wordt gerepresenteerd door"@nl ;
    rdfs:isDefinedBy <http://id.loc.gov/vocabulary/preservation/relationshipSubType> ;
    rdfs:subPropertyOf premis:relationship ;
    skos:definition "A relationship in which an abstract intellectual entity is represented as a file or representation or a software agent is represented by an environment object. Has a reciprocal relationship of represents."@en,
        "Relation dans laquelle une entité intellectuelle (intellectual entity) abstraite est représentée par un fichier (file) ou une représentation (representation) ou un logiciel est représenté par un objet d'environnement. A une relation réciproque avec represents."@fr,
        "Een relatie waarin een abstracte intellectuele entiteit (intellectual entity) wordt gerepresenteerd als een bestand (file) of representatie (representatie), of een software-agent wordt gerepresenteerd door een omgevingsobject. Heeft een wederkerige relatie met represents."@nl .

<http://id.loc.gov/vocabulary/preservation/relationshipSubType/rep> a owl:ObjectProperty ;
    rdfs:label "represents"@en,
        "représente"@fr,
        "representeert"@nl ;
    rdfs:isDefinedBy <http://id.loc.gov/vocabulary/preservation/relationshipSubType> ;
    rdfs:subPropertyOf premis:relationship ;
    skos:definition "A relationship in which a file or representation is captured in an abstract intellectual entity description that it represents. It is a statement of what can depict or stand for the Intellectual Entity. Has a reciprocal relationship of isRepresentedBy."@en,
        "Une relation dans laquelle un fichier (file) ou une représentation (representation) est capturé dans une description abstraite de l'entité intellectuelle (intellectual entity) qu'elle représente. Il s'agit d'une déclaration de ce qui peut dépeindre ou représenter l'entité intellectuelle (intellectual entity). A une relation réciproque avec isRepresentedBy."@fr,
        "Een relatie waarin een bestand (file) of representatie (representation) wordt vastgelegd in een abstracte intellectuele entiteitsbeschrijving die het representeert. Het is een verklaring van wat de Intellectuele Entiteit kan afbeelden of vertegenwoordigen. Heeft een wederkerige relatie met isRepresentedBy."@nl .

skos:note a rdf:Property,
        owl:AnnotationProperty ;
    rdfs:label "note"@en,
        "note"@fr,
        "notitie"@nl ;
    rdfs:isDefinedBy <http://www.w3.org/2004/02/skos/core> ;
    skos:definition "A general note, for any purpose."@en,
        "Une note générale, pour tout usage."@fr,
        "Een algemene notitie, voor eender welk doel."@nl ;
    skos:scopeNote "This property may be used directly, or as a super-property for more specific note types."@en,
        "Cette propriété peut être utilisée directement, ou comme super-propriété pour des types de notes plus spécifiques."@fr,
        "Deze eigenschap kan direct gebruikt worden, of als super-eigenschap voor meer specifieke notitietypes."@nl .

<http://www.w3.org/2008/05/skos-xl> a owl:Ontology ;
    dct:contributor "Participants in W3C's Semantic Web Deployment Working Group."@en ;
    dct:creator "Alistair Miles",
        "Sean Bechhofer" ;
    dct:description "An RDF vocabulary extending SKOS and allowing the description and linking of lexical entities."@en ;
    dct:title "SKOS XL Vocabulary"@en ;
    rdfs:seeAlso <http://www.w3.org/2008/05/skos> ;
    owl:imports <http://www.w3.org/2004/02/skos/core> .

premis:relationship a owl:ObjectProperty ;
    rdfs:label "has relationship"@en,
        "a une relation"@fr,
        "heeft een relatie"@nl ;
    rdfs:domain [ a owl:Class ;
            owl:unionOf ( premis:Agent premis:Object ) ] ;
    rdfs:isDefinedBy premis: ;
    rdfs:range premis:Object ;
    rdfs:seeAlso <http://id.loc.gov/vocabulary/preservation/relationshipSubType> .

<http://www.w3.org/2004/02/skos/core> a owl:Ontology ;
    dct:contributor "Dave Beckett",
        "Nikki Rogers",
        "Participants in W3C's Semantic Web Deployment Working Group."@en ;
    dct:creator "Alistair Miles",
        "Sean Bechhofer" ;
    dct:description "An RDF vocabulary for describing the basic structure and content of concept schemes such as thesauri, classification schemes, subject heading lists, taxonomies, 'folksonomies', other types of controlled vocabulary, and also concept schemes embedded in glossaries and terminologies."@en,
        "Un vocabulaire RDF pour décrire la structure et le contenu de schémas de concepts tels que les thésaurus, les schémas de classification, les listes de sujets, les taxonomies, les 'folksonomies', d'autres types de vocabulaires contrôlés, et aussi des schémas de concepts intégrés dans des glossaires et des terminologies."@fr,
        "Een RDF-vocabularium voor het beschrijven van de basisstructuur en inhoud van conceptenschema's (concept schemes) zoals thesauri, classificatieschema’s, 'subject heading' lijsten, taxonomieën, folksonomieën, andere soorten gecontroleerde vocabularia, alsook conceptenschema's die geïntegreerd zijn in glossaria en terminologieën."@nl ;
    dct:title "SKOS Vocabulary"@en,
        "Vocabulaire SKOS"@fr,
        "SKOS Vocabularium"@nl ;
    rdfs:seeAlso <http://www.w3.org/TR/skos-reference/> .

